@prefix cs: <http://pid.geoscience.gov.au/def/Association_Type> .
@prefix dcterms: <http://purl.org/dc/terms/> .
@prefix rdfs: <http://www.w3.org/2000/01/rdf-schema#> .
@prefix sdo: <https://schema.org/> .
@prefix skos: <http://www.w3.org/2004/02/skos/core#> .
@prefix xsd: <http://www.w3.org/2001/XMLSchema#> .

<http://pid.geoscience.gov.au/def/Association_Type/collective_title> a skos:Concept ;
    rdfs:isDefinedBy cs: ;
    skos:definition "common title for a collection of resources where title identifies elements of a series collectively, combined with information about what volumes are available at the source cite"@en ;
    skos:inScheme cs: ;
    skos:prefLabel "collective title"@en ;
    skos:topConceptOf cs: .

<http://pid.geoscience.gov.au/def/Association_Type/cross_reference> a skos:Concept ;
    rdfs:isDefinedBy cs: ;
    skos:definition "reference from one resource to another"@en ;
    skos:inScheme cs: ;
    skos:prefLabel "cross reference"@en ;
    skos:topConceptOf cs: .

<http://pid.geoscience.gov.au/def/Association_Type/dependency> a skos:Concept ;
    rdfs:isDefinedBy cs: ;
    skos:definition "associated through a dependency"@en ;
    skos:inScheme cs: ;
    skos:prefLabel "dependency"@en ;
    skos:topConceptOf cs: .

<http://pid.geoscience.gov.au/def/Association_Type/generated> a skos:Concept ;
    rdfs:isDefinedBy cs: ;
    skos:definition "inverse of wasGeneratedBy where the domain resource generated the range resoure implying that the domain resource is a temporal event."@en ;
    skos:inScheme cs: ;
    skos:prefLabel "generated"@en ;
    skos:scopeNote "inverse of wasGeneratedBy where the domain resource generated the range resoure implying that the domain resource is a temporal event, such as a data processing action, and the range resource is an entity"@en ;
    skos:topConceptOf cs: .

<http://pid.geoscience.gov.au/def/Association_Type/had_derivation> a skos:Concept ;
    rdfs:isDefinedBy cs: ;
    skos:definition "inverse of wasDerivedFrom where the range resource was derived from the domain resource"@en ;
    skos:inScheme cs: ;
    skos:prefLabel "had derivation"@en ;
    skos:topConceptOf cs: .

<http://pid.geoscience.gov.au/def/Association_Type/informed> a skos:Concept ;
    rdfs:isDefinedBy cs: ;
    skos:definition "inverse of wasInformedBy "@en ;
    skos:inScheme cs: ;
    skos:prefLabel "informed"@en ;
    skos:topConceptOf cs: .

<http://pid.geoscience.gov.au/def/Association_Type/is_composed_of> a skos:Concept ;
    rdfs:isDefinedBy cs: ;
    skos:definition "reference to resources that are parts of this resource"@en ;
    skos:inScheme cs: ;
    skos:prefLabel "is composed of"@en ;
    skos:topConceptOf cs: .

<http://pid.geoscience.gov.au/def/Association_Type/larger_work_citation> a skos:Concept ;
    rdfs:isDefinedBy cs: ;
    skos:definition "reference to a master resource of which this one is a part"@en ;
    skos:inScheme cs: ;
    skos:prefLabel "larger work citation"@en ;
    skos:topConceptOf cs: .

<http://pid.geoscience.gov.au/def/Association_Type/operated_on_by> a skos:Concept ;
    rdfs:isDefinedBy cs: ;
    skos:definition "inverse of operatesOn where the domain resource is, or can be, operated on (queried, subsetted etc.) by the range resource which must be an agent"@en ;
    skos:inScheme cs: ;
    skos:prefLabel "operated on by"@en ;
    skos:scopeNote "inverse of operatesOn where the domain resource is, or can be, operated on (queried, subsetted etc.) by the range resource which must be an agent (i.e. is something that bears some form of responsibility for the operation taking place)"@en ;
    skos:topConceptOf cs: .

<http://pid.geoscience.gov.au/def/Association_Type/operates_on> a skos:Concept ;
    rdfs:isDefinedBy cs: ;
    skos:definition "an equivalent relationship to srv:operatesOn from a Service to a Dataset"@en ;
    skos:inScheme cs: ;
    skos:prefLabel "operates on"@en ;
    skos:topConceptOf cs: .

<http://pid.geoscience.gov.au/def/Association_Type/part_of_a_seamless_database> a skos:Concept ;
    rdfs:isDefinedBy cs: ;
    skos:definition "part of same structured set of data held in a computer"@en ;
    skos:inScheme cs: ;
    skos:prefLabel "part of a seamless database"@en ;
    skos:topConceptOf cs: .

<http://pid.geoscience.gov.au/def/Association_Type/revision_of> a skos:Concept ;
    rdfs:isDefinedBy cs: ;
    skos:definition "resource is a revision of associated resource"@en ;
    skos:inScheme cs: ;
    skos:prefLabel "revision of"@en ;
    skos:topConceptOf cs: .

<http://pid.geoscience.gov.au/def/Association_Type/series> a skos:Concept ;
    rdfs:isDefinedBy cs: ;
    skos:definition "associated through a common heritage such as produced to a common product specification"@en ;
    skos:inScheme cs: ;
    skos:prefLabel "series"@en ;
    skos:topConceptOf cs: .

<http://pid.geoscience.gov.au/def/Association_Type/stereo_mate> a skos:Concept ;
    rdfs:isDefinedBy cs: ;
    skos:definition "part of a set of imagery that when used together, provides three-dimensional images"@en ;
    skos:inScheme cs: ;
    skos:prefLabel "stereo mate"@en ;
    skos:topConceptOf cs: .

<http://pid.geoscience.gov.au/def/Association_Type/was_derived_from> a skos:Concept ;
    rdfs:isDefinedBy cs: ;
    skos:definition "the domain resource was derived from the range resource which must have been an entity (i.e. not an actor with agency or a temporal event)"@en ;
    skos:inScheme cs: ;
    skos:prefLabel "was derived from"@en ;
    skos:topConceptOf cs: .

<http://pid.geoscience.gov.au/def/Association_Type/was_generated_by> a skos:Concept ;
    rdfs:isDefinedBy cs: ;
    skos:definition "the domain resource was generated by the range resource which must have been a temporal event such as a data processing action or a field survey"@en ;
    skos:inScheme cs: ;
    skos:prefLabel "was generated by"@en ;
    skos:topConceptOf cs: .

<http://pid.geoscience.gov.au/def/Association_Type/was_informed_by> a skos:Concept ;
    rdfs:isDefinedBy cs: ;
    skos:definition "The domain resource was informed by the range resource which must have been an Entity (i.e. not an Agent with agency or an Activity temporal event)."@en ;
    skos:inScheme cs: ;
    skos:prefLabel "was informed by"@en ;
    skos:scopeNote "The domain resource was informed by the range resource which must have been an Entity (i.e. not an Agent with agency or an Activity temporal event).This is a looser association than wasDerivedFrom and does not indicate direct derivation, as wasDerivedFrom does."@en ;
    skos:topConceptOf cs: .

<https://linked.data.gov.au/org/ga/voc-wg> a sdo:Organization ;
    sdo:affiliation <https://linked.data.gov.au/org/ga> ;
    sdo:name "Geoscience Australia Vocabulary Working Group" ;
    sdo:url <https://www.ga.gov.au/data-pubs/datastandards> .

<https://linked.data.gov.au/org/ga> a sdo:Organization ;
    sdo:name "Geoscience Australia" ;
    sdo:url <https://www.ga.gov.au> .

cs: a skos:ConceptScheme ;
    dcterms:created "2019-03-12T11:48:09"^^xsd:dateTime ;
    dcterms:creator <https://linked.data.gov.au/org/ga/voc-wg> ;
    dcterms:modified "2019-03-12T11:48:09"^^xsd:dateTime ;
    dcterms:provenance "GA's ORAPROD database tables"@en ;
    dcterms:publisher <https://linked.data.gov.au/org/ga> ;
    skos:changeNote "This vocabulary created directly from the database"@en ;
    skos:definition "Geoscience Australia's 12-Mar-2019 version of the Association Type vocabulary"@en ;
    skos:hasTopConcept <http://pid.geoscience.gov.au/def/Association_Type/collective_title>,
        <http://pid.geoscience.gov.au/def/Association_Type/cross_reference>,
        <http://pid.geoscience.gov.au/def/Association_Type/dependency>,
        <http://pid.geoscience.gov.au/def/Association_Type/generated>,
        <http://pid.geoscience.gov.au/def/Association_Type/had_derivation>,
        <http://pid.geoscience.gov.au/def/Association_Type/informed>,
        <http://pid.geoscience.gov.au/def/Association_Type/is_composed_of>,
        <http://pid.geoscience.gov.au/def/Association_Type/larger_work_citation>,
        <http://pid.geoscience.gov.au/def/Association_Type/operated_on_by>,
        <http://pid.geoscience.gov.au/def/Association_Type/operates_on>,
        <http://pid.geoscience.gov.au/def/Association_Type/part_of_a_seamless_database>,
        <http://pid.geoscience.gov.au/def/Association_Type/revision_of>,
        <http://pid.geoscience.gov.au/def/Association_Type/series>,
        <http://pid.geoscience.gov.au/def/Association_Type/stereo_mate>,
        <http://pid.geoscience.gov.au/def/Association_Type/was_derived_from>,
        <http://pid.geoscience.gov.au/def/Association_Type/was_generated_by>,
        <http://pid.geoscience.gov.au/def/Association_Type/was_informed_by> ;
    skos:prefLabel "Association Type"@en .

