@prefix cs: <http://pid.geoscience.gov.au/def/Data_Types> .
@prefix dcterms: <http://purl.org/dc/terms/> .
@prefix sdo: <https://schema.org/> .
@prefix skos: <http://www.w3.org/2004/02/skos/core#> .
@prefix xsd: <http://www.w3.org/2001/XMLSchema#> .

<http://pid.geoscience.gov.au/def/Data_Types/BATH> a skos:Concept ;
    skos:altLabel "BATH"@en ;
    skos:definition "MANDATORY FIELD"@en ;
    skos:inScheme cs: ;
    skos:prefLabel "Bathymetry data"@en ;
    skos:topConceptOf cs: .

<http://pid.geoscience.gov.au/def/Data_Types/ECO> a skos:Concept ;
    skos:altLabel "ECO"@en ;
    skos:definition "MANDATORY FIELD"@en ;
    skos:inScheme cs: ;
    skos:prefLabel "Ecological/Habitat data"@en ;
    skos:topConceptOf cs: .

<http://pid.geoscience.gov.au/def/Data_Types/ELE> a skos:Concept ;
    skos:altLabel "ELE"@en ;
    skos:definition "MANDATORY FIELD"@en ;
    skos:inScheme cs: ;
    skos:prefLabel "Elevation data"@en ;
    skos:topConceptOf cs: .

<http://pid.geoscience.gov.au/def/Data_Types/FDE> a skos:Concept ;
    skos:altLabel "FDE"@en ;
    skos:definition "MANDATORY FIELD"@en ;
    skos:inScheme cs: ;
    skos:prefLabel "Electromagnetic data, Frequency-domain "@en ;
    skos:topConceptOf cs: .

<http://pid.geoscience.gov.au/def/Data_Types/GEOL> a skos:Concept ;
    skos:altLabel "GEOL"@en ;
    skos:definition "MANDATORY FIELD"@en ;
    skos:inScheme cs: ;
    skos:prefLabel "Geology data"@en ;
    skos:topConceptOf cs: .

<http://pid.geoscience.gov.au/def/Data_Types/GRAV> a skos:Concept ;
    skos:altLabel "GRAV"@en ;
    skos:definition "MANDATORY FIELD"@en ;
    skos:inScheme cs: ;
    skos:prefLabel "Gravity data"@en ;
    skos:topConceptOf cs: .

<http://pid.geoscience.gov.au/def/Data_Types/HYDROBAOFS> a skos:Concept ;
    skos:altLabel "HYDROBAOFS"@en ;
    skos:definition "The British Admiralty was responsible for the charting of Australian waters until this task was taken over by the Royal Australian Navy.  These are the original fairsheets (using lead line sounding) u"@en ;
    skos:inScheme cs: ;
    skos:prefLabel "Hydrographic Soundings - BA (British Admiralty) Original Fairsheets"@en ;
    skos:scopeNote "The British Admiralty was responsible for the charting of Australian waters until this task was taken over by the Royal Australian Navy.  These are the original fairsheets (using lead line sounding) used to produce the British Admiralty charts"@en ;
    skos:topConceptOf cs: .

<http://pid.geoscience.gov.au/def/Data_Types/HYDROBASC> a skos:Concept ;
    skos:altLabel "HYDROBASC"@en ;
    skos:definition "The British Admiralty was responsible for the charting of Australian waters until this task was taken over by the Royal Australian Navy.  All of these charts have now been superceded by Australian cha"@en ;
    skos:inScheme cs: ;
    skos:prefLabel "Hydrographic Soundings - BA (British Admiralty) Superseded Charts"@en ;
    skos:scopeNote "The British Admiralty was responsible for the charting of Australian waters until this task was taken over by the Royal Australian Navy.  All of these charts have now been superceded by Australian charts"@en ;
    skos:topConceptOf cs: .

<http://pid.geoscience.gov.au/def/Data_Types/HYDROFS_NOTRAN> a skos:Concept ;
    skos:altLabel "HYDROFS_NOTRAN"@en ;
    skos:definition "Fairsheet data is Hydrographic Sounding data that has been checked for accuracy and plotted onto a paper fairsheet as the penultimate stage of producing charts for navigation.  These fairsheets could "@en ;
    skos:inScheme cs: ;
    skos:prefLabel "Hydrographic Soundings - Sounding Fairsheets (State Govt, International, commercial)"@en ;
    skos:scopeNote "Fairsheet data is Hydrographic Sounding data that has been checked for accuracy and plotted onto a paper fairsheet as the penultimate stage of producing charts for navigation.  These fairsheets could have been produced by computer plotting or hand plotting the soundings.  They were produced by State Government Agencies, International Organisations or Commercial Entities. "@en ;
    skos:topConceptOf cs: .

<http://pid.geoscience.gov.au/def/Data_Types/HYDROFS_RANCG> a skos:Concept ;
    skos:altLabel "HYDROFS_RANCG"@en ;
    skos:definition "Fairsheet data is Hydrographic Sounding data that has been checked for accuracy and plotted onto a paper fairsheet as the penultimate stage of producing charts for navigation.  These fairsheets have b"@en ;
    skos:inScheme cs: ;
    skos:prefLabel "Hydrographic Soundings - Sounding Fairsheets (RAN, Computer Generated)"@en ;
    skos:scopeNote "Fairsheet data is Hydrographic Sounding data that has been checked for accuracy and plotted onto a paper fairsheet as the penultimate stage of producing charts for navigation.  These fairsheets have been made by computer plotting the soundings.  They were produced by the Royal Australian Navy "@en ;
    skos:topConceptOf cs: .

<http://pid.geoscience.gov.au/def/Data_Types/HYDROFS_RANHD> a skos:Concept ;
    skos:altLabel "HYDROFS_RANHD"@en ;
    skos:definition "Fairsheet data is Hydrographic Sounding data that has been checked for accuracy and plotted onto a paper fairsheet as the penultimate stage of producing charts for navigation.  These fairsheets have b"@en ;
    skos:inScheme cs: ;
    skos:prefLabel "Hydrographic Soundings - Sounding Fairsheets (RAN, Hand Drawn and Numbered)"@en ;
    skos:scopeNote "Fairsheet data is Hydrographic Sounding data that has been checked for accuracy and plotted onto a paper fairsheet as the penultimate stage of producing charts for navigation.  These fairsheets have been made by hand plotting the soundings.  They were produced by the Royal Australian Navy "@en ;
    skos:topConceptOf cs: .

<http://pid.geoscience.gov.au/def/Data_Types/HYDROGEBCOSS> a skos:Concept ;
    skos:altLabel "HYDROGEBCOSS"@en ;
    skos:definition "The General Bathymetric Charts of the Oceans are produced under the auspices of the IHO and IHB using shiptrack data from many nations.  These are sounding sheets used to produce the GEBCO charts.  Th"@en ;
    skos:inScheme cs: ;
    skos:prefLabel "Hydrographic Soundings - GEBCO (General Bathymetric Chart of the Oceans) Sounding Sheets"@en ;
    skos:scopeNote "The General Bathymetric Charts of the Oceans are produced under the auspices of the IHO and IHB using shiptrack data from many nations.  These are sounding sheets used to produce the GEBCO charts.  These have been superceded by a new GEBCO centenary edition digital product. "@en ;
    skos:topConceptOf cs: .

<http://pid.geoscience.gov.au/def/Data_Types/HYDROGEBCOTPS> a skos:Concept ;
    skos:altLabel "HYDROGEBCOTPS"@en ;
    skos:definition "The General Bathymetric Charts of the Oceans are produced under the auspices of the IHO and IHB using shiptrack data from many nations.  These charts show the loaction of the shiptracks used to produc"@en ;
    skos:inScheme cs: ;
    skos:prefLabel "Hydrographic Soundings - GEBCO (General Bathymetric Chart of the Oceans) Track plot Sheets"@en ;
    skos:scopeNote "The General Bathymetric Charts of the Oceans are produced under the auspices of the IHO and IHB using shiptrack data from many nations.  These charts show the loaction of the shiptracks used to produce the GEBCO charts.  These have been superceded by a new GEBCO centenary edition digital product. "@en ;
    skos:topConceptOf cs: .

<http://pid.geoscience.gov.au/def/Data_Types/HYDROICCAUST> a skos:Concept ;
    skos:altLabel "HYDROICCAUST"@en ;
    skos:definition "Sheets showing the loaction of Charts and Chart related products."@en ;
    skos:inScheme cs: ;
    skos:prefLabel "Hydrographic Soundings - Indexes and Catalogues of Charts in the Australian Region"@en ;
    skos:topConceptOf cs: .

<http://pid.geoscience.gov.au/def/Data_Types/HYDROLADS_C> a skos:Concept ;
    skos:altLabel "HYDROLADS_C"@en ;
    skos:definition "Laser Airborne Depth Sounder (LADS) data is collected by directing a laser light source into the ocean which can be used to determine water depth in shallow water (less than 35m)  LADS data is high pr"@en ;
    skos:inScheme cs: ;
    skos:prefLabel "Hydrographic Soundings - Laser Airborne Depth Sounder (Commercial)"@en ;
    skos:scopeNote "Laser Airborne Depth Sounder (LADS) data is collected by directing a laser light source into the ocean which can be used to determine water depth in shallow water (less than 35m)  LADS data is high precision and high confidence.  This data has been collected by commercial organisations"@en ;
    skos:topConceptOf cs: .

<http://pid.geoscience.gov.au/def/Data_Types/HYDROLADS_RAN> a skos:Concept ;
    skos:altLabel "HYDROLADS_RAN"@en ;
    skos:definition "Laser Airborne Depth Sounder (LADS) data is collected by directing a laser light source into the ocean which can be used to determine water depth in shallow water (less than 35m)  LADS data is high pr"@en ;
    skos:inScheme cs: ;
    skos:prefLabel "Hydrographic Soundings - Laser Airborne Depth Sounder (RAN)"@en ;
    skos:scopeNote "Laser Airborne Depth Sounder (LADS) data is collected by directing a laser light source into the ocean which can be used to determine water depth in shallow water (less than 35m)  LADS data is high precision and high confidence.  This data has been collected for the Royal Australian Navy."@en ;
    skos:topConceptOf cs: .

<http://pid.geoscience.gov.au/def/Data_Types/HYDROMISCCH> a skos:Concept ;
    skos:altLabel "HYDROMISCCH"@en ;
    skos:definition "Charts are nautical maps used for navigating vessels in safe waters."@en ;
    skos:inScheme cs: ;
    skos:prefLabel "Hydrographic Soundings - Charts"@en ;
    skos:topConceptOf cs: .

<http://pid.geoscience.gov.au/def/Data_Types/HYDRONATMAP> a skos:Concept ;
    skos:altLabel "HYDRONATMAP"@en ;
    skos:definition "NATMAP, a Commonwealth Agency undertook bathymetric surveys of Australias continental shelf over a period of several years in the early 1970s.  Generally the spacing of the sounding tracks is 3 nautic"@en ;
    skos:inScheme cs: ;
    skos:prefLabel "Hydrographic Soundings - NATMAP Bathymetry bathymetric surveys"@en ;
    skos:scopeNote "NATMAP, a Commonwealth Agency undertook bathymetric surveys of Australias continental shelf over a period of several years in the early 1970s.  Generally the spacing of the sounding tracks is 3 nautical miles (1852 metres) with soundings taken more frequently.  Two sets of maps exist in this series, 1:150,000 working charts and 1:250,000 production charts.  The 1:150,000 charts contain more soundings and are to be used in preference to the 1:250,000 charts where available."@en ;
    skos:topConceptOf cs: .

<http://pid.geoscience.gov.au/def/Data_Types/HYDRORANAFI> a skos:Concept ;
    skos:altLabel "HYDRORANAFI"@en ;
    skos:definition "Superceded sheets showing the index of file locations for the fairsheet holdings of the Royal Australian Navy"@en ;
    skos:inScheme cs: ;
    skos:prefLabel "Hydrographic Soundings - RAN Area File Index"@en ;
    skos:topConceptOf cs: .

<http://pid.geoscience.gov.au/def/Data_Types/MAG> a skos:Concept ;
    skos:altLabel "MAG"@en ;
    skos:definition "MANDATORY FIELD"@en ;
    skos:inScheme cs: ;
    skos:prefLabel "Magnetic data"@en ;
    skos:topConceptOf cs: .

<http://pid.geoscience.gov.au/def/Data_Types/RAD> a skos:Concept ;
    skos:altLabel "RAD"@en ;
    skos:definition "MANDATORY FIELD"@en ;
    skos:inScheme cs: ;
    skos:prefLabel "Radiometric data, 4-channel"@en ;
    skos:topConceptOf cs: .

<http://pid.geoscience.gov.au/def/Data_Types/RAL> a skos:Concept ;
    skos:altLabel "RAL"@en ;
    skos:definition "MANDATORY FIELD"@en ;
    skos:inScheme cs: ;
    skos:prefLabel "Radiometric data, 256-channel"@en ;
    skos:topConceptOf cs: .

<http://pid.geoscience.gov.au/def/Data_Types/SEIS> a skos:Concept ;
    skos:altLabel "SEIS"@en ;
    skos:definition "MANDATORY FIELD"@en ;
    skos:inScheme cs: ;
    skos:prefLabel "Seismic data"@en ;
    skos:topConceptOf cs: .

<http://pid.geoscience.gov.au/def/Data_Types/SEISF> a skos:Concept ;
    skos:altLabel "SEISF"@en ;
    skos:definition "MANDATORY FIELD"@en ;
    skos:inScheme cs: ;
    skos:prefLabel "Seismic data, Refraction"@en ;
    skos:topConceptOf cs: .

<http://pid.geoscience.gov.au/def/Data_Types/SEISR> a skos:Concept ;
    skos:altLabel "SEISR"@en ;
    skos:definition "MANDATORY FIELD"@en ;
    skos:inScheme cs: ;
    skos:prefLabel "Seismic data, Reflection"@en ;
    skos:topConceptOf cs: .

<http://pid.geoscience.gov.au/def/Data_Types/SWATH> a skos:Concept ;
    skos:altLabel "SWATH"@en ;
    skos:definition "MANDATORY FIELD"@en ;
    skos:inScheme cs: ;
    skos:prefLabel "Swath data"@en ;
    skos:topConceptOf cs: .

<http://pid.geoscience.gov.au/def/Data_Types/TDE> a skos:Concept ;
    skos:altLabel "TDE"@en ;
    skos:definition "MANDATORY FIELD"@en ;
    skos:inScheme cs: ;
    skos:prefLabel "Electromagnetic data, Time-domain"@en ;
    skos:topConceptOf cs: .

<http://pid.geoscience.gov.au/def/Data_Types/WATER> a skos:Concept ;
    skos:altLabel "WATER"@en ;
    skos:definition "MANDATORY FIELD"@en ;
    skos:inScheme cs: ;
    skos:prefLabel "Water Samples or Water Chemistry data"@en ;
    skos:topConceptOf cs: .

<https://linked.data.gov.au/org/ga/voc-wg> a sdo:Organization ;
    sdo:affiliation <https://linked.data.gov.au/org/ga> ;
    sdo:name "Geoscience Australia Vocabulary Working Group" ;
    sdo:url <https://www.ga.gov.au/data-pubs/datastandards> .

<https://linked.data.gov.au/org/ga> a sdo:Organization ;
    sdo:name "Geoscience Australia" ;
    sdo:url <https://www.ga.gov.au> .

cs: a skos:ConceptScheme ;
    dcterms:created "2019-03-12T11:48:09"^^xsd:dateTime ;
    dcterms:creator <https://linked.data.gov.au/org/ga/voc-wg> ;
    dcterms:issued "2019-03-12T11:48:09"^^xsd:dateTime ;
    dcterms:publisher <https://linked.data.gov.au/org/ga> ;
    skos:changeNote "This vocabulary created directly from the database"@en ;
    skos:editorialNote "This file contains the Geoscience Australia 12-Mar-2019 version of the Data Types vocabulary"@en ;
    skos:hasTopConcept <http://pid.geoscience.gov.au/def/Data_Types/BATH>,
        <http://pid.geoscience.gov.au/def/Data_Types/ECO>,
        <http://pid.geoscience.gov.au/def/Data_Types/ELE>,
        <http://pid.geoscience.gov.au/def/Data_Types/FDE>,
        <http://pid.geoscience.gov.au/def/Data_Types/GEOL>,
        <http://pid.geoscience.gov.au/def/Data_Types/GRAV>,
        <http://pid.geoscience.gov.au/def/Data_Types/HYDROBAOFS>,
        <http://pid.geoscience.gov.au/def/Data_Types/HYDROBASC>,
        <http://pid.geoscience.gov.au/def/Data_Types/HYDROFS_NOTRAN>,
        <http://pid.geoscience.gov.au/def/Data_Types/HYDROFS_RANCG>,
        <http://pid.geoscience.gov.au/def/Data_Types/HYDROFS_RANHD>,
        <http://pid.geoscience.gov.au/def/Data_Types/HYDROGEBCOSS>,
        <http://pid.geoscience.gov.au/def/Data_Types/HYDROGEBCOTPS>,
        <http://pid.geoscience.gov.au/def/Data_Types/HYDROICCAUST>,
        <http://pid.geoscience.gov.au/def/Data_Types/HYDROLADS_C>,
        <http://pid.geoscience.gov.au/def/Data_Types/HYDROLADS_RAN>,
        <http://pid.geoscience.gov.au/def/Data_Types/HYDROMISCCH>,
        <http://pid.geoscience.gov.au/def/Data_Types/HYDRONATMAP>,
        <http://pid.geoscience.gov.au/def/Data_Types/HYDRORANAFI>,
        <http://pid.geoscience.gov.au/def/Data_Types/MAG>,
        <http://pid.geoscience.gov.au/def/Data_Types/RAD>,
        <http://pid.geoscience.gov.au/def/Data_Types/RAL>,
        <http://pid.geoscience.gov.au/def/Data_Types/SEIS>,
        <http://pid.geoscience.gov.au/def/Data_Types/SEISF>,
        <http://pid.geoscience.gov.au/def/Data_Types/SEISR>,
        <http://pid.geoscience.gov.au/def/Data_Types/SWATH>,
        <http://pid.geoscience.gov.au/def/Data_Types/TDE>,
        <http://pid.geoscience.gov.au/def/Data_Types/WATER> ;
    skos:prefLabel "Geoscience Australia Vocabulary - Data Types"@en .

