@prefix cs: <http://pid.geoscience.gov.au/def/Distributed_Computing_Platform> .
@prefix dcterms: <http://purl.org/dc/terms/> .
@prefix rdfs: <http://www.w3.org/2000/01/rdf-schema#> .
@prefix sdo: <https://schema.org/> .
@prefix skos: <http://www.w3.org/2004/02/skos/core#> .
@prefix xsd: <http://www.w3.org/2001/XMLSchema#> .

<http://pid.geoscience.gov.au/def/Distributed_Computing_Platform/COM> a skos:Concept ;
    rdfs:isDefinedBy cs: ;
    skos:altLabel "COM"@en ;
    skos:definition "COM - Component Object Model (COM) is a binary-interface standard for software components introduced by Microsoft in 1993."@en ;
    skos:inScheme cs: ;
    skos:prefLabel "Component Object Model"@en ;
    skos:scopeNote "Component Object Model (COM) is a binary-interface standard for software components introduced by Microsoft in 1993. It is used to enable inter-process communication and dynamic object creation in a large range of programming languages. COM is the basis for several other Microsoft technologies and frameworks, including OLE, OLE Automation, ActiveX, COM+, DCOM, the Windows shell, DirectX, UMDF and Windows Runtime."@en ;
    skos:topConceptOf cs: .

<http://pid.geoscience.gov.au/def/Distributed_Computing_Platform/CORBA> a skos:Concept ;
    rdfs:isDefinedBy cs: ;
    skos:altLabel "CORBA"@en ;
    skos:definition "Corba is a general-purpose, object-oriented programming language."@en ;
    skos:inScheme cs: ;
    skos:prefLabel "Corba"@en ;
    skos:scopeNote "Corba is a general-purpose, object-oriented programming language. Corba is designed by Charles Esterbrook, and runs on the Microsoft .NET and Mono platforms. It is strongly influenced by Python, C#, Eiffel, Objective-C, and other programming languages. It supports both static and dynamic typing. It has support for unit tests and contracts. It has lambda expressions, closures, list comprehensions, and generators.  Corba is an open-source project; it was released under the MIT License on February 29, 2008."@en ;
    skos:topConceptOf cs: .

<http://pid.geoscience.gov.au/def/Distributed_Computing_Platform/JAVA> a skos:Concept ;
    rdfs:isDefinedBy cs: ;
    skos:altLabel "JAVA"@en ;
    skos:definition "Java is an object-oriented language"@en ;
    skos:inScheme cs: ;
    skos:prefLabel "Java"@en ;
    skos:scopeNote "Java is an object-oriented language similar to C++, but simplified to eliminate language features that cause common programming errors. Java source code files (files with a .java extension) are compiled into a format called bytecode (files with a .class extension), which can then be executed by a Java interpreter."@en ;
    skos:topConceptOf cs: .

<http://pid.geoscience.gov.au/def/Distributed_Computing_Platform/SQL> a skos:Concept ;
    rdfs:isDefinedBy cs: ;
    skos:altLabel "SQL"@en ;
    skos:definition "SQL (Structured Query Language) is a standard interactive and programming language for getting information from and updating a database."@en ;
    skos:inScheme cs: ;
    skos:prefLabel "Structured Query Language"@en ;
    skos:scopeNote "Structured Query Language (SQL) is special-purpose programming language designed for managing data held in a relational database management system (RDBMS), or for stream processing in a relational data stream management system (RDSMS). According to ANSI (American National Standards Institute), it is the standard language for relational database management systems."@en ;
    skos:topConceptOf cs: .

<http://pid.geoscience.gov.au/def/Distributed_Computing_Platform/WebServices> a skos:Concept ;
    rdfs:isDefinedBy cs: ;
    skos:altLabel "WebServices"@en ;
    skos:definition "A Web service is a method of communication between two electronic devices over a network."@en ;
    skos:inScheme cs: ;
    skos:prefLabel "Web Services"@en ;
    skos:scopeNote "A Web service is a method of communication between two electronic devices over a network. It is a software function provided at a network address over the Web with the service always on as in the concept of utility computing."@en ;
    skos:topConceptOf cs: .

<http://pid.geoscience.gov.au/def/Distributed_Computing_Platform/XML> a skos:Concept ;
    rdfs:isDefinedBy cs: ;
    skos:altLabel "XML"@en ;
    skos:definition "Extensible Markup Language (XML) is a markup language that defines a set of rules for encoding documents in a format which is both human-readable and machine-readable."@en ;
    skos:inScheme cs: ;
    skos:prefLabel "Extensible Markup Language"@en ;
    skos:scopeNote "Extensible Markup Language (XML) is a markup language that defines a set of rules for encoding documents in a format which is both human-readable and machine-readable. It is defined by the W3C's XML 1.0 Specification and by several other related specifications, all of which are free open standards."@en ;
    skos:topConceptOf cs: .

<https://linked.data.gov.au/org/ga/voc-wg> a sdo:Organization ;
    sdo:affiliation <https://linked.data.gov.au/org/ga> ;
    sdo:name "Geoscience Australia Vocabulary Working Group" ;
    sdo:url <https://www.ga.gov.au/data-pubs/datastandards> .

<https://linked.data.gov.au/org/ga> a sdo:Organization ;
    sdo:name "Geoscience Australia" ;
    sdo:url <https://www.ga.gov.au> .

cs: a skos:ConceptScheme ;
    dcterms:created "2019-03-12T11:48:09"^^xsd:dateTime ;
    dcterms:creator <https://linked.data.gov.au/org/ga/voc-wg> ;
    dcterms:modified "2019-03-12T11:48:09"^^xsd:dateTime ;
    dcterms:provenance "GA's ORAPROD database tables"@en ;
    dcterms:publisher <https://linked.data.gov.au/org/ga> ;
    skos:changeNote "This vocabulary created directly from the database"@en ;
    skos:definition "Geoscience Australia's 12-Mar-2019 version of the Distributed Computing Platform vocabulary"@en ;
    skos:hasTopConcept <http://pid.geoscience.gov.au/def/Distributed_Computing_Platform/COM>,
        <http://pid.geoscience.gov.au/def/Distributed_Computing_Platform/CORBA>,
        <http://pid.geoscience.gov.au/def/Distributed_Computing_Platform/JAVA>,
        <http://pid.geoscience.gov.au/def/Distributed_Computing_Platform/SQL>,
        <http://pid.geoscience.gov.au/def/Distributed_Computing_Platform/WebServices>,
        <http://pid.geoscience.gov.au/def/Distributed_Computing_Platform/XML> ;
    skos:prefLabel "Distributed Computing Platform"@en .

