@prefix cs: <http://pid.geoscience.gov.au/def/Gamma_Ray_Spectrometry> .
@prefix dcterms: <http://purl.org/dc/terms/> .
@prefix rdfs: <http://www.w3.org/2000/01/rdf-schema#> .
@prefix sdo: <https://schema.org/> .
@prefix skos: <http://www.w3.org/2004/02/skos/core#> .
@prefix xsd: <http://www.w3.org/2001/XMLSchema#> .

<http://pid.geoscience.gov.au/def/Gamma_Ray_Spectrometry/GR-DR> a skos:Concept ;
    rdfs:isDefinedBy cs: ;
    skos:altLabel "GR-DR"@en ;
    skos:definition "An estimate of the air-absorbed dose rate (in nG/h ie. Nanograys per hour) at ground level from natural sources of radiation can be made from the fully corrected airborne total count count rates (cps)"@en ;
    skos:inScheme cs: ;
    skos:prefLabel "gamma ray dose-rate"@en ;
    skos:scopeNote "An estimate of the air-absorbed dose rate (in nG/h ie. Nanograys per hour) at ground level from natural sources of radiation can be made from the fully corrected airborne total count count rates (cps).  The S.I. unit of absorbed dose is the gray (Gy).  One Gy = 1 Joule/Kg."@en ;
    skos:topConceptOf cs: .

<http://pid.geoscience.gov.au/def/Gamma_Ray_Spectrometry/GR-K> a skos:Concept ;
    rdfs:isDefinedBy cs: ;
    skos:altLabel "GR-K"@en ;
    skos:definition "Gamma-rays emitted from the natural decay of Potassium (K-40) and measured by gamma-ray spectrometers. This applies to airborne and ground surveys and to borehole logging.  The gamma-rays have energie"@en ;
    skos:inScheme cs: ;
    skos:prefLabel "gamma ray Potassium"@en ;
    skos:scopeNote "Gamma-rays emitted from the natural decay of Potassium (K-40) and measured by gamma-ray spectrometers. This applies to airborne and ground surveys and to borehole logging.  The gamma-rays have energies between 1.37 Mev and 1.57 Mev.  The main photo-peak is at 1.46 Mev. The fully corrected airborne count rates (cps) are converted to mean ground level abundances of Potassium in units of percent Potassium."@en ;
    skos:topConceptOf cs: .

<http://pid.geoscience.gov.au/def/Gamma_Ray_Spectrometry/GR-TC> a skos:Concept ;
    rdfs:isDefinedBy cs: ;
    skos:altLabel "GR-TC"@en ;
    skos:definition "An estimate of the air-absorbed dose rate (in nG/h ie. Nanograys per hour) at ground level from natural sources of radiation can be made from the fully corrected airborne total count count rates (cps)"@en ;
    skos:inScheme cs: ;
    skos:prefLabel "gamma ray Total Counts"@en ;
    skos:scopeNote "An estimate of the air-absorbed dose rate (in nG/h ie. Nanograys per hour) at ground level from natural sources of radiation can be made from the fully corrected airborne total count count rates (cps).  The S.I. unit of absorbed dose is the gray (Gy).  One Gy = 1 Joule/Kg."@en ;
    skos:topConceptOf cs: .

<http://pid.geoscience.gov.au/def/Gamma_Ray_Spectrometry/GR-TH> a skos:Concept ;
    rdfs:isDefinedBy cs: ;
    skos:altLabel "GR-TH"@en ;
    skos:definition "Gamma-rays emitted from the natural decay of Thorium and measured by gamma-ray spectrometers. This applies to airborne and ground surveys and to borehole logging. The gamma-ray emissions from one of t"@en ;
    skos:inScheme cs: ;
    skos:prefLabel "gamma ray Thorium"@en ;
    skos:scopeNote "Gamma-rays emitted from the natural decay of Thorium and measured by gamma-ray spectrometers. This applies to airborne and ground surveys and to borehole logging. The gamma-ray emissions from one of the Thorium decay series daughter products, Thallium (Tl-208), are measured to estimate Thorium concentrations. The gamma-rays have energies between 2.41 Mev and 2.81 Mev.  The main photo-peak is at 2.61 Mev. The fully corrected airborne count rates (cps) are converted to mean ground level abundances of Thorium in units of ppm Thorium."@en ;
    skos:topConceptOf cs: .

<http://pid.geoscience.gov.au/def/Gamma_Ray_Spectrometry/GR-U> a skos:Concept ;
    rdfs:isDefinedBy cs: ;
    skos:altLabel "GR-U"@en ;
    skos:definition "Gamma-rays emitted from the natural decay of Uranium and measured by gamma-ray spectrometers. This applies to airborne and ground surveys and to borehole logging.  The gamma-ray emissions from one of "@en ;
    skos:inScheme cs: ;
    skos:prefLabel "gamma ray Uranium"@en ;
    skos:scopeNote "Gamma-rays emitted from the natural decay of Uranium and measured by gamma-ray spectrometers. This applies to airborne and ground surveys and to borehole logging.  The gamma-ray emissions from one of the Uranium decay series daughter products, bismuth (Bi-214), are measured to estimate Uranium concentrations. The gamma-rays have energies between 1.66 Mev and 1.86 Mev.  The main photo-peak is at 1.76 Mev. The fully corrected airborne count rates (cps) are converted to mean ground level abundances of Uranium in units of ppm Uranium."@en ;
    skos:topConceptOf cs: .

<https://linked.data.gov.au/org/ga/voc-wg> a sdo:Organization ;
    sdo:affiliation <https://linked.data.gov.au/org/ga> ;
    sdo:name "Geoscience Australia Vocabulary Working Group" ;
    sdo:url <https://www.ga.gov.au/data-pubs/datastandards> .

<https://linked.data.gov.au/org/ga> a sdo:Organization ;
    sdo:name "Geoscience Australia" ;
    sdo:url <https://www.ga.gov.au> .

cs: a skos:ConceptScheme ;
    dcterms:created "2019-03-12T11:48:09"^^xsd:dateTime ;
    dcterms:creator <https://linked.data.gov.au/org/ga/voc-wg> ;
    dcterms:modified "2019-03-12T11:48:09"^^xsd:dateTime ;
    dcterms:provenance "GA's ORAPROD database tables"@en ;
    dcterms:publisher <https://linked.data.gov.au/org/ga> ;
    skos:changeNote "This vocabulary created directly from the database"@en ;
    skos:definition "Geoscience Australia's 12-Mar-2019 version of the Gamma Ray Spectrometry vocabulary"@en ;
    skos:hasTopConcept <http://pid.geoscience.gov.au/def/Gamma_Ray_Spectrometry/GR-DR>,
        <http://pid.geoscience.gov.au/def/Gamma_Ray_Spectrometry/GR-K>,
        <http://pid.geoscience.gov.au/def/Gamma_Ray_Spectrometry/GR-TC>,
        <http://pid.geoscience.gov.au/def/Gamma_Ray_Spectrometry/GR-TH>,
        <http://pid.geoscience.gov.au/def/Gamma_Ray_Spectrometry/GR-U> ;
    skos:prefLabel "Gamma Ray Spectrometry"@en .

