@prefix cs: <http://pid.geoscience.gov.au/def/Horizontal_Order> .
@prefix dcterms: <http://purl.org/dc/terms/> .
@prefix sdo: <https://schema.org/> .
@prefix skos: <http://www.w3.org/2004/02/skos/core#> .
@prefix xsd: <http://www.w3.org/2001/XMLSchema#> .

<http://pid.geoscience.gov.au/def/Horizontal_Order/0> a skos:Concept ;
    skos:definition "ORDERS assigned in a similar manner to CLASS where C value (for one sigma) = 3."@en ;
    skos:inScheme cs: ;
    skos:prefLabel "0"@en ;
    skos:topConceptOf cs: .

<http://pid.geoscience.gov.au/def/Horizontal_Order/00> a skos:Concept ;
    skos:definition "ORDERS assigned in a similar manner to CLASS where C value (for one sigma) = 1."@en ;
    skos:inScheme cs: ;
    skos:prefLabel "00"@en ;
    skos:topConceptOf cs: .

<http://pid.geoscience.gov.au/def/Horizontal_Order/1> a skos:Concept ;
    skos:definition "ORDERS assigned in a similar manner to CLASS where C value (for one sigma) = 7.5."@en ;
    skos:inScheme cs: ;
    skos:prefLabel "1"@en ;
    skos:topConceptOf cs: .

<http://pid.geoscience.gov.au/def/Horizontal_Order/2> a skos:Concept ;
    skos:definition "ORDERS assigned in a similar manner to CLASS where C value (for one sigma) = 15."@en ;
    skos:inScheme cs: ;
    skos:prefLabel "2"@en ;
    skos:topConceptOf cs: .

<http://pid.geoscience.gov.au/def/Horizontal_Order/3> a skos:Concept ;
    skos:definition "ORDERS assigned in a similar manner to CLASS where C value (for one sigma) = 30."@en ;
    skos:inScheme cs: ;
    skos:prefLabel "3"@en ;
    skos:topConceptOf cs: .

<http://pid.geoscience.gov.au/def/Horizontal_Order/4> a skos:Concept ;
    skos:definition "ORDERS assigned in a similar manner to CLASS where C value (for one sigma) = 50."@en ;
    skos:inScheme cs: ;
    skos:prefLabel "4"@en ;
    skos:topConceptOf cs: .

<http://pid.geoscience.gov.au/def/Horizontal_Order/5> a skos:Concept ;
    skos:definition "ORDERS assigned in a similar manner to CLASS where C value (for one sigma) = 100."@en ;
    skos:inScheme cs: ;
    skos:prefLabel "5"@en ;
    skos:topConceptOf cs: .

<http://pid.geoscience.gov.au/def/Horizontal_Order/PROV> a skos:Concept ;
    skos:definition "MANDATORY FIELD"@en ;
    skos:inScheme cs: ;
    skos:prefLabel "PROV"@en ;
    skos:topConceptOf cs: .

<https://linked.data.gov.au/org/ga/voc-wg> a sdo:Organization ;
    sdo:affiliation <https://linked.data.gov.au/org/ga> ;
    sdo:name "Geoscience Australia Vocabulary Working Group" ;
    sdo:url <https://www.ga.gov.au/data-pubs/datastandards> .

<https://linked.data.gov.au/org/ga> a sdo:Organization ;
    sdo:name "Geoscience Australia" ;
    sdo:url <https://www.ga.gov.au> .

cs: a skos:ConceptScheme ;
    dcterms:created "2019-03-12T11:48:09"^^xsd:dateTime ;
    dcterms:creator <https://linked.data.gov.au/org/ga/voc-wg> ;
    dcterms:issued "2019-03-12T11:48:09"^^xsd:dateTime ;
    dcterms:publisher <https://linked.data.gov.au/org/ga> ;
    skos:changeNote "This vocabulary created directly from the database"@en ;
    skos:editorialNote "This file contains the Geoscience Australia 12-Mar-2019 version of the Horizontal Order vocabulary"@en ;
    skos:hasTopConcept <http://pid.geoscience.gov.au/def/Horizontal_Order/0>,
        <http://pid.geoscience.gov.au/def/Horizontal_Order/00>,
        <http://pid.geoscience.gov.au/def/Horizontal_Order/1>,
        <http://pid.geoscience.gov.au/def/Horizontal_Order/2>,
        <http://pid.geoscience.gov.au/def/Horizontal_Order/3>,
        <http://pid.geoscience.gov.au/def/Horizontal_Order/4>,
        <http://pid.geoscience.gov.au/def/Horizontal_Order/5>,
        <http://pid.geoscience.gov.au/def/Horizontal_Order/PROV> ;
    skos:prefLabel "Geoscience Australia Vocabulary - Horizontal Order"@en .

