@prefix cs: <http://pid.geoscience.gov.au/def/Hydrocarbon_Show_Interpretation> .
@prefix dcterms: <http://purl.org/dc/terms/> .
@prefix sdo: <https://schema.org/> .
@prefix skos: <http://www.w3.org/2004/02/skos/core#> .
@prefix xsd: <http://www.w3.org/2001/XMLSchema#> .

<http://pid.geoscience.gov.au/def/Hydrocarbon_Show_Interpretation/G2> a skos:Concept ;
    skos:altLabel "G2"@en ;
    skos:definition "Gas zone with water saturation less than approximately 80% with poor results from well testing"@en ;
    skos:inScheme cs: ;
    skos:prefLabel "Unproven gas zone"@en ;
    skos:topConceptOf cs: .

<http://pid.geoscience.gov.au/def/Hydrocarbon_Show_Interpretation/G4> a skos:Concept ;
    skos:altLabel "G4"@en ;
    skos:definition "Gas zone with water saturation less than approximately 80% with supporting results from well testing"@en ;
    skos:inScheme cs: ;
    skos:prefLabel "Proven gas zone"@en ;
    skos:topConceptOf cs: .

<http://pid.geoscience.gov.au/def/Hydrocarbon_Show_Interpretation/L2> a skos:Concept ;
    skos:altLabel "L2"@en ;
    skos:definition "Oil zone with water saturation less than approximately 80% with poor results from well testing"@en ;
    skos:inScheme cs: ;
    skos:prefLabel "Unproven oil zone"@en ;
    skos:topConceptOf cs: .

<http://pid.geoscience.gov.au/def/Hydrocarbon_Show_Interpretation/L4> a skos:Concept ;
    skos:altLabel "L4"@en ;
    skos:definition "Oil zone with water saturation less than approximately 80% with supporting results from well testing"@en ;
    skos:inScheme cs: ;
    skos:prefLabel "Proven oil zone"@en ;
    skos:topConceptOf cs: .

<http://pid.geoscience.gov.au/def/Hydrocarbon_Show_Interpretation/NS> a skos:Concept ;
    skos:altLabel "NS"@en ;
    skos:definition "No shows for any category"@en,
        "No zones of significant saturation observed"@en ;
    skos:inScheme cs: ;
    skos:prefLabel "No indications"@en,
        "No pay"@en ;
    skos:topConceptOf cs: .

<https://linked.data.gov.au/org/ga/voc-wg> a sdo:Organization ;
    sdo:affiliation <https://linked.data.gov.au/org/ga> ;
    sdo:name "Geoscience Australia Vocabulary Working Group" ;
    sdo:url <https://www.ga.gov.au/data-pubs/datastandards> .

<https://linked.data.gov.au/org/ga> a sdo:Organization ;
    sdo:name "Geoscience Australia" ;
    sdo:url <https://www.ga.gov.au> .

cs: a skos:ConceptScheme ;
    dcterms:created "2019-03-12T11:48:09"^^xsd:dateTime ;
    dcterms:creator <https://linked.data.gov.au/org/ga/voc-wg> ;
    dcterms:issued "2019-03-12T11:48:09"^^xsd:dateTime ;
    dcterms:publisher <https://linked.data.gov.au/org/ga> ;
    skos:changeNote "This vocabulary created directly from the database"@en ;
    skos:editorialNote "This file contains the Geoscience Australia 12-Mar-2019 version of the Hydrocarbon Show Interpretation vocabulary"@en ;
    skos:hasTopConcept <http://pid.geoscience.gov.au/def/Hydrocarbon_Show_Interpretation/G2>,
        <http://pid.geoscience.gov.au/def/Hydrocarbon_Show_Interpretation/G4>,
        <http://pid.geoscience.gov.au/def/Hydrocarbon_Show_Interpretation/L2>,
        <http://pid.geoscience.gov.au/def/Hydrocarbon_Show_Interpretation/L4>,
        <http://pid.geoscience.gov.au/def/Hydrocarbon_Show_Interpretation/NS> ;
    skos:prefLabel "Geoscience Australia Vocabulary - Hydrocarbon Show Interpretation"@en .

