@prefix cs: <http://pid.geoscience.gov.au/def/Hydrocarbon_Show_Category> .
@prefix dcterms: <http://purl.org/dc/terms/> .
@prefix sdo: <https://schema.org/> .
@prefix skos: <http://www.w3.org/2004/02/skos/core#> .
@prefix xsd: <http://www.w3.org/2001/XMLSchema#> .

<http://pid.geoscience.gov.au/def/Hydrocarbon_Show_Category/CORE> a skos:Concept ;
    skos:altLabel "CORE"@en ;
    skos:definition "Hydrocarbon shows from cores. See HYDROCARBON SHOW CORE lookup type for valid values."@en ;
    skos:inScheme cs: ;
    skos:prefLabel "HYDROCARBON SHOW CORE"@en ;
    skos:topConceptOf cs: .

<http://pid.geoscience.gov.au/def/Hydrocarbon_Show_Category/CUTTINGS> a skos:Concept ;
    skos:altLabel "CUTTINGS"@en ;
    skos:definition "Hydrocarbon shows from cuttings. See HYDROCARBON SHOW CUTTINGS lookup type for valid values."@en ;
    skos:inScheme cs: ;
    skos:prefLabel "HYDROCARBON SHOW CUTTINGS"@en ;
    skos:topConceptOf cs: .

<http://pid.geoscience.gov.au/def/Hydrocarbon_Show_Category/FLOW> a skos:Concept ;
    skos:altLabel "FLOW"@en ;
    skos:definition "Hydrocarbon shows from well production tests. See HYDROCARBON SHOW FLOW lookup type for valid values."@en ;
    skos:inScheme cs: ;
    skos:prefLabel "HYDROCARBON SHOW FLOW"@en ;
    skos:topConceptOf cs: .

<http://pid.geoscience.gov.au/def/Hydrocarbon_Show_Category/INTERPRETATION> a skos:Concept ;
    skos:altLabel "INTERPRETATION"@en ;
    skos:definition "Hydrocarbon shows from interpretation of several categories or other sources. See HYDROCARBON SHOW INTERPRETATION lookup type for valid values."@en ;
    skos:inScheme cs: ;
    skos:prefLabel "HYDROCARBON SHOW INTERPRETATION"@en ;
    skos:topConceptOf cs: .

<http://pid.geoscience.gov.au/def/Hydrocarbon_Show_Category/LOG> a skos:Concept ;
    skos:altLabel "LOG"@en ;
    skos:definition "Hydrocarbon shows from logs. See HYDROCARBON SHOW LOG lookup type for valid values."@en ;
    skos:inScheme cs: ;
    skos:prefLabel "HYDROCARBON SHOW LOG"@en ;
    skos:topConceptOf cs: .

<http://pid.geoscience.gov.au/def/Hydrocarbon_Show_Category/MUD_LOGGING> a skos:Concept ;
    skos:altLabel "MUD LOGGING"@en ;
    skos:definition "Hydrocarbon shows from mud logging. See HYDROCARBON SHOW MUD LOGGING lookup type for valid values."@en ;
    skos:inScheme cs: ;
    skos:prefLabel "HYDROCARBON SHOW MUD LOGGING"@en ;
    skos:topConceptOf cs: .

<http://pid.geoscience.gov.au/def/Hydrocarbon_Show_Category/PRESSURE_SURVEY> a skos:Concept ;
    skos:altLabel "PRESSURE SURVEY"@en ;
    skos:definition "Hydrocarbon shows from pressure survey. See HYDROCARBON SHOW PRESSURE SURVEY lookup type for valid values."@en ;
    skos:inScheme cs: ;
    skos:prefLabel "HYDROCARBON SHOW PRESSURE SURVEY"@en ;
    skos:topConceptOf cs: .

<http://pid.geoscience.gov.au/def/Hydrocarbon_Show_Category/RECOVERY> a skos:Concept ;
    skos:altLabel "RECOVERY"@en ;
    skos:definition "Hydrocarbon shows from well testing. See HYDROCARBON SHOW CORE lookup type for valid values."@en ;
    skos:inScheme cs: ;
    skos:prefLabel "HYDROCARBON SHOW RECOVERY"@en ;
    skos:topConceptOf cs: .

<http://pid.geoscience.gov.au/def/Hydrocarbon_Show_Category/SHOW> a skos:Concept ;
    skos:altLabel "SHOW"@en ;
    skos:definition "Hydrocarbon shows values used prior to 26 Nov 2007. For legacy data only - DO NOT USE."@en ;
    skos:inScheme cs: ;
    skos:prefLabel "HYDROCARBON SHOW"@en ;
    skos:topConceptOf cs: .

<http://pid.geoscience.gov.au/def/Hydrocarbon_Show_Category/SWC> a skos:Concept ;
    skos:altLabel "SWC"@en ;
    skos:definition "Hydrocarbon shows from sidewall cores. See HYDROCARBON SHOW SWC lookup type for valid values."@en ;
    skos:inScheme cs: ;
    skos:prefLabel "HYDROCARBON SHOW SWC"@en ;
    skos:topConceptOf cs: .

<https://linked.data.gov.au/org/ga/voc-wg> a sdo:Organization ;
    sdo:affiliation <https://linked.data.gov.au/org/ga> ;
    sdo:name "Geoscience Australia Vocabulary Working Group" ;
    sdo:url <https://www.ga.gov.au/data-pubs/datastandards> .

<https://linked.data.gov.au/org/ga> a sdo:Organization ;
    sdo:name "Geoscience Australia" ;
    sdo:url <https://www.ga.gov.au> .

cs: a skos:ConceptScheme ;
    dcterms:created "2019-03-12T11:48:09"^^xsd:dateTime ;
    dcterms:creator <https://linked.data.gov.au/org/ga/voc-wg> ;
    dcterms:issued "2019-03-12T11:48:09"^^xsd:dateTime ;
    dcterms:publisher <https://linked.data.gov.au/org/ga> ;
    skos:changeNote "This vocabulary created directly from the database"@en ;
    skos:editorialNote "This file contains the Geoscience Australia 12-Mar-2019 version of the Hydrocarbon Show Category vocabulary"@en ;
    skos:hasTopConcept <http://pid.geoscience.gov.au/def/Hydrocarbon_Show_Category/CORE>,
        <http://pid.geoscience.gov.au/def/Hydrocarbon_Show_Category/CUTTINGS>,
        <http://pid.geoscience.gov.au/def/Hydrocarbon_Show_Category/FLOW>,
        <http://pid.geoscience.gov.au/def/Hydrocarbon_Show_Category/INTERPRETATION>,
        <http://pid.geoscience.gov.au/def/Hydrocarbon_Show_Category/LOG>,
        <http://pid.geoscience.gov.au/def/Hydrocarbon_Show_Category/MUD_LOGGING>,
        <http://pid.geoscience.gov.au/def/Hydrocarbon_Show_Category/PRESSURE_SURVEY>,
        <http://pid.geoscience.gov.au/def/Hydrocarbon_Show_Category/RECOVERY>,
        <http://pid.geoscience.gov.au/def/Hydrocarbon_Show_Category/SHOW>,
        <http://pid.geoscience.gov.au/def/Hydrocarbon_Show_Category/SWC> ;
    skos:prefLabel "Geoscience Australia Vocabulary - Hydrocarbon Show Category"@en .

