@prefix cs: <http://pid.geoscience.gov.au/def/Hydrocarbon_Show_Flow> .
@prefix dcterms: <http://purl.org/dc/terms/> .
@prefix rdfs: <http://www.w3.org/2000/01/rdf-schema#> .
@prefix sdo: <https://schema.org/> .
@prefix skos: <http://www.w3.org/2004/02/skos/core#> .
@prefix xsd: <http://www.w3.org/2001/XMLSchema#> .

<http://pid.geoscience.gov.au/def/Hydrocarbon_Show_Flow/C2> a skos:Concept ;
    rdfs:isDefinedBy cs: ;
    skos:altLabel "C2"@en ;
    skos:definition "Condensate scum, globules or emulsion or unmeasured volume of condensate recovered"@en ;
    skos:inScheme cs: ;
    skos:prefLabel "Trace condensate"@en ;
    skos:topConceptOf cs: .

<http://pid.geoscience.gov.au/def/Hydrocarbon_Show_Flow/C3> a skos:Concept ;
    rdfs:isDefinedBy cs: ;
    skos:altLabel "C3"@en ;
    skos:definition "Discrete recovery of clean condensate"@en ;
    skos:inScheme cs: ;
    skos:prefLabel "Condensate recovery"@en ;
    skos:topConceptOf cs: .

<http://pid.geoscience.gov.au/def/Hydrocarbon_Show_Flow/C5> a skos:Concept ;
    rdfs:isDefinedBy cs: ;
    skos:altLabel "C5"@en ;
    skos:definition "Measured flow rate of clean condensate"@en ;
    skos:inScheme cs: ;
    skos:prefLabel "Condensate flow"@en ;
    skos:topConceptOf cs: .

<http://pid.geoscience.gov.au/def/Hydrocarbon_Show_Flow/G1> a skos:Concept ;
    rdfs:isDefinedBy cs: ;
    skos:altLabel "G1"@en ;
    skos:definition "Solution gas recovered from water"@en ;
    skos:inScheme cs: ;
    skos:prefLabel "Solution gas from water"@en ;
    skos:topConceptOf cs: .

<http://pid.geoscience.gov.au/def/Hydrocarbon_Show_Flow/G2> a skos:Concept ;
    rdfs:isDefinedBy cs: ;
    skos:altLabel "G2"@en ;
    skos:definition "Unmeasured volume or flow of gas observed or solution gas recovered from water or water"@en ;
    skos:editorialNote "Two definitions from the DB combined into one" ;
    skos:inScheme cs: ;
    skos:prefLabel "Trace gas"@en,
        "Trace solution gas from oil"@en ;
    skos:topConceptOf cs: .

<http://pid.geoscience.gov.au/def/Hydrocarbon_Show_Flow/G3> a skos:Concept ;
    rdfs:isDefinedBy cs: ;
    skos:altLabel "G3"@en ;
    skos:definition "Discrete recovery of gas; Discrete recovery of solution gas from oil"@en ;
    skos:editorialNote "Two definitions from the DB combined into one" ;
    skos:inScheme cs: ;
    skos:prefLabel "Gas recovery"@en,
        "Solution gas from oil"@en ;
    skos:topConceptOf cs: .

<http://pid.geoscience.gov.au/def/Hydrocarbon_Show_Flow/G5> a skos:Concept ;
    rdfs:isDefinedBy cs: ;
    skos:altLabel "G5"@en ;
    skos:definition "Measured flow rate of gas; Measured flow rate of solution gas from oil"@en ;
    skos:editorialNote "Two definitions from the DB combined into one" ;
    skos:inScheme cs: ;
    skos:prefLabel "Gas flow"@en,
        "Solution gas flow from oil"@en ;
    skos:topConceptOf cs: .

<http://pid.geoscience.gov.au/def/Hydrocarbon_Show_Flow/L2> a skos:Concept ;
    rdfs:isDefinedBy cs: ;
    skos:altLabel "L2"@en ;
    skos:definition "Oil scum, globules or emulsion or unmeasured volume of oil recovered"@en ;
    skos:inScheme cs: ;
    skos:prefLabel "Trace oil"@en ;
    skos:topConceptOf cs: .

<http://pid.geoscience.gov.au/def/Hydrocarbon_Show_Flow/L3> a skos:Concept ;
    rdfs:isDefinedBy cs: ;
    skos:altLabel "L3"@en ;
    skos:definition "Discrete recovery of clean oil"@en ;
    skos:inScheme cs: ;
    skos:prefLabel "Oil recovery"@en ;
    skos:topConceptOf cs: .

<http://pid.geoscience.gov.au/def/Hydrocarbon_Show_Flow/L5> a skos:Concept ;
    rdfs:isDefinedBy cs: ;
    skos:altLabel "L5"@en ;
    skos:definition "Measured flow rate of clean oil"@en ;
    skos:inScheme cs: ;
    skos:prefLabel "Oil flow"@en ;
    skos:topConceptOf cs: .

<http://pid.geoscience.gov.au/def/Hydrocarbon_Show_Flow/NR> a skos:Concept ;
    rdfs:isDefinedBy cs: ;
    skos:altLabel "NR"@en ;
    skos:definition "Unable to test target zone"@en ;
    skos:inScheme cs: ;
    skos:prefLabel "Failed test"@en ;
    skos:topConceptOf cs: .

<http://pid.geoscience.gov.au/def/Hydrocarbon_Show_Flow/NS> a skos:Concept ;
    rdfs:isDefinedBy cs: ;
    skos:altLabel "NS"@en ;
    skos:definition "Testing attempted but no samples taken and/or no oil or gas rate observed"@en ;
    skos:inScheme cs: ;
    skos:prefLabel "No flow or recovery"@en ;
    skos:topConceptOf cs: .

<http://pid.geoscience.gov.au/def/Hydrocarbon_Show_Flow/NT> a skos:Concept ;
    rdfs:isDefinedBy cs: ;
    skos:altLabel "NT"@en ;
    skos:definition "No flow tests attempted (Drill stem tests, production tests)"@en ;
    skos:inScheme cs: ;
    skos:prefLabel "No tests"@en ;
    skos:topConceptOf cs: .

<https://linked.data.gov.au/org/ga/voc-wg> a sdo:Organization ;
    sdo:affiliation <https://linked.data.gov.au/org/ga> ;
    sdo:name "Geoscience Australia Vocabulary Working Group" ;
    sdo:url <https://www.ga.gov.au/data-pubs/datastandards> .

<https://linked.data.gov.au/org/ga> a sdo:Organization ;
    sdo:name "Geoscience Australia" ;
    sdo:url <https://www.ga.gov.au> .

cs: a skos:ConceptScheme ;
    dcterms:created "2019-03-12T11:48:09"^^xsd:dateTime ;
    dcterms:creator <https://linked.data.gov.au/org/ga/voc-wg> ;
    dcterms:modified "2019-03-12T11:48:09"^^xsd:dateTime ;
    dcterms:provenance "GA's ORAPROD database tables"@en ;
    dcterms:publisher <https://linked.data.gov.au/org/ga> ;
    skos:changeNote "This vocabulary created directly from the database"@en ;
    skos:definition "Geoscience Australia's 12-Mar-2019 version of the Hydrocarbon Show Flow vocabulary"@en ;
    skos:hasTopConcept <http://pid.geoscience.gov.au/def/Hydrocarbon_Show_Flow/C2>,
        <http://pid.geoscience.gov.au/def/Hydrocarbon_Show_Flow/C3>,
        <http://pid.geoscience.gov.au/def/Hydrocarbon_Show_Flow/C5>,
        <http://pid.geoscience.gov.au/def/Hydrocarbon_Show_Flow/G1>,
        <http://pid.geoscience.gov.au/def/Hydrocarbon_Show_Flow/G2>,
        <http://pid.geoscience.gov.au/def/Hydrocarbon_Show_Flow/G3>,
        <http://pid.geoscience.gov.au/def/Hydrocarbon_Show_Flow/G5>,
        <http://pid.geoscience.gov.au/def/Hydrocarbon_Show_Flow/L2>,
        <http://pid.geoscience.gov.au/def/Hydrocarbon_Show_Flow/L3>,
        <http://pid.geoscience.gov.au/def/Hydrocarbon_Show_Flow/L5>,
        <http://pid.geoscience.gov.au/def/Hydrocarbon_Show_Flow/NR>,
        <http://pid.geoscience.gov.au/def/Hydrocarbon_Show_Flow/NS>,
        <http://pid.geoscience.gov.au/def/Hydrocarbon_Show_Flow/NT> ;
    skos:prefLabel "Hydrocarbon Show Flow"@en .

