PREFIX : <https://pid.geoscience.gov.au/def/voc/ga/BoreholePurpose/>
PREFIX astatus: <https://linked.data.gov.au/def/reg-statuses/>
PREFIX cs: <https://pid.geoscience.gov.au/def/voc/ga/BoreholePurpose>
PREFIX dcat: <http://www.w3.org/ns/dcat#>
PREFIX dcterms: <http://purl.org/dc/terms/>
PREFIX owl: <http://www.w3.org/2002/07/owl#>
PREFIX rdfs: <http://www.w3.org/2000/01/rdf-schema#>
PREFIX schema: <https://schema.org/>
PREFIX skos: <http://www.w3.org/2004/02/skos/core#>
PREFIX xsd: <http://www.w3.org/2001/XMLSchema#>

:appraisal
    a skos:Concept ;
    dcterms:identifier "appraisal"^^xsd:token ;
    skos:definition "Borehole drilled into a formation shown to be potentially productive, and is used to obtain more information a resource."@en ;
    skos:inScheme cs: ;
    skos:prefLabel "appraisal"@en ;
    skos:topConceptOf cs: ;
.

:coalQuality
    a skos:Concept ;
    dcterms:identifier "coalQuality"^^xsd:token ;
    skos:definition "Borehole drilled to obtain samples for laboratory testing and coal analysis. "@en ;
    skos:inScheme cs: ;
    skos:prefLabel "coal quality"@en ;
    skos:topConceptOf cs: ;
.

:development
    a skos:Concept ;
    dcterms:identifier "development"^^xsd:token ;
    skos:definition "Borehole drilled into an area or zone already proven to be productive, in order to assist in the recovery of a resource (eg, oil, gas, water). Includes service wells for hydrocarbon recovery, and CSG methane release wells."@en ;
    skos:inScheme cs: ;
    skos:prefLabel "development"@en ;
    skos:topConceptOf cs: ;
.

:environmental
    a skos:Concept ;
    dcterms:identifier "environmental"^^xsd:token ;
    skos:definition "Borehole drilled to obtain samples of or from strata for laboratory analysis of parameters which may impact on the environment, including water quality."@en ;
    skos:inScheme cs: ;
    skos:prefLabel "environmental"@en ;
    skos:topConceptOf cs: ;
.

:exploration
    a skos:Concept ;
    dcterms:identifier "exploration"^^xsd:token ;
    skos:definition "A borehole drilled primarily for the purpose of exploration for natural resources. ie, into an unproven area to determine and evaluate the resource potential and production capabilities of a previously undeveloped area or zone."@en ;
    skos:inScheme cs: ;
    skos:prefLabel "exploration"@en ;
    skos:topConceptOf cs: ;
.

:gasAnalysis
    a skos:Concept ;
    dcterms:identifier "gasAnalysis"^^xsd:token ;
    skos:definition "Borehole drilled for gas analysis. Typical applications include exploration, compliance and greenhouse gas emissions. "@en ;
    skos:inScheme cs: ;
    skos:prefLabel "gas analysis"@en ;
    skos:topConceptOf cs: ;
.

:geochemistry
    a skos:Concept ;
    dcterms:identifier "geochemistry"^^xsd:token ;
    skos:definition "A borehole drilled primarily for the purpose of collecting samples for geochemical analysis."@en ;
    skos:inScheme cs: ;
    skos:prefLabel "geochemistry"@en ;
    skos:topConceptOf cs: ;
.

:geothermal
    a skos:Concept ;
    dcterms:identifier "geothermal"^^xsd:token ;
    skos:definition "Borehole drilled to investigate the geotechnical properties of the strata and provide samples for mechanical testing. "@en ;
    skos:inScheme cs: ;
    skos:prefLabel "geotechnical"@en ;
    skos:topConceptOf cs: ;
.

:hydrological
    a skos:Concept ;
    dcterms:identifier "hydrological"^^xsd:token ;
    skos:definition "Borehole drilled to investigate water level, or piezometer installation. "@en ;
    skos:inScheme cs: ;
    skos:prefLabel "hydrological"@en ;
    skos:topConceptOf cs: ;
.

:lox
    a skos:Concept ;
    dcterms:identifier "lox"^^xsd:token ;
    skos:definition "Borehole drilled to obtain samples to determine the amount of oxidation of any coal seam by either visual and tactile or coal analysis methods. "@en ;
    skos:inScheme cs: ;
    skos:prefLabel "lox"@en ;
    skos:topConceptOf cs: ;
.

:monitoring
    a skos:Concept ;
    dcterms:identifier "monitoring"^^xsd:token ;
    skos:definition "A groundwater borehole used for the purpose of monitoring. (eg, groundwater levels)"@en ;
    skos:inScheme cs: ;
    skos:prefLabel "monitoring"@en ;
    skos:topConceptOf cs: ;
.

:research
    a skos:Concept ;
    dcterms:identifier "research"^^xsd:token ;
    skos:definition "A generic term to cover boreholes drilled primarily for the purpose of scientific research."@en ;
    skos:inScheme cs: ;
    skos:prefLabel "research"@en ;
    skos:topConceptOf cs: ;
.

:scientificInvestigationConstents
    a skos:Concept ;
    dcterms:identifier "scientificInvestigationConstents"^^xsd:token ;
    skos:definition "Borehole drilled under a scientific investigation consent granted under the OPGGS Act 2006 (amended 2012) or of the repealed Petroleum (Submerged Lands) Act 1967."@en ;
    skos:inScheme cs: ;
    skos:prefLabel "Scientific Investigation Consents"@en ;
    skos:topConceptOf cs: ;
.

:sequestration
    a skos:Concept ;
    dcterms:identifier "sequestration"^^xsd:token ;
    skos:definition "A borehole drilled for the purpose of underground storage of a commodity (eg, CO2 sequestration, aquifer storage and recovery)"@en ;
    skos:inScheme cs: ;
    skos:prefLabel "sequestration"@en ;
    skos:topConceptOf cs: ;
.

:service
    a skos:Concept ;
    dcterms:identifier "service"^^xsd:token ;
    skos:definition "Borehole drilled to provide a conduit or access to and from mine workings for equipment or materials. "@en ;
    skos:inScheme cs: ;
    skos:prefLabel "service"@en ;
    skos:topConceptOf cs: ;
.

:stratigraphicInvestigation
    a skos:Concept ;
    dcterms:identifier "stratigraphicInvestigation"^^xsd:token ;
    skos:definition "A borehole drilled primarily for the purpose of stratigraphic investigation."@en ;
    skos:inScheme cs: ;
    skos:prefLabel "stratigraphic investigation"@en ;
    skos:topConceptOf cs: ;
.

:structure
    a skos:Concept ;
    dcterms:identifier "structure"^^xsd:token ;
    skos:definition "Borehole drilled to investigate the attitude of strata and the impact of any tectonic features. "@en ;
    skos:inScheme cs: ;
    skos:prefLabel "structure"@en ;
    skos:topConceptOf cs: ;
.

:unknown
    a skos:Concept ;
    dcterms:identifier "unknown"^^xsd:token ;
    skos:definition "The purpose for drilling the borehole is not known."@en ;
    skos:inScheme cs: ;
    skos:prefLabel "unknown"@en ;
    skos:topConceptOf cs: ;
.

:watersupply
    a skos:Concept ;
    dcterms:identifier "watersupply"^^xsd:token ;
    skos:definition "A groundwater borehole drilled for the primary purpose of water supply. The bores may supply water for irrigation, stock, domestic use, or industrial use."@en ;
    skos:inScheme cs: ;
    skos:prefLabel "water supply"@en ;
    skos:topConceptOf cs: ;
.

cs:
    a skos:ConceptScheme ;
    dcterms:created "2022-08-09"^^xsd:date ;
    dcterms:creator <https://linked.data.gov.au/org/ga> ;
    dcterms:identifier "BoreholePurpose"^^xsd:token ;
    dcterms:modified "2022-08-09"^^xsd:date ;
    dcterms:provenance "Geoscience Australia Borehole Purpose (BOREHOLE.LU_BOREHOLE_PURPOSES)"@en ;
    dcterms:publisher <https://linked.data.gov.au/org/ga> ;
    rdfs:seeAlso <https://pid.geoscience.gov.au/dataset/ga/148553> ;
    owl:versionInfo "1" ;
    skos:definition "Purpose or intention for which the borehole was drilled. eg, exploration, development or production, geotechnical. Equivalent to PPDM Business Intention."@en ;
    skos:hasTopConcept
        :appraisal ,
        :coalQuality ,
        :development ,
        :environmental ,
        :exploration ,
        :gasAnalysis ,
        :geochemistry ,
        :geothermal ,
        :hydrological ,
        :lox ,
        :monitoring ,
        :research ,
        :scientificInvestigationConstents ,
        :sequestration ,
        :service ,
        :stratigraphicInvestigation ,
        :structure ,
        :unknown ,
        :watersupply ;
    skos:prefLabel "Borehole Geology - Purpose"@en ;
    dcat:contactPoint "Team Lead - Information Services; Energy, Minerals and Groundwater Division" ;
    schema:status astatus:experimental ;
.
