PREFIX : <https://pid.geoscience.gov.au/def/voc/ga/ContactCharacter/>
PREFIX astatus: <https://linked.data.gov.au/def/reg-statuses/>
PREFIX cs: <https://pid.geoscience.gov.au/def/voc/ga/ContactCharacter>
PREFIX dcat: <http://www.w3.org/ns/dcat#>
PREFIX dcterms: <http://purl.org/dc/terms/>
PREFIX owl: <http://www.w3.org/2002/07/owl#>
PREFIX schema: <https://schema.org/>
PREFIX skos: <http://www.w3.org/2004/02/skos/core#>
PREFIX xsd: <http://www.w3.org/2001/XMLSchema#>

:gradational
    a skos:Concept ;
    skos:broader :diffuse ;
    skos:definition "The contact from one geological unit to another is diffuse, by a gradual and consistent change generally in one direction of grainsize or composition, such that a sharp boundary cannot be defined."@en ;
    skos:inScheme cs: ;
    skos:prefLabel "gradational"@en ;
.

:interfingering
    a skos:Concept ;
    skos:definition "A geological unit contact that is formed over some distance by interfingering of parts of one unit with the adjacent unit."@en ;
    skos:inScheme cs: ;
    skos:prefLabel "interfingering"@en ;
    skos:topConceptOf cs: ;
.

:sharp
    a skos:Concept ;
    skos:definition "The contact between geological units is sharp or easily defined at a single interface."@en ;
    skos:inScheme cs: ;
    skos:prefLabel "sharp"@en ;
    skos:topConceptOf cs: ;
.

:diffuse
    a skos:Concept ;
    skos:definition "The contact between two geological units cannot be defined at a sharp interface.  The transition from one unit to another may be gradational (ie, exhibiting a consistent change in grainsize or composition), may involve irregular mixing of units, or may be obscured by alteration."@en ;
    skos:inScheme cs: ;
    skos:narrower :gradational ;
    skos:prefLabel "diffuse"@en ;
    skos:topConceptOf cs: ;
.

cs:
    a skos:ConceptScheme ;
    dcterms:created "2022-08-11"^^xsd:date ;
    dcterms:creator <https://linked.data.gov.au/org/ga> ;
    dcterms:modified "2022-08-11"^^xsd:date ;
    dcterms:publisher <https://linked.data.gov.au/org/ga> ;
    owl:versionInfo "1" ;
    skos:definition "Terms to describe the character of a contact between two geological units."@en ;
    skos:hasTopConcept
        :diffuse ,
        :interfingering ,
        :sharp ;
    skos:historyNote "Geoscience Australia Contact Character (FGDM.LU_contact-character)"@en ;
    skos:prefLabel "Field Geology - Contact Character"@en ;
    dcat:contactPoint "Team Lead - Information Services; Energy, Minerals and Groundwater Division" ;
    schema:status astatus:experimental ;
.

