PREFIX : <https://pid.geoscience.gov.au/def/voc/ga/DateQualifier/>
PREFIX cs: <https://pid.geoscience.gov.au/def/voc/ga/DateQualifier>
PREFIX dcat: <http://www.w3.org/ns/dcat#>
PREFIX owl: <http://www.w3.org/2002/07/owl#>
PREFIX rdfs: <http://www.w3.org/2000/01/rdf-schema#>
PREFIX schema: <https://schema.org/>
PREFIX skos: <http://www.w3.org/2004/02/skos/core#>
PREFIX xsd: <http://www.w3.org/2001/XMLSchema#>

:dateUnknown
    a skos:Concept ;
    rdfs:isDefinedBy <http://www.opengis.net/def/nil/OGC/0/unknown> ;
    skos:definition "The recorded date is unknown"@en ;
    skos:inScheme cs: ;
    skos:prefLabel "date unknown"@en ;
    skos:topConceptOf cs: ;
.

:estimatedEarliest
    a skos:Concept ;
    skos:broader :estimated ;
    skos:definition "The recorded date is the earliest known date, but it is possible the true date is earlier than what is recorded."@en ;
    skos:inScheme cs: ;
    skos:prefLabel "estimated earliest"@en ;
.

:estimatedLatest
    a skos:Concept ;
    skos:broader :estimated ;
    skos:definition "The recorded date is the latest known date, but it is possible the true date is later than what is recorded."@en ;
    skos:inScheme cs: ;
    skos:prefLabel "estimated latest"@en ;
.

:known
    a skos:Concept ;
    skos:definition "The recorded date is known"@en ;
    skos:inScheme cs: ;
    skos:prefLabel "known"@en ;
    skos:topConceptOf cs: ;
.

:estimated
    a skos:Concept ;
    skos:definition "The recorded date is estimated"@en ;
    skos:inScheme cs: ;
    skos:narrower
        :estimatedEarliest ,
        :estimatedLatest ;
    skos:prefLabel "estimated"@en ;
    skos:topConceptOf cs: ;
.

cs:
    a skos:ConceptScheme ;
    rdfs:seeAlso "https://pid.geoscience.gov.au/dataset/ga/148553" ;
    owl:versionInfo "1" ;
    skos:changeNote "2024-10-16 NJC: update to be VocPub 4.10 valid"@en ;
    schema:citation "Geoscience Australia Date Qualifer Terms (BOREHOLE.LU_DATE_QUALIFIERS)" ;
    skos:definition "Terms to describe the confidence or quality in a recorded date "@en ;
    skos:hasTopConcept
        :dateUnknown ,
        :estimated ,
        :known ;
    skos:prefLabel "Borehole Geology - Date Qualifier"@en ;
    dcat:contactPoint "Team Lead - Information Services; Minerals, Energy and Groundwater Division" ;
    schema:creator <https://linked.data.gov.au/org/ga> ;
    schema:dateCreated "2022-08-04"^^xsd:date ;
    schema:dateModified "2024-10-16"^^xsd:date ;
    schema:publisher <https://linked.data.gov.au/org/ga> ;
.
