PREFIX : <https://pid.geoscience.gov.au/def/voc/ga/DirectionalSurveyClass/>
PREFIX cs: <https://pid.geoscience.gov.au/def/voc/ga/DirectionalSurveyClass>
PREFIX dcat: <http://www.w3.org/ns/dcat#>
PREFIX dcterms: <http://purl.org/dc/terms/>
PREFIX owl: <http://www.w3.org/2002/07/owl#>
PREFIX rdfs: <http://www.w3.org/2000/01/rdf-schema#>
PREFIX sdo: <https://schema.org/>
PREFIX skos: <http://www.w3.org/2004/02/skos/core#>
PREFIX xsd: <http://www.w3.org/2001/XMLSchema#>

:azimuthAndInclination
    a skos:Concept ;
    skos:definition "The directional survey is comprised of azimuth and inclination measurements."@en ;
    skos:inScheme cs: ;
    skos:prefLabel "azimuth and inclination"@en ;
    skos:topConceptOf cs: ;
.

:inclinationOnly
    a skos:Concept ;
    skos:definition "The directional survey is comprised of only inclination measurements."@en ;
    skos:inScheme cs: ;
    skos:prefLabel "inclination only"@en ;
    skos:topConceptOf cs: ;
.

cs:
    a skos:ConceptScheme ;
    dcterms:created "2022-08-04"^^xsd:date ;
    dcterms:creator <https://linked.data.gov.au/org/ga> ;
    dcterms:modified "2022-08-04"^^xsd:date ;
    dcterms:provenance "Geoscience Australia Directional Survey Class (BOREHOLE.LU_DIR_SRVY_CLASS)"@en ;
    dcterms:publisher <https://linked.data.gov.au/org/ga> ;
    rdfs:seeAlso <https://pid.geoscience.gov.au/dataset/ga/148553> ;
    owl:versionInfo "1" ;
    skos:definition "Terms to denote whether the directional survey is comprised of azimuth and inclination measurements, or only inclination measurements."@en ;
    skos:hasTopConcept
        :azimuthAndInclination ,
        :inclinationOnly ;
    skos:prefLabel "Borehole Geology - Directional Survey Class"@en ;
    dcat:contactPoint "Team Lead - Information Services; Minerals, Energy and Groundwater Division" ;
.
