PREFIX cs: <https://pid.geoscience.gov.au/def/voc/ga/DirectionalSurveyAzimuth>
PREFIX dcat: <http://www.w3.org/ns/dcat#>
PREFIX dcterms: <http://purl.org/dc/terms/>
PREFIX owl: <http://www.w3.org/2002/07/owl#>
PREFIX rdfs: <http://www.w3.org/2000/01/rdf-schema#>
PREFIX sdo: <https://schema.org/>
PREFIX skos: <http://www.w3.org/2004/02/skos/core#>
PREFIX xsd: <http://www.w3.org/2001/XMLSchema#>

<https://pid.geoscience.gov.au/def/voc/ga/DirectionalSurveyAzimuth/gridNorth>
    a skos:Concept ;
    dcterms:identifier "gridNorth"^^xsd:token ;
    dcterms:provenance "GA"@en ;
    skos:definition "Azimuth measurements in this directional survey are relative to a local grid north."@en ;
    skos:exactMatch <http://resource.geoscience.gov.au/classifier/ga/directional_survey_azimuth_north_type/grid_north> ;
    skos:inScheme cs: ;
    skos:prefLabel "grid north"@en ;
    skos:topConceptOf cs: ;
.

<https://pid.geoscience.gov.au/def/voc/ga/DirectionalSurveyAzimuth/magneticNorth>
    a skos:Concept ;
    dcterms:identifier "magneticNorth"^^xsd:token ;
    dcterms:provenance "GA"@en ;
    skos:definition "Azimuth measurements in this directional survey are relative to magnetic north."@en ;
    skos:exactMatch <http://resource.geoscience.gov.au/classifier/ga/directional_survey_azimuth_north_type/magnetic_north> ;
    skos:inScheme cs: ;
    skos:prefLabel "magnetic north"@en ;
    skos:topConceptOf cs: ;
.

<https://pid.geoscience.gov.au/def/voc/ga/DirectionalSurveyAzimuth/trueNorth>
    a skos:Concept ;
    dcterms:identifier "trueNorth"^^xsd:token ;
    dcterms:provenance "GA"@en ;
    skos:definition "Azimuth measurements in this directional survey are relative to true north."@en ;
    skos:exactMatch <http://resource.geoscience.gov.au/classifier/ga/directional_survey_azimuth_north_type/true_north> ;
    skos:inScheme cs: ;
    skos:prefLabel "true north"@en ;
    skos:topConceptOf cs: ;
.

<https://linked.data.gov.au/org/ga>
    a sdo:Organization ;
    sdo:description "Geoscience Australia is Australia's pre-eminent public sector geoscience organisation. It is the nation's trusted advisor on the geology and geography of Australia. It applies science and technology to describe and understand the Earth for the benefit of Australia."@en ;
    sdo:name "Geoscience Australia" ;
    sdo:url "https://www.ga.gov.au"^^xsd:anyURI ;
.

cs:
    a skos:ConceptScheme ;
    dcterms:created "2022-08-04"^^xsd:date ;
    dcterms:creator <https://linked.data.gov.au/org/ga> ;
    dcterms:identifier "DirectionalSurveyAzimuth"^^xsd:token ;
    dcterms:modified "2022-08-04"^^xsd:date ;
    dcterms:provenance "Geoscience Australia Directional Survey Azimuth Terms (BOREHOLE.LU_DIR_SRVY_AZ_TYPE)"@en ;
    dcterms:publisher <https://linked.data.gov.au/org/ga> ;
    rdfs:seeAlso <https://pid.geoscience.gov.au/dataset/ga/148553> ;
    owl:versionInfo "1" ;
    skos:definition "The type of North datum used for azimuth measurements (eg, true north, magnetic north, local grid north)."@en ;
    skos:hasTopConcept
        <https://pid.geoscience.gov.au/def/voc/ga/DirectionalSurveyAzimuth/gridNorth> ,
        <https://pid.geoscience.gov.au/def/voc/ga/DirectionalSurveyAzimuth/magneticNorth> ,
        <https://pid.geoscience.gov.au/def/voc/ga/DirectionalSurveyAzimuth/trueNorth> ;
    skos:prefLabel "Borehole Geology - Directional Survey Azimuth "@en ;
    dcat:contactPoint "Team Lead - Information Services; Minerals, Energy and Groundwater Division " ;
.
