PREFIX : <https://pid.geoscience.gov.au/def/voc/ga/EntityTypeOrFeature/>
PREFIX astatus: <https://linked.data.gov.au/def/reg-statuses/>
PREFIX cs: <https://pid.geoscience.gov.au/def/voc/ga/EntityTypeOrFeature>
PREFIX dcat: <http://www.w3.org/ns/dcat#>
PREFIX dcterms: <http://purl.org/dc/terms/>
PREFIX owl: <http://www.w3.org/2002/07/owl#>
PREFIX rdfs: <http://www.w3.org/2000/01/rdf-schema#>
PREFIX schema: <https://schema.org/>
PREFIX skos: <http://www.w3.org/2004/02/skos/core#>
PREFIX xsd: <http://www.w3.org/2001/XMLSchema#>

:acreageRelease
    a skos:Concept ;
    skos:definition "Offshore acreage released by the various Australian Government-State/NT Joint Authorities."@en ;
    skos:inScheme cs: ;
    skos:prefLabel "acreage release"@en ;
    skos:topConceptOf cs: ;
.

:borehole
    a skos:Concept ;
    skos:definition "A generic term for any hole or shaft drilled into the Earth. A borehole may have many purposes (eg, petroleum, mineral, or groundwater exploration or production; stratigraphic or engineering investigation)."@en ;
    skos:inScheme cs: ;
    skos:prefLabel "borehole"@en ;
    skos:topConceptOf cs: ;
.

:country
    a skos:Concept ;
    dcterms:provenance "See GA Country Codes vocab"@en ;
    skos:definition "Country name (ISO 3166-1998 Code for the representation of names of countries)"@en ;
    skos:inScheme cs: ;
    skos:prefLabel "country"@en ;
    skos:topConceptOf cs: ;
.

:emitter
    a skos:Concept ;
    skos:definition "This entity contains data about CO2 Emission sources - including power stations, petroleum fields, gas processing plants, oil refineries, coke production plants"@en ;
    skos:inScheme cs: ;
    skos:prefLabel "emitter"@en ;
    skos:topConceptOf cs: ;
.

:essci
    a skos:Concept ;
    skos:definition "This entity contains data about ESSCIs - environmentally sustainable sites for CO2 injection"@en ;
    skos:inScheme cs: ;
    skos:prefLabel "ESSCI"@en ;
    skos:topConceptOf cs: ;
.

:estuary
    a skos:Concept ;
    skos:definition "This entity contains data about Australian estuaries"@en ;
    skos:inScheme cs: ;
    skos:prefLabel "estuary"@en ;
    skos:topConceptOf cs: ;
.

:explorationPermit
    a skos:Concept ;
    skos:definition "Permit to provide exclusive rights to undertake seismic surveys and drilling in a defined area."@en ;
    skos:inScheme cs: ;
    skos:prefLabel "exploration permit"@en ;
    skos:topConceptOf cs: ;
.

:facies
    a skos:Concept ;
    skos:definition "This entity contains information about facies - derived from within Australian estuaries"@en ;
    skos:inScheme cs: ;
    skos:prefLabel "facies"@en ;
    skos:topConceptOf cs: ;
.

:fieldSite
    a skos:Concept ;
    skos:definition "Place (site) where an observation and/or measurement was made and/or sampling took place. For example observations/measurements/samples of rocks, soil, stream sediments, water, regolith, landform, vegetation, or rock properties."@en ;
    skos:inScheme cs: ;
    skos:prefLabel "field site"@en ;
    skos:topConceptOf cs: ;
.

:laboratory
    a skos:Concept ;
    skos:definition "A facility that provides controlled conditions in which scientific or technological research, experiments, and measurement may be performed."@en ;
    skos:inScheme cs: ;
    skos:prefLabel "laboratory"@en ;
    skos:topConceptOf cs: ;
.

:mapsheet
    a skos:Concept ;
    skos:definition "A MAPSHEET is the bounding polygon of the map as in, for example, the National Mapping 1:250 000 map sheet index. Mapsheets can be any scale, and include standard mapsheet boundaries and non-standard mapsheet boundaries."@en ;
    skos:inScheme cs: ;
    skos:prefLabel "mapsheet"@en ;
    skos:topConceptOf cs: ;
.

:marsegment
    a skos:Concept ;
    skos:definition "This table contains information on data subsets of a survey, referred to as segments. Operations segments are defined by a substantial change in the recording parameters of a survey, loop segments are defined where the survey loops on itself, and sampling segments identify where the ship may have stopped or slowed for sampling."@en ;
    skos:inScheme cs: ;
    skos:prefLabel "MARSEGMENT"@en ;
    skos:topConceptOf cs: ;
.

:mineWaste
    a skos:Concept ;
    skos:definition "Locality of mining or processing plant waste, such as tailings dam, slag heap, or dumps"@en ;
    skos:inScheme cs: ;
    skos:prefLabel "mine waste"@en ;
    skos:topConceptOf cs: ;
.

:mineralDeposit
    a skos:Concept ;
    skos:definition "An aggregation of mineralisation that may or may not have resources defined"@en ;
    skos:inScheme cs: ;
    skos:prefLabel "mineral deposit"@en ;
    skos:topConceptOf cs: ;
.

:mineralOccurrence
    a skos:Concept ;
    skos:definition "A mineral accumulation in the lithosphere."@en ;
    skos:inScheme cs: ;
    skos:prefLabel "mineral occurrence"@en ;
    skos:topConceptOf cs: ;
.

:mineralProject
    a skos:Concept ;
    skos:definition "A mining operation or mineral exploration project that includes multiple mineral deposits"@en ;
    skos:inScheme cs: ;
    skos:prefLabel "mineral project"@en ;
    skos:topConceptOf cs: ;
.

:mineralisedZone
    a skos:Concept ;
    skos:definition "A mineralised zone may describe a zone of uneconomic mineralisation or an economic orebody. There may be one or more mineralised zone within a specific Mineral Deposit entity."@en ;
    skos:inScheme cs: ;
    skos:prefLabel "mineralised zone"@en ;
    skos:topConceptOf cs: ;
.

:museumCollection
    a skos:Concept ;
    skos:definition "a generic term for any CPC/PALEO and mineral specimen museum collection."@en ;
    skos:inScheme cs: ;
    skos:prefLabel "museum collection"@en ;
    skos:topConceptOf cs: ;
.

:observatory
    a skos:Concept ;
    skos:definition "This entity contains data about observatories - buildings or places set apart for, and furnished with instruments for making, observations of natural phenomena; esp., for magnetic observations, ,astronomical, meteorological"@en ;
    skos:inScheme cs: ;
    skos:prefLabel "observatory"@en ;
    skos:topConceptOf cs: ;
.

:opggsaReprocessing
    a skos:Concept ;
    skos:definition "This entity contains data for reprocessing activities carried out under the Offshore Petroleum and Greenhouse Gas Storage Act."@en ;
    skos:inScheme cs: ;
    skos:prefLabel "OPGGSA reprocessing"@en ;
    skos:topConceptOf cs: ;
.

:pipeline
    a skos:Concept ;
    skos:definition "This entity contains data about pipelines - containers joining two connection points for the transportation of oil, gas, water or other materials"@en ;
    skos:inScheme cs: ;
    skos:prefLabel "pipeline"@en ;
    skos:topConceptOf cs: ;
.

:placeName
    a skos:Concept ;
    skos:definition "This entity contains data about Gazetteer place names"@en ;
    skos:inScheme cs: ;
    skos:prefLabel "place name"@en ;
    skos:topConceptOf cs: ;
.

:politicalRegion
    a skos:Concept ;
    skos:definition "This entity contains data about political regions and boundaries."@en ;
    skos:inScheme cs: ;
    skos:prefLabel "political region"@en ;
    skos:topConceptOf cs: ;
.

:port
    a skos:Concept ;
    skos:definition "Harbour - a place by the sea, or by a river or other waterway,where ships and boats can dock, load, and unload."@en ;
    skos:inScheme cs: ;
    skos:prefLabel "port"@en ;
    skos:topConceptOf cs: ;
.

:powerStation
    a skos:Concept ;
    skos:definition "Site where fossil fuel, nuclear, hydro, solar, wind, biological or other resources are converted into electrical power."@en ;
    skos:inScheme cs: ;
    skos:prefLabel "power station"@en ;
    skos:topConceptOf cs: ;
.

:productionLicence
    a skos:Concept ;
    skos:definition "Licence granted to holder of exploration permit or retention lease, for the recovery of petroleum following a commercial discovery."@en ;
    skos:inScheme cs: ;
    skos:prefLabel "production licence"@en ;
    skos:topConceptOf cs: ;
.

:project
    a skos:Concept ;
    skos:definition "This entity contains data about projects"@en ;
    skos:inScheme cs: ;
    skos:prefLabel "project"@en ;
    skos:topConceptOf cs: ;
.

:province
    a skos:Concept ;
    skos:definition "This entity contains data about provinces"@en ;
    skos:inScheme cs: ;
    skos:prefLabel "province"@en ;
    skos:topConceptOf cs: ;
.

:resourceProcessingPlant
    a skos:Concept ;
    skos:definition "Locality for adding value to raw materials, particularly minerals."@en ;
    skos:inScheme cs: ;
    skos:prefLabel "resource processing plant"@en ;
    skos:topConceptOf cs: ;
.

:resourceProject
    a skos:Concept ;
    skos:definition "Proposed, planned or developing scheme, including infrastructure, for extracting resources that requires a large amount of time, effort, capital, or planning. Once developed, the type of entity could change to MINE, WELL, RESOURCE PROCESSING PLANT, or something similar."@en ;
    skos:inScheme cs: ;
    skos:prefLabel "resource project"@en ;
    skos:topConceptOf cs: ;
.

:retentionLease
    a skos:Concept ;
    skos:definition "Lease granted to holder of exploration permit, where a discovery is not currently commercial but is expected to become so."@en ;
    skos:inScheme cs: ;
    skos:prefLabel "retention lease"@en ;
    skos:topConceptOf cs: ;
.

:section
    a skos:Concept ;
    skos:definition "A set of observations and/or measurements and/or samples taken at points or intervals along a line, section or traverse, in any direction at or beneath the earth's surface (measured section). For example, observations of a group of stratigraphic units or regolith zones."@en ;
    skos:inScheme cs: ;
    skos:prefLabel "section"@en ;
    skos:topConceptOf cs: ;
.

:seismicline
    a skos:Concept ;
    skos:definition "Information about seismic lines for a given survey.  Each seismic line has a different name, but the parameters of seismic lines in any given segment should be similar.  A segment may consist of many lines, and a line may fall within more than 1 segment if the operating parameters change."@en ;
    skos:inScheme cs: ;
    skos:prefLabel "seismic line"@en ;
    skos:topConceptOf cs: ;
.

:state
    a skos:Concept ;
    skos:definition "All States and Territories (currently only Australian implemented)"@en ;
    skos:inScheme cs: ;
    skos:prefLabel "state"@en ;
    skos:topConceptOf cs: ;
.

:stratUnitDefinitionLocation
    a skos:Concept ;
    skos:definition "The physical points that outline a section or a point that indicates an area that displays the defining characteristics of a stratigraphic unit"@en ;
    skos:inScheme cs: ;
    skos:prefLabel "stratigraphic unit definition location"@en ;
    skos:topConceptOf cs: ;
.

:survey
    a skos:Concept ;
    skos:definition "This entity contains data for marine, gravity, seismic and airborne surveys."@en ;
    skos:inScheme cs: ;
    skos:prefLabel "survey"@en ;
    skos:topConceptOf cs: ;
.

:well
    a skos:Concept ;
    skos:definition "This entity contains general and header information about wells.  A well is an actual or proposed hole in the ground, designed to exchange fluids between a subsurface reservoir and the surface (or another reservoir) or to retrieve rock core or samples or to enable the detection and measurement of rock properties.  A well (eg sidetrack or horizontal well) may originate from another well defined by PARENT."@en ;
    skos:inScheme cs: ;
    skos:prefLabel "well"@en ;
    skos:topConceptOf cs: ;
.

:wildcatLocation
    a skos:Concept ;
    skos:definition "Permit to conduct further exploration and/or appraisal activities within the location blocks to determine more accurately the nature of the discovery."@en ;
    skos:inScheme cs: ;
    skos:prefLabel "wildcat location"@en ;
    skos:topConceptOf cs: ;
.

cs:
    a skos:ConceptScheme ;
    dcterms:created "2022-08-04"^^xsd:date ;
    dcterms:creator <https://linked.data.gov.au/org/ga> ;
    dcterms:modified "2022-08-04"^^xsd:date ;
    dcterms:provenance "Geoscience Australia Entity Type or Feature (A.ENTITY_TYPES)"@en ;
    dcterms:publisher <https://linked.data.gov.au/org/ga> ;
    rdfs:seeAlso <https://pid.geoscience.gov.au/dataset/ga/148553> ;
    owl:versionInfo "1" ;
    skos:definition "Type of entity or feature. (eg, measured section, borehole, field site)."@en ;
    skos:hasTopConcept
        :acreageRelease ,
        :borehole ,
        :country ,
        :emitter ,
        :essci ,
        :estuary ,
        :explorationPermit ,
        :facies ,
        :fieldSite ,
        :laboratory ,
        :mapsheet ,
        :marsegment ,
        :mineWaste ,
        :mineralDeposit ,
        :mineralOccurrence ,
        :mineralProject ,
        :mineralisedZone ,
        :museumCollection ,
        :observatory ,
        :opggsaReprocessing ,
        :pipeline ,
        :placeName ,
        :politicalRegion ,
        :port ,
        :powerStation ,
        :productionLicence ,
        :project ,
        :province ,
        :resourceProcessingPlant ,
        :resourceProject ,
        :retentionLease ,
        :section ,
        :seismicline ,
        :state ,
        :stratUnitDefinitionLocation ,
        :survey ,
        :well ,
        :wildcatLocation ;
    skos:prefLabel "General Geology - Entity or Feature Type"@en ;
    dcat:contactPoint "Team Lead - Information Services; Minerals, Energy and Groundwater Division " ;
    schema:status astatus:experimental ;
.
