PREFIX cs: <https://pid.geoscience.gov.au/def/voc/ga/field_site_purpose>
PREFIX dcat: <http://www.w3.org/ns/dcat#>
PREFIX dcterms: <http://purl.org/dc/terms/>
PREFIX owl: <http://www.w3.org/2002/07/owl#>
PREFIX rdfs: <http://www.w3.org/2000/01/rdf-schema#>
PREFIX sdo: <https://schema.org/>
PREFIX skos: <http://www.w3.org/2004/02/skos/core#>
PREFIX xsd: <http://www.w3.org/2001/XMLSchema#>

<https://pid.geoscience.gov.au/def/voc/ga/field_site_purpose/environmental_study>
    a skos:Concept ;
    dcterms:identifier "environmental_study"^^xsd:token ;
    skos:definition "A field site to make observations or collect samples for environmental purposes."@en ;
    skos:inScheme cs: ;
    skos:prefLabel "environmental study"@en ;
    skos:topConceptOf cs: ;
.

<https://pid.geoscience.gov.au/def/voc/ga/field_site_purpose/geochemistry>
    a skos:Concept ;
    dcterms:identifier "geochemistry"^^xsd:token ;
    skos:definition "A field site used to make observations or collect rock or regolith samples for geochemical (including isotopic) analysis."@en ;
    skos:inScheme cs: ;
    skos:prefLabel "geochemistry"@en ;
    skos:topConceptOf cs: ;
.

<https://pid.geoscience.gov.au/def/voc/ga/field_site_purpose/geochronology>
    a skos:Concept ;
    dcterms:identifier "geochronology"^^xsd:token ;
    skos:definition "A field site used to determine the age of geological materials."@en ;
    skos:inScheme cs: ;
    skos:prefLabel "geochronology"@en ;
    skos:topConceptOf cs: ;
.

<https://pid.geoscience.gov.au/def/voc/ga/field_site_purpose/geological_study>
    a skos:Concept ;
    dcterms:identifier "geological_study"^^xsd:token ;
    skos:definition "A field site from a geological survey, including lithological, stratigraphic, structural, metamorphic, and other geological description."@en ;
    skos:inScheme cs: ;
    skos:prefLabel "geological study"@en ;
    skos:topConceptOf cs: ;
.

<https://pid.geoscience.gov.au/def/voc/ga/field_site_purpose/geophysics>
    a skos:Concept ;
    dcterms:identifier "geophysics"^^xsd:token ;
    skos:definition "A field site to make observations about the geophysical properties at that location."@en ;
    skos:inScheme cs: ;
    skos:prefLabel "geophysics"@en ;
    skos:topConceptOf cs: ;
.

<https://pid.geoscience.gov.au/def/voc/ga/field_site_purpose/hydrochemistry>
    a skos:Concept ;
    dcterms:identifier "hydrochemistry"^^xsd:token ;
    skos:definition "A field site to make observations or collect samples for hydrochemical analysis."@en ;
    skos:inScheme cs: ;
    skos:prefLabel "hydrochemistry"@en ;
    skos:topConceptOf cs: ;
.

<https://pid.geoscience.gov.au/def/voc/ga/field_site_purpose/mineral_resource_appraisal>
    a skos:Concept ;
    dcterms:identifier "mineral_resource_appraisal"^^xsd:token ;
    skos:definition "A field site to make observations or collect samples for determining the mineral resource character or potential of an area."@en ;
    skos:inScheme cs: ;
    skos:prefLabel "mineral resource appraisal"@en ;
    skos:topConceptOf cs: ;
.

<https://pid.geoscience.gov.au/def/voc/ga/field_site_purpose/multi-purpose_appraisal>
    a skos:Concept ;
    dcterms:identifier "multi-purpose_appraisal"^^xsd:token ;
    skos:definition "A field site to make observations or collect samples for multiple purposes. (eg, geological description, geochemical sampling, geochronological sampling, etc)"@en ;
    skos:inScheme cs: ;
    skos:prefLabel "multi-purpose appraisal"@en ;
    skos:topConceptOf cs: ;
.

<https://pid.geoscience.gov.au/def/voc/ga/field_site_purpose/natural_resource_management_study>
    a skos:Concept ;
    dcterms:identifier "natural_resource_management_study"^^xsd:token ;
    skos:definition "A field site used for the purpose of determining the natural resource management aspects of an area."@en ;
    skos:inScheme cs: ;
    skos:prefLabel "natural resource management study"@en ;
    skos:topConceptOf cs: ;
.

<https://pid.geoscience.gov.au/def/voc/ga/field_site_purpose/neotectonics>
    a skos:Concept ;
    dcterms:identifier "neotectonics"^^xsd:token ;
    skos:definition "A field site to make observations or collect samples for determining the deformation/earthquake history of an area under conditions imposed by the current crustal stress regime."@en ;
    skos:inScheme cs: ;
    skos:prefLabel "neotectonics"@en ;
    skos:topConceptOf cs: ;
.

<https://pid.geoscience.gov.au/def/voc/ga/field_site_purpose/petrophysics>
    a skos:Concept ;
    dcterms:identifier "petrophysics"^^xsd:token ;
    skos:definition "A field site to make observations or collect samples for rock properties. (eg porosity, permeability, magnetic susceptibility)"@en ;
    skos:inScheme cs: ;
    skos:prefLabel "petrophysics"@en ;
    skos:topConceptOf cs: ;
.

<https://pid.geoscience.gov.au/def/voc/ga/field_site_purpose/unknown>
    a skos:Concept ;
    dcterms:identifier "unknown"^^xsd:token ;
    skos:definition "The field site purpose is unknown"@en ;
    skos:inScheme cs: ;
    skos:prefLabel "unknown"@en ;
    skos:topConceptOf cs: ;
.

<https://linked.data.gov.au/org/ga>
    a sdo:Organization ;
    sdo:description "Geoscience Australia is Australia's pre-eminent public sector geoscience organisation. It is the nation's trusted advisor on the geology and geography of Australia. It applies science and technology to describe and understand the Earth for the benefit of Australia."@en ;
    sdo:name "Geoscience Australia" ;
    sdo:url "https://www.ga.gov.au"^^xsd:anyURI ;
.

cs:
    a skos:ConceptScheme ;
    dcterms:created "2022-08-04"^^xsd:date ;
    dcterms:creator <https://linked.data.gov.au/org/ga> ;
    dcterms:identifier "field_site_purpose"^^xsd:token ;
    dcterms:modified "2022-08-04"^^xsd:date ;
    dcterms:publisher <https://linked.data.gov.au/org/ga> ;
    rdfs:seeAlso <https://pid.geoscience.gov.au/dataset/ga/148553> ;
    owl:versionInfo "1" ;
    skos:definition "The purpose of the field site (eg, geological study, geochemistry, neotectonics)."@en ;
    skos:hasTopConcept
        <https://pid.geoscience.gov.au/def/voc/ga/field_site_purpose/environmental_study> ,
        <https://pid.geoscience.gov.au/def/voc/ga/field_site_purpose/geochemistry> ,
        <https://pid.geoscience.gov.au/def/voc/ga/field_site_purpose/geochronology> ,
        <https://pid.geoscience.gov.au/def/voc/ga/field_site_purpose/geological_study> ,
        <https://pid.geoscience.gov.au/def/voc/ga/field_site_purpose/geophysics> ,
        <https://pid.geoscience.gov.au/def/voc/ga/field_site_purpose/hydrochemistry> ,
        <https://pid.geoscience.gov.au/def/voc/ga/field_site_purpose/mineral_resource_appraisal> ,
        <https://pid.geoscience.gov.au/def/voc/ga/field_site_purpose/multi-purpose_appraisal> ,
        <https://pid.geoscience.gov.au/def/voc/ga/field_site_purpose/natural_resource_management_study> ,
        <https://pid.geoscience.gov.au/def/voc/ga/field_site_purpose/neotectonics> ,
        <https://pid.geoscience.gov.au/def/voc/ga/field_site_purpose/petrophysics> ,
        <https://pid.geoscience.gov.au/def/voc/ga/field_site_purpose/unknown> ;
    skos:historyNote "Geoscience Australia Field Site Purpose Terms (FGDM. LU_FIELDSITE_PURPOSE)"@en ;
    skos:prefLabel "Field Geology - Field Site Purpose "@en ;
    dcat:contactPoint "Team Lead - Information Services; Minerals, Energy and Groundwater Division" ;
.
