PREFIX : <https://pid.geoscience.gov.au/def/voc/ga/ModesOfOccurence/>
PREFIX cs: <https://pid.geoscience.gov.au/def/voc/ga/ModesOfOccurence>
PREFIX dcat: <http://www.w3.org/ns/dcat#>
PREFIX owl: <http://www.w3.org/2002/07/owl#>
PREFIX rdfs: <http://www.w3.org/2000/01/rdf-schema#>
PREFIX schema: <https://schema.org/>
PREFIX skos: <http://www.w3.org/2004/02/skos/core#>
PREFIX xsd: <http://www.w3.org/2001/XMLSchema#>

:akmolith
    a skos:Concept ;
    skos:broader :intrusion ;
    skos:definition "an intrusion along a decollement zone, with or without tonguelike extensions into the surrounding rock"@en ;
    skos:inScheme cs: ;
    skos:prefLabel "akmolith"@en ;
.

:amygdale
    a skos:Concept ;
    skos:broader :volcanic-feature ;
    skos:definition "a gas cavity or vesicle in an igneous rock which is filled with secondary minerals"@en ;
    skos:inScheme cs: ;
    skos:prefLabel "amygdale"@en ;
.

:apophysis
    a skos:Concept ;
    skos:broader :intrusion ;
    skos:definition "an offshoot from a larger intrusive body"@en ;
    skos:inScheme cs: ;
    skos:prefLabel "apophysis"@en ;
.

:batholith
    a skos:Concept ;
    skos:definition "a discordant magma body with exposed surface area of more than 100 square kilometres; typically consists of multiple intrusions."@en ;
    skos:inScheme cs: ;
    skos:prefLabel "batholith"@en ;
    skos:topConceptOf cs: ;
.

:bioclast
    a skos:Concept ;
    skos:broader :clast ;
    skos:definition "a fragment or clast in a rock composed of the remains of organisms"@en ;
    skos:inScheme cs: ;
    skos:prefLabel "bioclast"@en ;
.

:block
    a skos:Concept ;
    skos:broader :pyroclast ;
    skos:definition "an angular pyroclast > 64 mm"@en ;
    skos:inScheme cs: ;
    skos:prefLabel "block"@en ;
.

:bomb
    a skos:Concept ;
    skos:broader :pyroclast ;
    skos:definition "a clot of lava, usually mafic-ultramafic, ejected from a volcanic vent while viscous, and which assumes a rounded shape as it solidifies in flight"@en ;
    skos:inScheme cs: ;
    skos:prefLabel "bomb"@en ;
.

:cactolith
    a skos:Concept ;
    skos:broader :intrusion ;
    skos:definition "an obscurely cactus-shaped intrusion."@en ;
    skos:inScheme cs: ;
    skos:prefLabel "cactolith"@en ;
.

:chonolith
    a skos:Concept ;
    skos:broader :intrusion ;
    skos:definition "an intrusion so irregular as to defy description"@en ;
    skos:inScheme cs: ;
    skos:prefLabel "chonolith"@en ;
.

:concretion
    a skos:Concept ;
    skos:definition "a hard, compact mass or aggregate of mineral matter, normally subsperical but commonly oblate, disc-shaped or irregular.  Formed from precipitation from solution about a nucleus or centre"@en ;
    skos:inScheme cs: ;
    skos:prefLabel "concretion"@en ;
    skos:topConceptOf cs: ;
.

:cone-sheet
    a skos:Concept ;
    skos:broader :ring-complex ;
    skos:definition "an arcuate dyke that dips 30-45 degrees towards the centre of the arc; occur in concentric sets, presumably converging at a magmatic centre"@en ;
    skos:inScheme cs: ;
    skos:prefLabel "cone sheet"@en ;
.

:cooling-column
    a skos:Concept ;
    skos:broader :volcanic-feature ;
    skos:definition "a cooling unit in a volcanic rock defined by polygonal jointing perpendicular to the flow surface"@en ;
    skos:inScheme cs: ;
    skos:prefLabel "cooling column"@en ;
.

:cryptoexplosive
    a skos:Concept ;
    skos:broader :volcanic-feature ;
    skos:definition "a volcanic body of rock formed by subsurface explosive activity"@en ;
    skos:inScheme cs: ;
    skos:prefLabel "cryptoexplosive"@en ;
.

:cumulate-mineral
    a skos:Concept ;
    skos:broader :crystal ;
    skos:definition "a crystal formed during accumulation of early-formed crystals from a magma"@en ;
    skos:inScheme cs: ;
    skos:prefLabel "cumulate mineral"@en ;
.

:cupola
    a skos:Concept ;
    skos:broader :intrusion ;
    skos:definition "a large upward projection of the roof of an igneous intrusion into the country rock above."@en ;
    skos:inScheme cs: ;
    skos:prefLabel "cupola"@en ;
.

:ductolith
    a skos:Concept ;
    skos:broader :intrusion ;
    skos:definition "a concordant intrusion, teardrop-shaped in cross section"@en ;
    skos:inScheme cs: ;
    skos:prefLabel "ductolith"@en ;
.

:dyke
    a skos:Concept ;
    skos:broader :intrusion ;
    skos:definition "a tabular igneous intrusion that cuts across the bedding or foliation of the country rock"@en ;
    skos:inScheme cs: ;
    skos:prefLabel "dyke"@en ;
.

:dyke-swarm
    a skos:Concept ;
    skos:broader :intrusion ;
    skos:definition "a set of dykes, generally subparallel, with a common origin"@en ;
    skos:inScheme cs: ;
    skos:prefLabel "dyke swarm"@en ;
.

:enclave
    a skos:Concept ;
    skos:broader :inclusion ;
    skos:definition "an inclusion within an igneous rock to which it may or may not be genetically related"@en ;
    skos:inScheme cs: ;
    skos:prefLabel "enclave"@en ;
.

:ethmolith
    a skos:Concept ;
    skos:broader :intrusion ;
    skos:definition "a discordant, funnel-shaped intrusion, tapers downward"@en ;
    skos:inScheme cs: ;
    skos:prefLabel "ethmolith"@en ;
.

:extrusive-dome
    a skos:Concept ;
    skos:broader :volcanic-feature ;
    skos:definition "an extrusion forming a bulbous dome above and around a volcanic vent"@en ;
    skos:inScheme cs: ;
    skos:prefLabel "extrusion dome"@en ;
.

:facies
    a skos:Concept ;
    skos:definition "a lateral variant of a lithostratigraphic or metamorphic unit"@en ;
    skos:inScheme cs: ;
    skos:prefLabel "facies"@en ;
    skos:topConceptOf cs: ;
.

:fissure
    a skos:Concept ;
    skos:broader :intrusion ;
    skos:definition "a volcanic conduit having the form of a crack or fissure."@en ;
    skos:inScheme cs: ;
    skos:prefLabel "fissure"@en ;
.

:floor-ascendant
    a skos:Concept ;
    skos:definition "a upward projection of country rock into an igneous intrusion"@en ;
    skos:inScheme cs: ;
    skos:prefLabel "floor ascendant"@en ;
    skos:topConceptOf cs: ;
.

:glomerocryst
    a skos:Concept ;
    skos:broader :crystal ;
    skos:definition "an aggregate of crystals of the same mineral"@en ;
    skos:inScheme cs: ;
    skos:prefLabel "glomerocryst"@en ;
.

:gneissic-band
    a skos:Concept ;
    skos:broader :band-layer ;
    skos:definition "a compositional band or layer in a gneiss mineralogically distinct from the surrounding material"@en ;
    skos:inScheme cs: ;
    skos:prefLabel "gneissic band"@en ;
.

:graphic-intergrowth
    a skos:Concept ;
    skos:definition "a regular poikilitic intergrowth of triangular or linear-angular shaped grains of one mineral within a larger other mineral, typically quartz with alkali feldspar"@en ;
    skos:inScheme cs: ;
    skos:prefLabel "graphic intergrowth"@en ;
    skos:topConceptOf cs: ;
.

:harpolith
    a skos:Concept ;
    skos:broader :phacolith ;
    skos:definition "a phacolith with a vertical axis; indicates multiple deformations"@en ;
    skos:inScheme cs: ;
    skos:prefLabel "harpolith"@en ;
.

:high-level-pluton
    a skos:Concept ;
    skos:broader :intrusion ;
    skos:definition "a pluton emplaced at a high or subvolcanic level in the crust"@en ;
    skos:inScheme cs: ;
    skos:prefLabel "high-level pluton"@en ;
.

:holoblast
    a skos:Concept ;
    skos:broader :crystalloblast ;
    skos:definition "a crystalloblast that is newly and completely formed during metamorphism"@en ;
    skos:inScheme cs: ;
    skos:prefLabel "holoblast"@en ;
.

:hydrothermal-alteration
    a skos:Concept ;
    skos:definition "a rock or mineral derived from hydrothermal alteration of a rock"@en ;
    skos:inScheme cs: ;
    skos:prefLabel "hydrothermal alteration"@en ;
    skos:topConceptOf cs: ;
.

:hypidioblast
    a skos:Concept ;
    skos:broader :crystalloblast ;
    skos:definition "a crystalloblast that is formed during metamorphism and is bounded in part by its characteristic crystal faces"@en ;
    skos:inScheme cs: ;
    skos:prefLabel "hypidioblast"@en ;
.

:idioblast
    a skos:Concept ;
    skos:broader :crystalloblast ;
    skos:definition "a crystalloblast that is formed during metamorphism and is bounded by its characteristic crystal faces"@en ;
    skos:inScheme cs: ;
    skos:prefLabel "idioblast"@en ;
.

:igneous-band
    a skos:Concept ;
    skos:broader :band-layer ;
    skos:definition "a compositional band or layer in an igneous rock mineralogically distict from the surrounding material"@en ;
    skos:inScheme cs: ;
    skos:prefLabel "igneous band"@en ;
.

:intraclast
    a skos:Concept ;
    skos:broader :clast ;
    skos:definition "a clast or fragment in a sedimentary rock of another penecontemporaneous sedimentary rock that has been eroded within the basin of deposition"@en ;
    skos:inScheme cs: ;
    skos:prefLabel "intraclast"@en ;
.

:irregular-vein
    a skos:Concept ;
    skos:broader :vein ;
    skos:definition "a vein with no obvious form."@en ;
    skos:inScheme cs: ;
    skos:prefLabel "irregular vein"@en ;
.

:laccolith
    a skos:Concept ;
    skos:broader :intrusion ;
    skos:definition "a concordant, flat-based, convex-up intrusion"@en ;
    skos:inScheme cs: ;
    skos:prefLabel "laccolith"@en ;
.

:lens
    a skos:Concept ;
    skos:broader :band-layer ;
    skos:definition "a discontinuous layer or bed within a sedimentary rock"@en ;
    skos:inScheme cs: ;
    skos:prefLabel "lens"@en ;
.

:leucosome
    a skos:Concept ;
    skos:definition "the light coloured part of a migmatite or other rock with compositional segregations, usually rich in quartz and feldspar"@en ;
    skos:inScheme cs: ;
    skos:prefLabel "leucosome"@en ;
    skos:topConceptOf cs: ;
.

:lopolith
    a skos:Concept ;
    skos:broader :intrusion ;
    skos:definition "a large, concordant, typically layered igneous intrusion whose floor is convex-down and whose roof may be convex-down or flat."@en ;
    skos:inScheme cs: ;
    skos:prefLabel "lopolith"@en ;
.

:marker-bed
    a skos:Concept ;
    skos:broader :bed ;
    skos:definition "a laterally continuous stratigraphic marker within another unit."@en ;
    skos:inScheme cs: ;
    skos:prefLabel "marker bed"@en ;
.

:melanosome
    a skos:Concept ;
    skos:definition "the dark coloured part of a migmatite or other rock with compositional segregations, rich in mafic minerals"@en ;
    skos:inScheme cs: ;
    skos:prefLabel "melanosome"@en ;
    skos:topConceptOf cs: ;
.

:microlite
    a skos:Concept ;
    skos:broader :crystal ;
    skos:definition "a microscopic crystal that polarises light and has some determinable optical properties"@en ;
    skos:inScheme cs: ;
    skos:prefLabel "microlite"@en ;
.

:nodule
    a skos:Concept ;
    skos:definition "A small rounded mass of a mineral or mineral aggregate, usually with a contrasting composition from the enclosing sediment or rock matrix in which it is embedded. A fragment of a coarse grained igneous rock occurring within a finer grained rock."@en ;
    skos:inScheme cs: ;
    skos:prefLabel "nodule"@en ;
    skos:topConceptOf cs: ;
.

:oikocryst
    a skos:Concept ;
    skos:broader :crystalloblast ;
    skos:definition "the enclosing crystal in a poikolitic texture"@en ;
    skos:inScheme cs: ;
    skos:prefLabel "oikocryst"@en ;
.

:oncolite
    a skos:Concept ;
    skos:broader :grain ;
    skos:definition "a variously shaped, concentrically laminated, calcareous sedimentary structure, usually less than 10 cm in diameter, formed by the accretion of successive layered masses of blue-green algae"@en ;
    skos:inScheme cs: ;
    skos:prefLabel "oncolite"@en ;
.

:ooid
    a skos:Concept ;
    skos:broader :grain ;
    skos:definition "a small round or ovate accretionary particle in an oolitic rock, formed of concentric carbonate layers around a nucleus in shallow, wave-agitated water"@en ;
    skos:inScheme cs: ;
    skos:prefLabel "ooid"@en ;
.

:pellet
    a skos:Concept ;
    skos:broader :grain ;
    skos:definition "a small, usually rounded aggregate of clay-sized calcareous (micritic) material, devoid of internal structure, and contained within a well sorted carbonate rock"@en ;
    skos:inScheme cs: ;
    skos:prefLabel "pellet"@en ;
.

:phenocryst
    a skos:Concept ;
    skos:broader :crystal ;
    skos:definition "a relatively large, conspicuous crystal in a porphyrytic igneous rock"@en ;
    skos:inScheme cs: ;
    skos:prefLabel "phenocryst"@en ;
.

:pillow
    a skos:Concept ;
    skos:broader :lava-flow ;
    skos:definition "a pillow-like lava body extruded beneath water"@en ;
    skos:inScheme cs: ;
    skos:prefLabel "pillow"@en ;
.

:pipe
    a skos:Concept ;
    skos:broader :intrusion ;
    skos:definition "a vertical conduit through the Earth's crust below a volcano, through which magmatic materials have passed; usually filled with volcanic breccia and fragments of older rock."@en ;
    skos:inScheme cs: ;
    skos:prefLabel "pipe"@en ;
.

:pisolite
    a skos:Concept ;
    skos:broader :grain ;
    skos:definition "a small round or ovate accretionary particle, larger and less regular than an ooid, formed by concentric precipitation around a nucleus typically of carbonate (limestone) or iron oxides (laterite)"@en ;
    skos:inScheme cs: ;
    skos:prefLabel "pisolite"@en ;
.

:planar-vein
    a skos:Concept ;
    skos:broader :vein ;
    skos:definition "a vein with length and width significantly greater than its thickness, giving the vein a tabular form."@en ;
    skos:inScheme cs: ;
    skos:prefLabel "planar vein"@en ;
.

:plug
    a skos:Concept ;
    skos:broader :volcanic-feature ;
    skos:definition "a roughly cylindrical mass of congealed magma that fills the conduit of an inactive volcano"@en ;
    skos:inScheme cs: ;
    skos:prefLabel "plug"@en ;
.

:pluton
    a skos:Concept ;
    skos:broader :intrusion ;
    skos:definition "a deep-seated igneous intrusion"@en ;
    skos:inScheme cs: ;
    skos:prefLabel "pluton"@en ;
.

:pod
    a skos:Concept ;
    skos:broader :intrusion ;
    skos:definition "an intrusion of elongate or lenticular form"@en ;
    skos:inScheme cs: ;
    skos:prefLabel "pod"@en ;
.

:poikiloblast
    a skos:Concept ;
    skos:broader :crystalloblast ;
    skos:definition "a crystal formed by recrystallisation during metamorphism with numerous inclusions of smaller grains"@en ;
    skos:inScheme cs: ;
    skos:prefLabel "poikiloblast"@en ;
.

:porphyroblast
    a skos:Concept ;
    skos:broader :crystalloblast ;
    skos:definition "a pseudoporphyritic crystal in a rock produced by metamorphic recrystallisation"@en ;
    skos:inScheme cs: ;
    skos:prefLabel "porphyroblast"@en ;
.

:porphyroclast
    a skos:Concept ;
    skos:broader :crystal ;
    skos:definition "a paleoblast within a finer grained recrystalllised and/or pulverised matrix"@en ;
    skos:inScheme cs: ;
    skos:prefLabel "porphyroclast"@en ;
.

:pseudomorph
    a skos:Concept ;
    skos:definition "a secondary mineral whose outward crystal form has been inherited from the orignal mineral it has replaced"@en ;
    skos:inScheme cs: ;
    skos:prefLabel "pseudomorph"@en ;
    skos:topConceptOf cs: ;
.

:reaction-rim
    a skos:Concept ;
    skos:broader :corona ;
    skos:definition "a peripheral zone around a mineral composed of the products of the reaction of an early solidified mineral with a surrounding melt"@en ;
    skos:inScheme cs: ;
    skos:prefLabel "reaction rim"@en ;
.

:righ-dyke
    a skos:Concept ;
    skos:broader :ring-complex ;
    skos:definition "an arcuate or subcircular dyke, generally associated with a volcanic centre."@en ;
    skos:inScheme cs: ;
    skos:prefLabel "ring dyke"@en ;
.

:roof-pendant
    a skos:Concept ;
    skos:definition "a downward projection of country rock into an igneous intrusion"@en ;
    skos:inScheme cs: ;
    skos:prefLabel "roof pendant"@en ;
    skos:topConceptOf cs: ;
.

:sedimentry-dyke
    a skos:Concept ;
    skos:definition "a tabular sedimentary intrusion that cuts across the bedding or foliation of the host rock"@en ;
    skos:inScheme cs: ;
    skos:prefLabel "sedimentary dyke"@en ;
    skos:topConceptOf cs: ;
.

:sheet
    a skos:Concept ;
    skos:broader :intrusion ;
    skos:definition "a tabular intrusion, concordant or slightly discordant."@en ;
    skos:inScheme cs: ;
    skos:prefLabel "sheet"@en ;
.

:sigmoidal-vein
    a skos:Concept ;
    skos:broader :vein ;
    skos:definition "a vein is curved so as to resemble the letter S in section."@en ;
    skos:inScheme cs: ;
    skos:prefLabel "sigmoidal vein"@en ;
.

:sill
    a skos:Concept ;
    skos:broader :intrusion ;
    skos:definition "a tabular igneous intrusion that parallels the bedding or foliation of the country rock."@en ;
    skos:inScheme cs: ;
    skos:prefLabel "sill"@en ;
.

:sphenolith
    a skos:Concept ;
    skos:broader :intrusion ;
    skos:definition "a wedge-like intrusion, partly concordant, partly discordant."@en ;
    skos:inScheme cs: ;
    skos:prefLabel "sphenolith"@en ;
.

:spherulite
    a skos:Concept ;
    skos:broader :volcanic-feature ;
    skos:definition "a rounded or spherical mass of acicular crystals, commonly of feldspar radiating from a central point.  Commonly formed from devitrification of volcanic glass"@en ;
    skos:inScheme cs: ;
    skos:prefLabel "spherulite"@en ;
.

:stock
    a skos:Concept ;
    skos:broader :intrusion ;
    skos:definition "a discordant magma body with exposed surface area of less than 100 square kilometres; may represent exposed portion of a much larger intrusion."@en ;
    skos:inScheme cs: ;
    skos:prefLabel "stock"@en ;
.

:symplectic-intergrowth
    a skos:Concept ;
    skos:definition "an intimate wormlike or irregular intergrowth of two different minerals"@en ;
    skos:inScheme cs: ;
    skos:prefLabel "symplectic intergrowth"@en ;
    skos:topConceptOf cs: ;
.

:unkown
    a skos:Concept ;
    skos:definition "mode of occurrence is unknown"@en ;
    skos:inScheme cs: ;
    skos:prefLabel "unknown"@en ;
    skos:topConceptOf cs: ;
.

:weathering-product
    a skos:Concept ;
    skos:definition "a secondary mineral or material derived from weathering of a rock"@en ;
    skos:inScheme cs: ;
    skos:prefLabel "weathering product"@en ;
    skos:topConceptOf cs: ;
.

:xenoblast
    a skos:Concept ;
    skos:broader :crystalloblast ;
    skos:definition "a mineral that has grown during metamorphism without development of its characteristic crystal faces"@en ;
    skos:inScheme cs: ;
    skos:prefLabel "xenoblast"@en ;
.

:xenocryst
    a skos:Concept ;
    skos:broader :crystal ;
    skos:definition "a crystal that resembles a phenocryst in an igneous rock, but that is foreign to the rock in which it occurs"@en ;
    skos:inScheme cs: ;
    skos:prefLabel "xenocryst"@en ;
.

:xenolith
    a skos:Concept ;
    skos:broader :inclusion ;
    skos:definition "a foreign inclusion in an igneous rock; a fragment of an earlier-formed part of the igneous rock that has a different composition from that of the host rock"@en ;
    skos:inScheme cs: ;
    skos:prefLabel "xenolith"@en ;
.

:bed
    a skos:Concept ;
    skos:broader :band-layer ;
    skos:definition "a layer of sedimentary material bounded above and below by more or less well-defined bedding surfaces"@en ;
    skos:inScheme cs: ;
    skos:narrower :marker-bed ;
    skos:prefLabel "bed"@en ;
.

:cement
    a skos:Concept ;
    skos:definition "chemically precipitated material occuring in the space between grains or clasts of a sedimentary rock"@en ;
    skos:inScheme cs: ;
    skos:narrower :interstitial-material ;
    skos:prefLabel "cement"@en ;
    skos:topConceptOf cs: ;
.

:corona
    a skos:Concept ;
    skos:broader :mineral-overgrowth ;
    skos:definition "a zone of minerals, commonly with radial arrangement, around another mineral"@en ;
    skos:inScheme cs: ;
    skos:narrower :reaction-rim ;
    skos:prefLabel "corona"@en ;
.

:detritus
    a skos:Concept ;
    skos:definition "sedimentary material derived from the waethering and/or erosion"@en ;
    skos:inScheme cs: ;
    skos:narrower :clast ;
    skos:prefLabel "detritus"@en ;
    skos:topConceptOf cs: ;
.

:groundmass
    a skos:Concept ;
    skos:definition "the finer grained material between the phenocrysts of a porphyritic igneous rock"@en ;
    skos:inScheme cs: ;
    skos:narrower :interstitial-material ;
    skos:prefLabel "groundmass"@en ;
    skos:topConceptOf cs: ;
.

:lava-flow
    a skos:Concept ;
    skos:broader :volcanic-feature ;
    skos:definition "a tabular extrusive igneous body."@en ;
    skos:inScheme cs: ;
    skos:narrower :pillow ;
    skos:prefLabel "lava flow"@en ;
.

:matrix
    a skos:Concept ;
    skos:definition "the finer grained material between the larger grains or clasts of a sedimentary rock"@en ;
    skos:inScheme cs: ;
    skos:narrower :interstitial-material ;
    skos:prefLabel "matrix"@en ;
    skos:topConceptOf cs: ;
.

:mineral-overgrowth
    a skos:Concept ;
    skos:definition "growth of one mineral around the margin of a pre-existing mineral grain"@en ;
    skos:inScheme cs: ;
    skos:narrower :corona ;
    skos:prefLabel "mineral overgrowth"@en ;
    skos:topConceptOf cs: ;
.

:phacolith
    a skos:Concept ;
    skos:broader :intrusion ;
    skos:definition "a concordant, lenticular intrusion, emplaced along a fold axis"@en ;
    skos:inScheme cs: ;
    skos:narrower :harpolith ;
    skos:prefLabel "phacolith"@en ;
.

:clast
    a skos:Concept ;
    skos:broader :detritus ;
    skos:definition "a fragment of pre-existing rocks which have been produced by the processes of weathering and/or erosion, and in general transported to a point of deposition."@en ;
    skos:inScheme cs: ;
    skos:narrower
        :bioclast ,
        :intraclast ;
    skos:prefLabel "clast"@en ;
.

:inclusion
    a skos:Concept ;
    skos:definition "a fragment of older material within an igneous rock to which it may or may not be genetically related"@en ;
    skos:inScheme cs: ;
    skos:narrower
        :enclave ,
        :xenolith ;
    skos:prefLabel "inclusion"@en ;
    skos:topConceptOf cs: ;
.

:interstitial-material
    a skos:Concept ;
    skos:broader
        :cement ,
        :groundmass ,
        :matrix ;
    skos:definition "the finer grained material that occurs between coarser grains or particles in a rock"@en ;
    skos:inScheme cs: ;
    skos:prefLabel "interstitial material"@en ;
.

:pyroclast
    a skos:Concept ;
    skos:broader :volcanic-feature ;
    skos:definition "a particle ejected during a volcanic eruption"@en ;
    skos:inScheme cs: ;
    skos:narrower
        :block ,
        :bomb ;
    skos:prefLabel "pyroclast"@en ;
.

:ring-complex
    a skos:Concept ;
    skos:broader :intrusion ;
    skos:definition "an association of ring dykes and cone sheets."@en ;
    skos:inScheme cs: ;
    skos:narrower
        :cone-sheet ,
        :righ-dyke ;
    skos:prefLabel "ring complex"@en ;
.

:vein
    a skos:Concept ;
    skos:definition "an epigenetic mineral filling of a fault or fracture in a host rock, in tabular or sheetlike form, often with associated host rock replacement."@en ;
    skos:inScheme cs: ;
    skos:narrower
        :irregular-vein ,
        :planar-vein ,
        :sigmoidal-vein ;
    skos:prefLabel "vein"@en ;
    skos:topConceptOf cs: ;
.

:band-layer
    a skos:Concept ;
    skos:definition "a thin layer, compositionally distinct from the surrounding material"@en ;
    skos:inScheme cs: ;
    skos:narrower
        :bed ,
        :gneissic-band ,
        :igneous-band ,
        :lens ;
    skos:prefLabel "band, layer"@en ;
    skos:topConceptOf cs: ;
.

:grain
    a skos:Concept ;
    skos:definition "a mineral or rock particle, generally lacking crystal faces, commonly in relation to sedimentary rocks"@en ;
    skos:inScheme cs: ;
    skos:narrower
        :oncolite ,
        :ooid ,
        :pellet ,
        :pisolite ;
    skos:prefLabel "grain"@en ;
    skos:topConceptOf cs: ;
.

:crystal
    a skos:Concept ;
    skos:definition "a homogeneous, solid body of a mineral or element having a regular repeating atomic arrangement"@en ;
    skos:inScheme cs: ;
    skos:narrower
        :crystalloblast ,
        :cumulate-mineral ,
        :glomerocryst ,
        :microlite ,
        :phenocryst ,
        :porphyroclast ,
        :xenocryst ;
    skos:prefLabel "crystal"@en ;
    skos:topConceptOf cs: ;
.

:crystalloblast
    a skos:Concept ;
    skos:broader :crystal ;
    skos:definition "a crystal of a mineral produced entirely by metamorphic processes"@en ;
    skos:inScheme cs: ;
    skos:narrower
        :holoblast ,
        :hypidioblast ,
        :idioblast ,
        :oikocryst ,
        :poikiloblast ,
        :porphyroblast ,
        :xenoblast ;
    skos:prefLabel "crystalloblast"@en ;
.

:volcanic-feature
    a skos:Concept ;
    skos:definition "a rock derived from igneous processes at or just below the Earth's surface"@en ;
    skos:inScheme cs: ;
    skos:narrower
        :amygdale ,
        :cooling-column ,
        :cryptoexplosive ,
        :extrusive-dome ,
        :lava-flow ,
        :plug ,
        :pyroclast ,
        :spherulite ;
    skos:prefLabel "volcanic feature"@en ;
    skos:topConceptOf cs: ;
.

:intrusion
    a skos:Concept ;
    skos:definition "a body of igneous rock formed by the process of emplacement of magma in pre-existing rock"@en ;
    skos:inScheme cs: ;
    skos:narrower
        :akmolith ,
        :apophysis ,
        :cactolith ,
        :chonolith ,
        :cupola ,
        :ductolith ,
        :dyke ,
        :dyke-swarm ,
        :ethmolith ,
        :fissure ,
        :high-level-pluton ,
        :laccolith ,
        :lopolith ,
        :phacolith ,
        :pipe ,
        :pluton ,
        :pod ,
        :ring-complex ,
        :sheet ,
        :sill ,
        :sphenolith ,
        :stock ;
    skos:prefLabel "intrusion"@en ;
    skos:topConceptOf cs: ;
.

cs:
    a skos:ConceptScheme ;
    rdfs:seeAlso "https://pid.geoscience.gov.au/dataset/ga/148553" ;
    owl:versionInfo "1" ;
    skos:changeNote "2024-10-16 NJC: update to be VocPub 4.10 valid"@en ;
    skos:definition "Mode of occurrence of geological units and samples (eg: dyke, bed, phenocryst)."@en ;
    skos:hasTopConcept
        :band-layer ,
        :batholith ,
        :cement ,
        :concretion ,
        :crystal ,
        :detritus ,
        :facies ,
        :floor-ascendant ,
        :grain ,
        :graphic-intergrowth ,
        :groundmass ,
        :hydrothermal-alteration ,
        :inclusion ,
        :intrusion ,
        :leucosome ,
        :matrix ,
        :melanosome ,
        :mineral-overgrowth ,
        :nodule ,
        :pseudomorph ,
        :roof-pendant ,
        :sedimentry-dyke ,
        :symplectic-intergrowth ,
        :unkown ,
        :vein ,
        :volcanic-feature ,
        :weathering-product ;
    skos:historyNote "Geoscience Australia Mode of Occurrence (FGDM.MODE_OCCURENCES)"@en ;
    skos:prefLabel "Field Geology - Mode of Occurrence"@en ;
    dcat:contactPoint "Team Lead - Information Services; Energy, Minerals and Groundwater Division " ;
    schema:creator <https://linked.data.gov.au/org/ga> ;
    schema:dateCreated "2022-08-09"^^xsd:date ;
    schema:dateModified "2024-10-16"^^xsd:date ;
    schema:publisher <https://linked.data.gov.au/org/ga> ;
.
