PREFIX cs: <https://pid.geoscience.gov.au/def/voc/ga/mode_of_occurrence>
PREFIX dcat: <http://www.w3.org/ns/dcat#>
PREFIX dcterms: <http://purl.org/dc/terms/>
PREFIX owl: <http://www.w3.org/2002/07/owl#>
PREFIX rdfs: <http://www.w3.org/2000/01/rdf-schema#>
PREFIX skos: <http://www.w3.org/2004/02/skos/core#>
PREFIX xsd: <http://www.w3.org/2001/XMLSchema#>

<https://pid.geoscience.gov.au/def/voc/ga/mode_of_occurrence/akmolith>
    a skos:Concept ;
    dcterms:identifier "akmolith"^^xsd:token ;
    skos:broader <https://pid.geoscience.gov.au/def/voc/ga/mode_of_occurrence/intrusion> ;
    skos:definition "an intrusion along a decollement zone, with or without tonguelike extensions into the surrounding rock"@en ;
    skos:inScheme cs: ;
    skos:prefLabel "akmolith"@en ;
.

<https://pid.geoscience.gov.au/def/voc/ga/mode_of_occurrence/amygdale>
    a skos:Concept ;
    dcterms:identifier "amygdale"^^xsd:token ;
    skos:broader <https://pid.geoscience.gov.au/def/voc/ga/mode_of_occurrence/volcanic_feature> ;
    skos:definition "a gas cavity or vesicle in an igneous rock which is filled with secondary minerals"@en ;
    skos:inScheme cs: ;
    skos:prefLabel "amygdale"@en ;
.

<https://pid.geoscience.gov.au/def/voc/ga/mode_of_occurrence/apophysis>
    a skos:Concept ;
    dcterms:identifier "apophysis"^^xsd:token ;
    skos:broader <https://pid.geoscience.gov.au/def/voc/ga/mode_of_occurrence/intrusion> ;
    skos:definition "an offshoot from a larger intrusive body"@en ;
    skos:inScheme cs: ;
    skos:prefLabel "apophysis"@en ;
.

<https://pid.geoscience.gov.au/def/voc/ga/mode_of_occurrence/batholith>
    a skos:Concept ;
    dcterms:identifier "batholith"^^xsd:token ;
    skos:definition "a discordant magma body with exposed surface area of more than 100 square kilometres; typically consists of multiple intrusions."@en ;
    skos:inScheme cs: ;
    skos:prefLabel "batholith"@en ;
    skos:topConceptOf cs: ;
.

<https://pid.geoscience.gov.au/def/voc/ga/mode_of_occurrence/bioclast>
    a skos:Concept ;
    dcterms:identifier "bioclast"^^xsd:token ;
    skos:broader <https://pid.geoscience.gov.au/def/voc/ga/mode_of_occurrence/clast> ;
    skos:definition "a fragment or clast in a rock composed of the remains of organisms"@en ;
    skos:inScheme cs: ;
    skos:prefLabel "bioclast"@en ;
.

<https://pid.geoscience.gov.au/def/voc/ga/mode_of_occurrence/block>
    a skos:Concept ;
    dcterms:identifier "block"^^xsd:token ;
    skos:broader <https://pid.geoscience.gov.au/def/voc/ga/mode_of_occurrence/pyroclast> ;
    skos:definition "an angular pyroclast > 64 mm"@en ;
    skos:inScheme cs: ;
    skos:prefLabel "block"@en ;
.

<https://pid.geoscience.gov.au/def/voc/ga/mode_of_occurrence/bomb>
    a skos:Concept ;
    dcterms:identifier "bomb"^^xsd:token ;
    skos:broader <https://pid.geoscience.gov.au/def/voc/ga/mode_of_occurrence/pyroclast> ;
    skos:definition "a clot of lava, usually mafic-ultramafic, ejected from a volcanic vent while viscous, and which assumes a rounded shape as it solidifies in flight"@en ;
    skos:inScheme cs: ;
    skos:prefLabel "bomb"@en ;
.

<https://pid.geoscience.gov.au/def/voc/ga/mode_of_occurrence/cactolith>
    a skos:Concept ;
    dcterms:identifier "cactolith"^^xsd:token ;
    skos:broader <https://pid.geoscience.gov.au/def/voc/ga/mode_of_occurrence/intrusion> ;
    skos:definition "an obscurely cactus-shaped intrusion."@en ;
    skos:inScheme cs: ;
    skos:prefLabel "cactolith"@en ;
.

<https://pid.geoscience.gov.au/def/voc/ga/mode_of_occurrence/chonolith>
    a skos:Concept ;
    dcterms:identifier "chonolith"^^xsd:token ;
    skos:broader <https://pid.geoscience.gov.au/def/voc/ga/mode_of_occurrence/intrusion> ;
    skos:definition "an intrusion so irregular as to defy description"@en ;
    skos:inScheme cs: ;
    skos:prefLabel "chonolith"@en ;
.

<https://pid.geoscience.gov.au/def/voc/ga/mode_of_occurrence/concretion>
    a skos:Concept ;
    dcterms:identifier "concretion"^^xsd:token ;
    skos:definition "a hard, compact mass or aggregate of mineral matter, normally subsperical but commonly oblate, disc-shaped or irregular.  Formed from precipitation from solution about a nucleus or centre"@en ;
    skos:inScheme cs: ;
    skos:prefLabel "concretion"@en ;
    skos:topConceptOf cs: ;
.

<https://pid.geoscience.gov.au/def/voc/ga/mode_of_occurrence/cone_sheet>
    a skos:Concept ;
    dcterms:identifier "cone_sheet"^^xsd:token ;
    skos:broader <https://pid.geoscience.gov.au/def/voc/ga/mode_of_occurrence/ring_complex> ;
    skos:definition "an arcuate dyke that dips 30-45 degrees towards the centre of the arc; occur in concentric sets, presumably converging at a magmatic centre"@en ;
    skos:inScheme cs: ;
    skos:prefLabel "cone sheet"@en ;
.

<https://pid.geoscience.gov.au/def/voc/ga/mode_of_occurrence/cooling_column>
    a skos:Concept ;
    dcterms:identifier "cooling_column"^^xsd:token ;
    skos:broader <https://pid.geoscience.gov.au/def/voc/ga/mode_of_occurrence/volcanic_feature> ;
    skos:definition "a cooling unit in a volcanic rock defined by polygonal jointing perpendicular to the flow surface"@en ;
    skos:inScheme cs: ;
    skos:prefLabel "cooling column"@en ;
.

<https://pid.geoscience.gov.au/def/voc/ga/mode_of_occurrence/cryptoexplosive>
    a skos:Concept ;
    dcterms:identifier "cryptoexplosive"^^xsd:token ;
    skos:broader <https://pid.geoscience.gov.au/def/voc/ga/mode_of_occurrence/volcanic_feature> ;
    skos:definition "a volcanic body of rock formed by subsurface explosive activity"@en ;
    skos:inScheme cs: ;
    skos:prefLabel "cryptoexplosive"@en ;
.

<https://pid.geoscience.gov.au/def/voc/ga/mode_of_occurrence/cumulate_mineral>
    a skos:Concept ;
    dcterms:identifier "cumulate_mineral"^^xsd:token ;
    skos:broader <https://pid.geoscience.gov.au/def/voc/ga/mode_of_occurrence/crystal> ;
    skos:definition "a crystal formed during accumulation of early-formed crystals from a magma"@en ;
    skos:inScheme cs: ;
    skos:prefLabel "cumulate mineral"@en ;
.

<https://pid.geoscience.gov.au/def/voc/ga/mode_of_occurrence/cupola>
    a skos:Concept ;
    dcterms:identifier "cupola"^^xsd:token ;
    skos:broader <https://pid.geoscience.gov.au/def/voc/ga/mode_of_occurrence/intrusion> ;
    skos:definition "a large upward projection of the roof of an igneous intrusion into the country rock above."@en ;
    skos:inScheme cs: ;
    skos:prefLabel "cupola"@en ;
.

<https://pid.geoscience.gov.au/def/voc/ga/mode_of_occurrence/ductolith>
    a skos:Concept ;
    dcterms:identifier "ductolith"^^xsd:token ;
    skos:broader <https://pid.geoscience.gov.au/def/voc/ga/mode_of_occurrence/intrusion> ;
    skos:definition "a concordant intrusion, teardrop-shaped in cross section"@en ;
    skos:inScheme cs: ;
    skos:prefLabel "ductolith"@en ;
.

<https://pid.geoscience.gov.au/def/voc/ga/mode_of_occurrence/dyke>
    a skos:Concept ;
    dcterms:identifier "dyke"^^xsd:token ;
    skos:broader <https://pid.geoscience.gov.au/def/voc/ga/mode_of_occurrence/intrusion> ;
    skos:definition "a tabular igneous intrusion that cuts across the bedding or foliation of the country rock"@en ;
    skos:inScheme cs: ;
    skos:prefLabel "dyke"@en ;
.

<https://pid.geoscience.gov.au/def/voc/ga/mode_of_occurrence/dyke_swarm>
    a skos:Concept ;
    dcterms:identifier "dyke_swarm"^^xsd:token ;
    skos:broader <https://pid.geoscience.gov.au/def/voc/ga/mode_of_occurrence/intrusion> ;
    skos:definition "a set of dykes, generally subparallel, with a common origin"@en ;
    skos:inScheme cs: ;
    skos:prefLabel "dyke swarm"@en ;
.

<https://pid.geoscience.gov.au/def/voc/ga/mode_of_occurrence/enclave>
    a skos:Concept ;
    dcterms:identifier "enclave"^^xsd:token ;
    skos:broader <https://pid.geoscience.gov.au/def/voc/ga/mode_of_occurrence/inclusion> ;
    skos:definition "an inclusion within an igneous rock to which it may or may not be genetically related"@en ;
    skos:inScheme cs: ;
    skos:prefLabel "enclave"@en ;
.

<https://pid.geoscience.gov.au/def/voc/ga/mode_of_occurrence/ethmolith>
    a skos:Concept ;
    dcterms:identifier "ethmolith"^^xsd:token ;
    skos:broader <https://pid.geoscience.gov.au/def/voc/ga/mode_of_occurrence/intrusion> ;
    skos:definition "a discordant, funnel-shaped intrusion, tapers downward"@en ;
    skos:inScheme cs: ;
    skos:prefLabel "ethmolith"@en ;
.

<https://pid.geoscience.gov.au/def/voc/ga/mode_of_occurrence/extrusive_dome>
    a skos:Concept ;
    dcterms:identifier "extrusive_dome"^^xsd:token ;
    skos:broader <https://pid.geoscience.gov.au/def/voc/ga/mode_of_occurrence/volcanic_feature> ;
    skos:definition "an extrusion forming a bulbous dome above and around a volcanic vent"@en ;
    skos:inScheme cs: ;
    skos:prefLabel "extrusion dome"@en ;
.

<https://pid.geoscience.gov.au/def/voc/ga/mode_of_occurrence/facies>
    a skos:Concept ;
    dcterms:identifier "facies"^^xsd:token ;
    skos:definition "a lateral variant of a lithostratigraphic or metamorphic unit"@en ;
    skos:inScheme cs: ;
    skos:prefLabel "facies"@en ;
    skos:topConceptOf cs: ;
.

<https://pid.geoscience.gov.au/def/voc/ga/mode_of_occurrence/fissure>
    a skos:Concept ;
    dcterms:identifier "fissure"^^xsd:token ;
    skos:broader <https://pid.geoscience.gov.au/def/voc/ga/mode_of_occurrence/intrusion> ;
    skos:definition "a volcanic conduit having the form of a crack or fissure."@en ;
    skos:inScheme cs: ;
    skos:prefLabel "fissure"@en ;
.

<https://pid.geoscience.gov.au/def/voc/ga/mode_of_occurrence/floor_ascendant>
    a skos:Concept ;
    dcterms:identifier "floor_ascendant"^^xsd:token ;
    skos:definition "a upward projection of country rock into an igneous intrusion"@en ;
    skos:inScheme cs: ;
    skos:prefLabel "floor ascendant"@en ;
    skos:topConceptOf cs: ;
.

<https://pid.geoscience.gov.au/def/voc/ga/mode_of_occurrence/glomerocryst>
    a skos:Concept ;
    dcterms:identifier "glomerocryst"^^xsd:token ;
    skos:broader <https://pid.geoscience.gov.au/def/voc/ga/mode_of_occurrence/crystal> ;
    skos:definition "an aggregate of crystals of the same mineral"@en ;
    skos:inScheme cs: ;
    skos:prefLabel "glomerocryst"@en ;
.

<https://pid.geoscience.gov.au/def/voc/ga/mode_of_occurrence/gneissic_band>
    a skos:Concept ;
    dcterms:identifier "gneissic_band"^^xsd:token ;
    skos:broader <https://pid.geoscience.gov.au/def/voc/ga/mode_of_occurrence/band_layer> ;
    skos:definition "a compositional band or layer in a gneiss mineralogically distinct from the surrounding material"@en ;
    skos:inScheme cs: ;
    skos:prefLabel "gneissic band"@en ;
.

<https://pid.geoscience.gov.au/def/voc/ga/mode_of_occurrence/graphic_intergrowth>
    a skos:Concept ;
    dcterms:identifier "graphic_intergrowth"^^xsd:token ;
    skos:definition "a regular poikilitic intergrowth of triangular or linear-angular shaped grains of one mineral within a larger other mineral, typically quartz with alkali feldspar"@en ;
    skos:inScheme cs: ;
    skos:prefLabel "graphic intergrowth"@en ;
    skos:topConceptOf cs: ;
.

<https://pid.geoscience.gov.au/def/voc/ga/mode_of_occurrence/harpolith>
    a skos:Concept ;
    dcterms:identifier "harpolith"^^xsd:token ;
    skos:broader <https://pid.geoscience.gov.au/def/voc/ga/mode_of_occurrence/phacolith> ;
    skos:definition "a phacolith with a vertical axis; indicates multiple deformations"@en ;
    skos:inScheme cs: ;
    skos:prefLabel "harpolith"@en ;
.

<https://pid.geoscience.gov.au/def/voc/ga/mode_of_occurrence/high_level_pluton>
    a skos:Concept ;
    dcterms:identifier "high_level_pluton"^^xsd:token ;
    skos:broader <https://pid.geoscience.gov.au/def/voc/ga/mode_of_occurrence/intrusion> ;
    skos:definition "a pluton emplaced at a high or subvolcanic level in the crust"@en ;
    skos:inScheme cs: ;
    skos:prefLabel "high-level pluton"@en ;
.

<https://pid.geoscience.gov.au/def/voc/ga/mode_of_occurrence/holoblast>
    a skos:Concept ;
    dcterms:identifier "holoblast"^^xsd:token ;
    skos:broader <https://pid.geoscience.gov.au/def/voc/ga/mode_of_occurrence/crystalloblast> ;
    skos:definition "a crystalloblast that is newly and completely formed during metamorphism"@en ;
    skos:inScheme cs: ;
    skos:prefLabel "holoblast"@en ;
.

<https://pid.geoscience.gov.au/def/voc/ga/mode_of_occurrence/hydrothermal_alteration>
    a skos:Concept ;
    dcterms:identifier "hydrothermal_alteration"^^xsd:token ;
    skos:definition "a rock or mineral derived from hydrothermal alteration of a rock"@en ;
    skos:inScheme cs: ;
    skos:prefLabel "hydrothermal alteration"@en ;
    skos:topConceptOf cs: ;
.

<https://pid.geoscience.gov.au/def/voc/ga/mode_of_occurrence/hypidioblast>
    a skos:Concept ;
    dcterms:identifier "hypidioblast"^^xsd:token ;
    skos:broader <https://pid.geoscience.gov.au/def/voc/ga/mode_of_occurrence/crystalloblast> ;
    skos:definition "a crystalloblast that is formed during metamorphism and is bounded in part by its characteristic crystal faces"@en ;
    skos:inScheme cs: ;
    skos:prefLabel "hypidioblast"@en ;
.

<https://pid.geoscience.gov.au/def/voc/ga/mode_of_occurrence/idioblast>
    a skos:Concept ;
    dcterms:identifier "idioblast"^^xsd:token ;
    skos:broader <https://pid.geoscience.gov.au/def/voc/ga/mode_of_occurrence/crystalloblast> ;
    skos:definition "a crystalloblast that is formed during metamorphism and is bounded by its characteristic crystal faces"@en ;
    skos:inScheme cs: ;
    skos:prefLabel "idioblast"@en ;
.

<https://pid.geoscience.gov.au/def/voc/ga/mode_of_occurrence/igneous_band>
    a skos:Concept ;
    dcterms:identifier "igneous_band"^^xsd:token ;
    skos:broader <https://pid.geoscience.gov.au/def/voc/ga/mode_of_occurrence/band_layer> ;
    skos:definition "a compositional band or layer in an igneous rock mineralogically distict from the surrounding material"@en ;
    skos:inScheme cs: ;
    skos:prefLabel "igneous band"@en ;
.

<https://pid.geoscience.gov.au/def/voc/ga/mode_of_occurrence/intraclast>
    a skos:Concept ;
    dcterms:identifier "intraclast"^^xsd:token ;
    skos:broader <https://pid.geoscience.gov.au/def/voc/ga/mode_of_occurrence/clast> ;
    skos:definition "a clast or fragment in a sedimentary rock of another penecontemporaneous sedimentary rock that has been eroded within the basin of deposition"@en ;
    skos:inScheme cs: ;
    skos:prefLabel "intraclast"@en ;
.

<https://pid.geoscience.gov.au/def/voc/ga/mode_of_occurrence/irregular_vein>
    a skos:Concept ;
    dcterms:identifier "irregular_vein"^^xsd:token ;
    skos:broader <https://pid.geoscience.gov.au/def/voc/ga/mode_of_occurrence/vein> ;
    skos:definition "a vein with no obvious form."@en ;
    skos:inScheme cs: ;
    skos:prefLabel "irregular vein"@en ;
.

<https://pid.geoscience.gov.au/def/voc/ga/mode_of_occurrence/laccolith>
    a skos:Concept ;
    dcterms:identifier "laccolith"^^xsd:token ;
    skos:broader <https://pid.geoscience.gov.au/def/voc/ga/mode_of_occurrence/intrusion> ;
    skos:definition "a concordant, flat-based, convex-up intrusion"@en ;
    skos:inScheme cs: ;
    skos:prefLabel "laccolith"@en ;
.

<https://pid.geoscience.gov.au/def/voc/ga/mode_of_occurrence/lens>
    a skos:Concept ;
    dcterms:identifier "lens"^^xsd:token ;
    skos:broader <https://pid.geoscience.gov.au/def/voc/ga/mode_of_occurrence/band_layer> ;
    skos:definition "a discontinuous layer or bed within a sedimentary rock"@en ;
    skos:inScheme cs: ;
    skos:prefLabel "lens"@en ;
.

<https://pid.geoscience.gov.au/def/voc/ga/mode_of_occurrence/leucosome>
    a skos:Concept ;
    dcterms:identifier "leucosome"^^xsd:token ;
    skos:definition "the light coloured part of a migmatite or other rock with compositional segregations, usually rich in quartz and feldspar"@en ;
    skos:inScheme cs: ;
    skos:prefLabel "leucosome"@en ;
    skos:topConceptOf cs: ;
.

<https://pid.geoscience.gov.au/def/voc/ga/mode_of_occurrence/lopolith>
    a skos:Concept ;
    dcterms:identifier "lopolith"^^xsd:token ;
    skos:broader <https://pid.geoscience.gov.au/def/voc/ga/mode_of_occurrence/intrusion> ;
    skos:definition "a large, concordant, typically layered igneous intrusion whose floor is convex-down and whose roof may be convex-down or flat."@en ;
    skos:inScheme cs: ;
    skos:prefLabel "lopolith"@en ;
.

<https://pid.geoscience.gov.au/def/voc/ga/mode_of_occurrence/marker_bed>
    a skos:Concept ;
    dcterms:identifier "marker_bed"^^xsd:token ;
    skos:broader <https://pid.geoscience.gov.au/def/voc/ga/mode_of_occurrence/bed> ;
    skos:definition "a laterally continuous stratigraphic marker within another unit."@en ;
    skos:inScheme cs: ;
    skos:prefLabel "marker bed"@en ;
.

<https://pid.geoscience.gov.au/def/voc/ga/mode_of_occurrence/melanosome>
    a skos:Concept ;
    dcterms:identifier "melanosome"^^xsd:token ;
    skos:definition "the dark coloured part of a migmatite or other rock with compositional segregations, rich in mafic minerals"@en ;
    skos:inScheme cs: ;
    skos:prefLabel "melanosome"@en ;
    skos:topConceptOf cs: ;
.

<https://pid.geoscience.gov.au/def/voc/ga/mode_of_occurrence/microlite>
    a skos:Concept ;
    dcterms:identifier "microlite"^^xsd:token ;
    skos:broader <https://pid.geoscience.gov.au/def/voc/ga/mode_of_occurrence/crystal> ;
    skos:definition "a microscopic crystal that polarises light and has some determinable optical properties"@en ;
    skos:inScheme cs: ;
    skos:prefLabel "microlite"@en ;
.

<https://pid.geoscience.gov.au/def/voc/ga/mode_of_occurrence/nodule>
    a skos:Concept ;
    dcterms:identifier "nodule"^^xsd:token ;
    skos:definition "A small rounded mass of a mineral or mineral aggregate, usually with a contrasting composition from the enclosing sediment or rock matrix in which it is embedded. A fragment of a coarse grained igneous rock occurring within a finer grained rock."@en ;
    skos:inScheme cs: ;
    skos:prefLabel "nodule"@en ;
    skos:topConceptOf cs: ;
.

<https://pid.geoscience.gov.au/def/voc/ga/mode_of_occurrence/oikocryst>
    a skos:Concept ;
    dcterms:identifier "oikocryst"^^xsd:token ;
    skos:broader <https://pid.geoscience.gov.au/def/voc/ga/mode_of_occurrence/crystalloblast> ;
    skos:definition "the enclosing crystal in a poikolitic texture"@en ;
    skos:inScheme cs: ;
    skos:prefLabel "oikocryst"@en ;
.

<https://pid.geoscience.gov.au/def/voc/ga/mode_of_occurrence/oncolite>
    a skos:Concept ;
    dcterms:identifier "oncolite"^^xsd:token ;
    skos:broader <https://pid.geoscience.gov.au/def/voc/ga/mode_of_occurrence/grain> ;
    skos:definition "a variously shaped, concentrically laminated, calcareous sedimentary structure, usually less than 10 cm in diameter, formed by the accretion of successive layered masses of blue-green algae"@en ;
    skos:inScheme cs: ;
    skos:prefLabel "oncolite"@en ;
.

<https://pid.geoscience.gov.au/def/voc/ga/mode_of_occurrence/ooid>
    a skos:Concept ;
    dcterms:identifier "ooid"^^xsd:token ;
    skos:broader <https://pid.geoscience.gov.au/def/voc/ga/mode_of_occurrence/grain> ;
    skos:definition "a small round or ovate accretionary particle in an oolitic rock, formed of concentric carbonate layers around a nucleus in shallow, wave-agitated water"@en ;
    skos:inScheme cs: ;
    skos:prefLabel "ooid"@en ;
.

<https://pid.geoscience.gov.au/def/voc/ga/mode_of_occurrence/pellet>
    a skos:Concept ;
    dcterms:identifier "pellet"^^xsd:token ;
    skos:broader <https://pid.geoscience.gov.au/def/voc/ga/mode_of_occurrence/grain> ;
    skos:definition "a small, usually rounded aggregate of clay-sized calcareous (micritic) material, devoid of internal structure, and contained within a well sorted carbonate rock"@en ;
    skos:inScheme cs: ;
    skos:prefLabel "pellet"@en ;
.

<https://pid.geoscience.gov.au/def/voc/ga/mode_of_occurrence/phenocryst>
    a skos:Concept ;
    dcterms:identifier "phenocryst"^^xsd:token ;
    skos:broader <https://pid.geoscience.gov.au/def/voc/ga/mode_of_occurrence/crystal> ;
    skos:definition "a relatively large, conspicuous crystal in a porphyrytic igneous rock"@en ;
    skos:inScheme cs: ;
    skos:prefLabel "phenocryst"@en ;
.

<https://pid.geoscience.gov.au/def/voc/ga/mode_of_occurrence/pillow>
    a skos:Concept ;
    dcterms:identifier "pillow"^^xsd:token ;
    skos:broader <https://pid.geoscience.gov.au/def/voc/ga/mode_of_occurrence/lava_flow> ;
    skos:definition "a pillow-like lava body extruded beneath water"@en ;
    skos:inScheme cs: ;
    skos:prefLabel "pillow"@en ;
.

<https://pid.geoscience.gov.au/def/voc/ga/mode_of_occurrence/pipe>
    a skos:Concept ;
    dcterms:identifier "pipe"^^xsd:token ;
    skos:broader <https://pid.geoscience.gov.au/def/voc/ga/mode_of_occurrence/intrusion> ;
    skos:definition "a vertical conduit through the Earth's crust below a volcano, through which magmatic materials have passed; usually filled with volcanic breccia and fragments of older rock."@en ;
    skos:inScheme cs: ;
    skos:prefLabel "pipe"@en ;
.

<https://pid.geoscience.gov.au/def/voc/ga/mode_of_occurrence/pisolite>
    a skos:Concept ;
    dcterms:identifier "pisolite"^^xsd:token ;
    skos:broader <https://pid.geoscience.gov.au/def/voc/ga/mode_of_occurrence/grain> ;
    skos:definition "a small round or ovate accretionary particle, larger and less regular than an ooid, formed by concentric precipitation around a nucleus typically of carbonate (limestone) or iron oxides (laterite)"@en ;
    skos:inScheme cs: ;
    skos:prefLabel "pisolite"@en ;
.

<https://pid.geoscience.gov.au/def/voc/ga/mode_of_occurrence/planar_vein>
    a skos:Concept ;
    dcterms:identifier "planar_vein"^^xsd:token ;
    skos:broader <https://pid.geoscience.gov.au/def/voc/ga/mode_of_occurrence/vein> ;
    skos:definition "a vein with length and width significantly greater than its thickness, giving the vein a tabular form."@en ;
    skos:inScheme cs: ;
    skos:prefLabel "planar vein"@en ;
.

<https://pid.geoscience.gov.au/def/voc/ga/mode_of_occurrence/plug>
    a skos:Concept ;
    dcterms:identifier "plug"^^xsd:token ;
    skos:broader <https://pid.geoscience.gov.au/def/voc/ga/mode_of_occurrence/volcanic_feature> ;
    skos:definition "a roughly cylindrical mass of congealed magma that fills the conduit of an inactive volcano"@en ;
    skos:inScheme cs: ;
    skos:prefLabel "plug"@en ;
.

<https://pid.geoscience.gov.au/def/voc/ga/mode_of_occurrence/pluton>
    a skos:Concept ;
    dcterms:identifier "pluton"^^xsd:token ;
    skos:broader <https://pid.geoscience.gov.au/def/voc/ga/mode_of_occurrence/intrusion> ;
    skos:definition "a deep-seated igneous intrusion"@en ;
    skos:inScheme cs: ;
    skos:prefLabel "pluton"@en ;
.

<https://pid.geoscience.gov.au/def/voc/ga/mode_of_occurrence/pod>
    a skos:Concept ;
    dcterms:identifier "pod"^^xsd:token ;
    skos:broader <https://pid.geoscience.gov.au/def/voc/ga/mode_of_occurrence/intrusion> ;
    skos:definition "an intrusion of elongate or lenticular form"@en ;
    skos:inScheme cs: ;
    skos:prefLabel "pod"@en ;
.

<https://pid.geoscience.gov.au/def/voc/ga/mode_of_occurrence/poikiloblast>
    a skos:Concept ;
    dcterms:identifier "poikiloblast"^^xsd:token ;
    skos:broader <https://pid.geoscience.gov.au/def/voc/ga/mode_of_occurrence/crystalloblast> ;
    skos:definition "a crystal formed by recrystallisation during metamorphism with numerous inclusions of smaller grains"@en ;
    skos:inScheme cs: ;
    skos:prefLabel "poikiloblast"@en ;
.

<https://pid.geoscience.gov.au/def/voc/ga/mode_of_occurrence/porphyroblast>
    a skos:Concept ;
    dcterms:identifier "porphyroblast"^^xsd:token ;
    skos:broader <https://pid.geoscience.gov.au/def/voc/ga/mode_of_occurrence/crystalloblast> ;
    skos:definition "a pseudoporphyritic crystal in a rock produced by metamorphic recrystallisation"@en ;
    skos:inScheme cs: ;
    skos:prefLabel "porphyroblast"@en ;
.

<https://pid.geoscience.gov.au/def/voc/ga/mode_of_occurrence/porphyroclast>
    a skos:Concept ;
    dcterms:identifier "porphyroclast"^^xsd:token ;
    skos:broader <https://pid.geoscience.gov.au/def/voc/ga/mode_of_occurrence/crystal> ;
    skos:definition "a paleoblast within a finer grained recrystalllised and/or pulverised matrix"@en ;
    skos:inScheme cs: ;
    skos:prefLabel "porphyroclast"@en ;
.

<https://pid.geoscience.gov.au/def/voc/ga/mode_of_occurrence/pseudomorph>
    a skos:Concept ;
    dcterms:identifier "pseudomorph"^^xsd:token ;
    skos:definition "a secondary mineral whose outward crystal form has been inherited from the orignal mineral it has replaced"@en ;
    skos:inScheme cs: ;
    skos:prefLabel "pseudomorph"@en ;
    skos:topConceptOf cs: ;
.

<https://pid.geoscience.gov.au/def/voc/ga/mode_of_occurrence/reaction_rim>
    a skos:Concept ;
    dcterms:identifier "reaction_rim"^^xsd:token ;
    skos:broader <https://pid.geoscience.gov.au/def/voc/ga/mode_of_occurrence/corona> ;
    skos:definition "a peripheral zone around a mineral composed of the products of the reaction of an early solidified mineral with a surrounding melt"@en ;
    skos:inScheme cs: ;
    skos:prefLabel "reaction rim"@en ;
.

<https://pid.geoscience.gov.au/def/voc/ga/mode_of_occurrence/righ_dyke>
    a skos:Concept ;
    dcterms:identifier "righ_dyke"^^xsd:token ;
    skos:broader <https://pid.geoscience.gov.au/def/voc/ga/mode_of_occurrence/ring_complex> ;
    skos:definition "an arcuate or subcircular dyke, generally associated with a volcanic centre."@en ;
    skos:inScheme cs: ;
    skos:prefLabel "ring dyke"@en ;
.

<https://pid.geoscience.gov.au/def/voc/ga/mode_of_occurrence/roof_pendant>
    a skos:Concept ;
    dcterms:identifier "roof_pendant"^^xsd:token ;
    skos:definition "a downward projection of country rock into an igneous intrusion"@en ;
    skos:inScheme cs: ;
    skos:prefLabel "roof pendant"@en ;
    skos:topConceptOf cs: ;
.

<https://pid.geoscience.gov.au/def/voc/ga/mode_of_occurrence/sedimentry_dyke>
    a skos:Concept ;
    dcterms:identifier "sedimentry_dyke"^^xsd:token ;
    skos:definition "a tabular sedimentary intrusion that cuts across the bedding or foliation of the host rock"@en ;
    skos:inScheme cs: ;
    skos:prefLabel "sedimentary dyke"@en ;
    skos:topConceptOf cs: ;
.

<https://pid.geoscience.gov.au/def/voc/ga/mode_of_occurrence/sheet>
    a skos:Concept ;
    dcterms:identifier "sheet"^^xsd:token ;
    skos:broader <https://pid.geoscience.gov.au/def/voc/ga/mode_of_occurrence/intrusion> ;
    skos:definition "a tabular intrusion, concordant or slightly discordant."@en ;
    skos:inScheme cs: ;
    skos:prefLabel "sheet"@en ;
.

<https://pid.geoscience.gov.au/def/voc/ga/mode_of_occurrence/sigmoidal_vein>
    a skos:Concept ;
    dcterms:identifier "sigmoidal_vein"^^xsd:token ;
    skos:broader <https://pid.geoscience.gov.au/def/voc/ga/mode_of_occurrence/vein> ;
    skos:definition "a vein is curved so as to resemble the letter S in section."@en ;
    skos:inScheme cs: ;
    skos:prefLabel "sigmoidal vein"@en ;
.

<https://pid.geoscience.gov.au/def/voc/ga/mode_of_occurrence/sill>
    a skos:Concept ;
    dcterms:identifier "sill"^^xsd:token ;
    skos:broader <https://pid.geoscience.gov.au/def/voc/ga/mode_of_occurrence/intrusion> ;
    skos:definition "a tabular igneous intrusion that parallels the bedding or foliation of the country rock."@en ;
    skos:inScheme cs: ;
    skos:prefLabel "sill"@en ;
.

<https://pid.geoscience.gov.au/def/voc/ga/mode_of_occurrence/sphenolith>
    a skos:Concept ;
    dcterms:identifier "sphenolith"^^xsd:token ;
    skos:broader <https://pid.geoscience.gov.au/def/voc/ga/mode_of_occurrence/intrusion> ;
    skos:definition "a wedge-like intrusion, partly concordant, partly discordant."@en ;
    skos:inScheme cs: ;
    skos:prefLabel "sphenolith"@en ;
.

<https://pid.geoscience.gov.au/def/voc/ga/mode_of_occurrence/spherulite>
    a skos:Concept ;
    dcterms:identifier "spherulite"^^xsd:token ;
    skos:broader <https://pid.geoscience.gov.au/def/voc/ga/mode_of_occurrence/volcanic_feature> ;
    skos:definition "a rounded or spherical mass of acicular crystals, commonly of feldspar radiating from a central point.  Commonly formed from devitrification of volcanic glass"@en ;
    skos:inScheme cs: ;
    skos:prefLabel "spherulite"@en ;
.

<https://pid.geoscience.gov.au/def/voc/ga/mode_of_occurrence/stock>
    a skos:Concept ;
    dcterms:identifier "stock"^^xsd:token ;
    skos:broader <https://pid.geoscience.gov.au/def/voc/ga/mode_of_occurrence/intrusion> ;
    skos:definition "a discordant magma body with exposed surface area of less than 100 square kilometres; may represent exposed portion of a much larger intrusion."@en ;
    skos:inScheme cs: ;
    skos:prefLabel "stock"@en ;
.

<https://pid.geoscience.gov.au/def/voc/ga/mode_of_occurrence/symplectic_intergrowth>
    a skos:Concept ;
    dcterms:identifier "symplectic_intergrowth"^^xsd:token ;
    skos:definition "an intimate wormlike or irregular intergrowth of two different minerals"@en ;
    skos:inScheme cs: ;
    skos:prefLabel "symplectic intergrowth"@en ;
    skos:topConceptOf cs: ;
.

<https://pid.geoscience.gov.au/def/voc/ga/mode_of_occurrence/unkown>
    a skos:Concept ;
    dcterms:identifier "unkown"^^xsd:token ;
    skos:definition "mode of occurrence is unknown"@en ;
    skos:inScheme cs: ;
    skos:prefLabel "unknown"@en ;
    skos:topConceptOf cs: ;
.

<https://pid.geoscience.gov.au/def/voc/ga/mode_of_occurrence/weathering_product>
    a skos:Concept ;
    dcterms:identifier "weathering_product"^^xsd:token ;
    skos:definition "a secondary mineral or material derived from weathering of a rock"@en ;
    skos:inScheme cs: ;
    skos:prefLabel "weathering product"@en ;
    skos:topConceptOf cs: ;
.

<https://pid.geoscience.gov.au/def/voc/ga/mode_of_occurrence/xenoblast>
    a skos:Concept ;
    dcterms:identifier "xenoblast"^^xsd:token ;
    skos:broader <https://pid.geoscience.gov.au/def/voc/ga/mode_of_occurrence/crystalloblast> ;
    skos:definition "a mineral that has grown during metamorphism without development of its characteristic crystal faces"@en ;
    skos:inScheme cs: ;
    skos:prefLabel "xenoblast"@en ;
.

<https://pid.geoscience.gov.au/def/voc/ga/mode_of_occurrence/xenocryst>
    a skos:Concept ;
    dcterms:identifier "xenocryst"^^xsd:token ;
    skos:broader <https://pid.geoscience.gov.au/def/voc/ga/mode_of_occurrence/crystal> ;
    skos:definition "a crystal that resembles a phenocryst in an igneous rock, but that is foreign to the rock in which it occurs"@en ;
    skos:inScheme cs: ;
    skos:prefLabel "xenocryst"@en ;
.

<https://pid.geoscience.gov.au/def/voc/ga/mode_of_occurrence/xenolith>
    a skos:Concept ;
    dcterms:identifier "xenolith"^^xsd:token ;
    skos:broader <https://pid.geoscience.gov.au/def/voc/ga/mode_of_occurrence/inclusion> ;
    skos:definition "a foreign inclusion in an igneous rock; a fragment of an earlier-formed part of the igneous rock that has a different composition from that of the host rock"@en ;
    skos:inScheme cs: ;
    skos:prefLabel "xenolith"@en ;
.

<https://pid.geoscience.gov.au/def/voc/ga/mode_of_occurrence/bed>
    a skos:Concept ;
    dcterms:identifier "bed"^^xsd:token ;
    skos:broader <https://pid.geoscience.gov.au/def/voc/ga/mode_of_occurrence/band_layer> ;
    skos:definition "a layer of sedimentary material bounded above and below by more or less well-defined bedding surfaces"@en ;
    skos:inScheme cs: ;
    skos:narrower <https://pid.geoscience.gov.au/def/voc/ga/mode_of_occurrence/marker_bed> ;
    skos:prefLabel "bed"@en ;
.

<https://pid.geoscience.gov.au/def/voc/ga/mode_of_occurrence/cement>
    a skos:Concept ;
    dcterms:identifier "cement"^^xsd:token ;
    skos:definition "chemically precipitated material occuring in the space between grains or clasts of a sedimentary rock"@en ;
    skos:inScheme cs: ;
    skos:narrower <https://pid.geoscience.gov.au/def/voc/ga/mode_of_occurrence/interstitial_material> ;
    skos:prefLabel "cement"@en ;
    skos:topConceptOf cs: ;
.

<https://pid.geoscience.gov.au/def/voc/ga/mode_of_occurrence/corona>
    a skos:Concept ;
    dcterms:identifier "corona"^^xsd:token ;
    skos:broader <https://pid.geoscience.gov.au/def/voc/ga/mode_of_occurrence/mineral_overgrowth> ;
    skos:definition "a zone of minerals, commonly with radial arrangement, around another mineral"@en ;
    skos:inScheme cs: ;
    skos:narrower <https://pid.geoscience.gov.au/def/voc/ga/mode_of_occurrence/reaction_rim> ;
    skos:prefLabel "corona"@en ;
.

<https://pid.geoscience.gov.au/def/voc/ga/mode_of_occurrence/detritus>
    a skos:Concept ;
    dcterms:identifier "detritus"^^xsd:token ;
    skos:definition "sedimentary material derived from the waethering and/or erosion"@en ;
    skos:inScheme cs: ;
    skos:narrower <https://pid.geoscience.gov.au/def/voc/ga/mode_of_occurrence/clast> ;
    skos:prefLabel "detritus"@en ;
    skos:topConceptOf cs: ;
.

<https://pid.geoscience.gov.au/def/voc/ga/mode_of_occurrence/groundmass>
    a skos:Concept ;
    dcterms:identifier "groundmass"^^xsd:token ;
    skos:definition "the finer grained material between the phenocrysts of a porphyritic igneous rock"@en ;
    skos:inScheme cs: ;
    skos:narrower <https://pid.geoscience.gov.au/def/voc/ga/mode_of_occurrence/interstitial_material> ;
    skos:prefLabel "groundmass"@en ;
    skos:topConceptOf cs: ;
.

<https://pid.geoscience.gov.au/def/voc/ga/mode_of_occurrence/lava_flow>
    a skos:Concept ;
    dcterms:identifier "lava_flow"^^xsd:token ;
    skos:broader <https://pid.geoscience.gov.au/def/voc/ga/mode_of_occurrence/volcanic_feature> ;
    skos:definition "a tabular extrusive igneous body."@en ;
    skos:inScheme cs: ;
    skos:narrower <https://pid.geoscience.gov.au/def/voc/ga/mode_of_occurrence/pillow> ;
    skos:prefLabel "lava flow"@en ;
.

<https://pid.geoscience.gov.au/def/voc/ga/mode_of_occurrence/matrix>
    a skos:Concept ;
    dcterms:identifier "matrix"^^xsd:token ;
    skos:definition "the finer grained material between the larger grains or clasts of a sedimentary rock"@en ;
    skos:inScheme cs: ;
    skos:narrower <https://pid.geoscience.gov.au/def/voc/ga/mode_of_occurrence/interstitial_material> ;
    skos:prefLabel "matrix"@en ;
    skos:topConceptOf cs: ;
.

<https://pid.geoscience.gov.au/def/voc/ga/mode_of_occurrence/mineral_overgrowth>
    a skos:Concept ;
    dcterms:identifier "mineral_overgrowth"^^xsd:token ;
    skos:definition "growth of one mineral around the margin of a pre-existing mineral grain"@en ;
    skos:inScheme cs: ;
    skos:narrower <https://pid.geoscience.gov.au/def/voc/ga/mode_of_occurrence/corona> ;
    skos:prefLabel "mineral overgrowth"@en ;
    skos:topConceptOf cs: ;
.

<https://pid.geoscience.gov.au/def/voc/ga/mode_of_occurrence/phacolith>
    a skos:Concept ;
    dcterms:identifier "phacolith"^^xsd:token ;
    skos:broader <https://pid.geoscience.gov.au/def/voc/ga/mode_of_occurrence/intrusion> ;
    skos:definition "a concordant, lenticular intrusion, emplaced along a fold axis"@en ;
    skos:inScheme cs: ;
    skos:narrower <https://pid.geoscience.gov.au/def/voc/ga/mode_of_occurrence/harpolith> ;
    skos:prefLabel "phacolith"@en ;
.

<https://pid.geoscience.gov.au/def/voc/ga/mode_of_occurrence/clast>
    a skos:Concept ;
    dcterms:identifier "clast"^^xsd:token ;
    skos:broader <https://pid.geoscience.gov.au/def/voc/ga/mode_of_occurrence/detritus> ;
    skos:definition "a fragment of pre-existing rocks which have been produced by the processes of weathering and/or erosion, and in general transported to a point of deposition."@en ;
    skos:inScheme cs: ;
    skos:narrower
        <https://pid.geoscience.gov.au/def/voc/ga/mode_of_occurrence/bioclast> ,
        <https://pid.geoscience.gov.au/def/voc/ga/mode_of_occurrence/intraclast> ;
    skos:prefLabel "clast"@en ;
.

<https://pid.geoscience.gov.au/def/voc/ga/mode_of_occurrence/inclusion>
    a skos:Concept ;
    dcterms:identifier "inclusion"^^xsd:token ;
    skos:definition "a fragment of older material within an igneous rock to which it may or may not be genetically related"@en ;
    skos:inScheme cs: ;
    skos:narrower
        <https://pid.geoscience.gov.au/def/voc/ga/mode_of_occurrence/enclave> ,
        <https://pid.geoscience.gov.au/def/voc/ga/mode_of_occurrence/xenolith> ;
    skos:prefLabel "inclusion"@en ;
    skos:topConceptOf cs: ;
.

<https://pid.geoscience.gov.au/def/voc/ga/mode_of_occurrence/interstitial_material>
    a skos:Concept ;
    dcterms:identifier "interstitial_material"^^xsd:token ;
    skos:broader
        <https://pid.geoscience.gov.au/def/voc/ga/mode_of_occurrence/cement> ,
        <https://pid.geoscience.gov.au/def/voc/ga/mode_of_occurrence/groundmass> ,
        <https://pid.geoscience.gov.au/def/voc/ga/mode_of_occurrence/matrix> ;
    skos:definition "the finer grained material that occurs between coarser grains or particles in a rock"@en ;
    skos:inScheme cs: ;
    skos:prefLabel "interstitial material"@en ;
.

<https://pid.geoscience.gov.au/def/voc/ga/mode_of_occurrence/pyroclast>
    a skos:Concept ;
    dcterms:identifier "pyroclast"^^xsd:token ;
    skos:broader <https://pid.geoscience.gov.au/def/voc/ga/mode_of_occurrence/volcanic_feature> ;
    skos:definition "a particle ejected during a volcanic eruption"@en ;
    skos:inScheme cs: ;
    skos:narrower
        <https://pid.geoscience.gov.au/def/voc/ga/mode_of_occurrence/block> ,
        <https://pid.geoscience.gov.au/def/voc/ga/mode_of_occurrence/bomb> ;
    skos:prefLabel "pyroclast"@en ;
.

<https://pid.geoscience.gov.au/def/voc/ga/mode_of_occurrence/ring_complex>
    a skos:Concept ;
    dcterms:identifier "ring_complex"^^xsd:token ;
    skos:broader <https://pid.geoscience.gov.au/def/voc/ga/mode_of_occurrence/intrusion> ;
    skos:definition "an association of ring dykes and cone sheets."@en ;
    skos:inScheme cs: ;
    skos:narrower
        <https://pid.geoscience.gov.au/def/voc/ga/mode_of_occurrence/cone_sheet> ,
        <https://pid.geoscience.gov.au/def/voc/ga/mode_of_occurrence/righ_dyke> ;
    skos:prefLabel "ring complex"@en ;
.

<https://pid.geoscience.gov.au/def/voc/ga/mode_of_occurrence/vein>
    a skos:Concept ;
    dcterms:identifier "vein"^^xsd:token ;
    skos:definition "an epigenetic mineral filling of a fault or fracture in a host rock, in tabular or sheetlike form, often with associated host rock replacement."@en ;
    skos:inScheme cs: ;
    skos:narrower
        <https://pid.geoscience.gov.au/def/voc/ga/mode_of_occurrence/irregular_vein> ,
        <https://pid.geoscience.gov.au/def/voc/ga/mode_of_occurrence/planar_vein> ,
        <https://pid.geoscience.gov.au/def/voc/ga/mode_of_occurrence/sigmoidal_vein> ;
    skos:prefLabel "vein"@en ;
    skos:topConceptOf cs: ;
.

<https://pid.geoscience.gov.au/def/voc/ga/mode_of_occurrence/band_layer>
    a skos:Concept ;
    dcterms:identifier "band_layer"^^xsd:token ;
    skos:definition "a thin layer, compositionally distinct from the surrounding material"@en ;
    skos:inScheme cs: ;
    skos:narrower
        <https://pid.geoscience.gov.au/def/voc/ga/mode_of_occurrence/bed> ,
        <https://pid.geoscience.gov.au/def/voc/ga/mode_of_occurrence/gneissic_band> ,
        <https://pid.geoscience.gov.au/def/voc/ga/mode_of_occurrence/igneous_band> ,
        <https://pid.geoscience.gov.au/def/voc/ga/mode_of_occurrence/lens> ;
    skos:prefLabel "band, layer"@en ;
    skos:topConceptOf cs: ;
.

<https://pid.geoscience.gov.au/def/voc/ga/mode_of_occurrence/grain>
    a skos:Concept ;
    dcterms:identifier "grain"^^xsd:token ;
    skos:definition "a mineral or rock particle, generally lacking crystal faces, commonly in relation to sedimentary rocks"@en ;
    skos:inScheme cs: ;
    skos:narrower
        <https://pid.geoscience.gov.au/def/voc/ga/mode_of_occurrence/oncolite> ,
        <https://pid.geoscience.gov.au/def/voc/ga/mode_of_occurrence/ooid> ,
        <https://pid.geoscience.gov.au/def/voc/ga/mode_of_occurrence/pellet> ,
        <https://pid.geoscience.gov.au/def/voc/ga/mode_of_occurrence/pisolite> ;
    skos:prefLabel "grain"@en ;
    skos:topConceptOf cs: ;
.

<https://pid.geoscience.gov.au/def/voc/ga/mode_of_occurrence/crystal>
    a skos:Concept ;
    dcterms:identifier "crystal"^^xsd:token ;
    skos:definition "a homogeneous, solid body of a mineral or element having a regular repeating atomic arrangement"@en ;
    skos:inScheme cs: ;
    skos:narrower
        <https://pid.geoscience.gov.au/def/voc/ga/mode_of_occurrence/crystalloblast> ,
        <https://pid.geoscience.gov.au/def/voc/ga/mode_of_occurrence/cumulate_mineral> ,
        <https://pid.geoscience.gov.au/def/voc/ga/mode_of_occurrence/glomerocryst> ,
        <https://pid.geoscience.gov.au/def/voc/ga/mode_of_occurrence/microlite> ,
        <https://pid.geoscience.gov.au/def/voc/ga/mode_of_occurrence/phenocryst> ,
        <https://pid.geoscience.gov.au/def/voc/ga/mode_of_occurrence/porphyroclast> ,
        <https://pid.geoscience.gov.au/def/voc/ga/mode_of_occurrence/xenocryst> ;
    skos:prefLabel "crystal"@en ;
    skos:topConceptOf cs: ;
.

<https://pid.geoscience.gov.au/def/voc/ga/mode_of_occurrence/crystalloblast>
    a skos:Concept ;
    dcterms:identifier "crystalloblast"^^xsd:token ;
    skos:broader <https://pid.geoscience.gov.au/def/voc/ga/mode_of_occurrence/crystal> ;
    skos:definition "a crystal of a mineral produced entirely by metamorphic processes"@en ;
    skos:inScheme cs: ;
    skos:narrower
        <https://pid.geoscience.gov.au/def/voc/ga/mode_of_occurrence/holoblast> ,
        <https://pid.geoscience.gov.au/def/voc/ga/mode_of_occurrence/hypidioblast> ,
        <https://pid.geoscience.gov.au/def/voc/ga/mode_of_occurrence/idioblast> ,
        <https://pid.geoscience.gov.au/def/voc/ga/mode_of_occurrence/oikocryst> ,
        <https://pid.geoscience.gov.au/def/voc/ga/mode_of_occurrence/poikiloblast> ,
        <https://pid.geoscience.gov.au/def/voc/ga/mode_of_occurrence/porphyroblast> ,
        <https://pid.geoscience.gov.au/def/voc/ga/mode_of_occurrence/xenoblast> ;
    skos:prefLabel "crystalloblast"@en ;
.

<https://pid.geoscience.gov.au/def/voc/ga/mode_of_occurrence/volcanic_feature>
    a skos:Concept ;
    dcterms:identifier "volcanic_feature"^^xsd:token ;
    skos:definition "a rock derived from igneous processes at or just below the Earth's surface"@en ;
    skos:inScheme cs: ;
    skos:narrower
        <https://pid.geoscience.gov.au/def/voc/ga/mode_of_occurrence/amygdale> ,
        <https://pid.geoscience.gov.au/def/voc/ga/mode_of_occurrence/cooling_column> ,
        <https://pid.geoscience.gov.au/def/voc/ga/mode_of_occurrence/cryptoexplosive> ,
        <https://pid.geoscience.gov.au/def/voc/ga/mode_of_occurrence/extrusive_dome> ,
        <https://pid.geoscience.gov.au/def/voc/ga/mode_of_occurrence/lava_flow> ,
        <https://pid.geoscience.gov.au/def/voc/ga/mode_of_occurrence/plug> ,
        <https://pid.geoscience.gov.au/def/voc/ga/mode_of_occurrence/pyroclast> ,
        <https://pid.geoscience.gov.au/def/voc/ga/mode_of_occurrence/spherulite> ;
    skos:prefLabel "volcanic feature"@en ;
    skos:topConceptOf cs: ;
.

<https://pid.geoscience.gov.au/def/voc/ga/mode_of_occurrence/intrusion>
    a skos:Concept ;
    dcterms:identifier "intrusion"^^xsd:token ;
    skos:definition "a body of igneous rock formed by the process of emplacement of magma in pre-existing rock"@en ;
    skos:inScheme cs: ;
    skos:narrower
        <https://pid.geoscience.gov.au/def/voc/ga/mode_of_occurrence/akmolith> ,
        <https://pid.geoscience.gov.au/def/voc/ga/mode_of_occurrence/apophysis> ,
        <https://pid.geoscience.gov.au/def/voc/ga/mode_of_occurrence/cactolith> ,
        <https://pid.geoscience.gov.au/def/voc/ga/mode_of_occurrence/chonolith> ,
        <https://pid.geoscience.gov.au/def/voc/ga/mode_of_occurrence/cupola> ,
        <https://pid.geoscience.gov.au/def/voc/ga/mode_of_occurrence/ductolith> ,
        <https://pid.geoscience.gov.au/def/voc/ga/mode_of_occurrence/dyke> ,
        <https://pid.geoscience.gov.au/def/voc/ga/mode_of_occurrence/dyke_swarm> ,
        <https://pid.geoscience.gov.au/def/voc/ga/mode_of_occurrence/ethmolith> ,
        <https://pid.geoscience.gov.au/def/voc/ga/mode_of_occurrence/fissure> ,
        <https://pid.geoscience.gov.au/def/voc/ga/mode_of_occurrence/high_level_pluton> ,
        <https://pid.geoscience.gov.au/def/voc/ga/mode_of_occurrence/laccolith> ,
        <https://pid.geoscience.gov.au/def/voc/ga/mode_of_occurrence/lopolith> ,
        <https://pid.geoscience.gov.au/def/voc/ga/mode_of_occurrence/phacolith> ,
        <https://pid.geoscience.gov.au/def/voc/ga/mode_of_occurrence/pipe> ,
        <https://pid.geoscience.gov.au/def/voc/ga/mode_of_occurrence/pluton> ,
        <https://pid.geoscience.gov.au/def/voc/ga/mode_of_occurrence/pod> ,
        <https://pid.geoscience.gov.au/def/voc/ga/mode_of_occurrence/ring_complex> ,
        <https://pid.geoscience.gov.au/def/voc/ga/mode_of_occurrence/sheet> ,
        <https://pid.geoscience.gov.au/def/voc/ga/mode_of_occurrence/sill> ,
        <https://pid.geoscience.gov.au/def/voc/ga/mode_of_occurrence/sphenolith> ,
        <https://pid.geoscience.gov.au/def/voc/ga/mode_of_occurrence/stock> ;
    skos:prefLabel "intrusion"@en ;
    skos:topConceptOf cs: ;
.

cs:
    a skos:ConceptScheme ;
    dcterms:created "2022-08-09"^^xsd:date ;
    dcterms:creator <https://linked.data.gov.au/org/ga> ;
    dcterms:identifier "mode_of_occurrence"^^xsd:token ;
    dcterms:modified "2022-08-09"^^xsd:date ;
    dcterms:provenance "Geoscience Australia Mode of Occurence (FGDM.MODE_OCCURENCES)"@en ;
    dcterms:publisher <https://linked.data.gov.au/org/ga> ;
    rdfs:seeAlso <https://pid.geoscience.gov.au/dataset/ga/148553> ;
    owl:versionInfo "1" ;
    skos:definition "Mode of occurrence of geological units and samples (eg: dyke, bed, phenocryst)."@en ;
    skos:hasTopConcept
        <https://pid.geoscience.gov.au/def/voc/ga/mode_of_occurrence/band_layer> ,
        <https://pid.geoscience.gov.au/def/voc/ga/mode_of_occurrence/batholith> ,
        <https://pid.geoscience.gov.au/def/voc/ga/mode_of_occurrence/cement> ,
        <https://pid.geoscience.gov.au/def/voc/ga/mode_of_occurrence/concretion> ,
        <https://pid.geoscience.gov.au/def/voc/ga/mode_of_occurrence/crystal> ,
        <https://pid.geoscience.gov.au/def/voc/ga/mode_of_occurrence/detritus> ,
        <https://pid.geoscience.gov.au/def/voc/ga/mode_of_occurrence/facies> ,
        <https://pid.geoscience.gov.au/def/voc/ga/mode_of_occurrence/floor_ascendant> ,
        <https://pid.geoscience.gov.au/def/voc/ga/mode_of_occurrence/grain> ,
        <https://pid.geoscience.gov.au/def/voc/ga/mode_of_occurrence/graphic_intergrowth> ,
        <https://pid.geoscience.gov.au/def/voc/ga/mode_of_occurrence/groundmass> ,
        <https://pid.geoscience.gov.au/def/voc/ga/mode_of_occurrence/hydrothermal_alteration> ,
        <https://pid.geoscience.gov.au/def/voc/ga/mode_of_occurrence/inclusion> ,
        <https://pid.geoscience.gov.au/def/voc/ga/mode_of_occurrence/intrusion> ,
        <https://pid.geoscience.gov.au/def/voc/ga/mode_of_occurrence/leucosome> ,
        <https://pid.geoscience.gov.au/def/voc/ga/mode_of_occurrence/matrix> ,
        <https://pid.geoscience.gov.au/def/voc/ga/mode_of_occurrence/melanosome> ,
        <https://pid.geoscience.gov.au/def/voc/ga/mode_of_occurrence/mineral_overgrowth> ,
        <https://pid.geoscience.gov.au/def/voc/ga/mode_of_occurrence/nodule> ,
        <https://pid.geoscience.gov.au/def/voc/ga/mode_of_occurrence/pseudomorph> ,
        <https://pid.geoscience.gov.au/def/voc/ga/mode_of_occurrence/roof_pendant> ,
        <https://pid.geoscience.gov.au/def/voc/ga/mode_of_occurrence/sedimentry_dyke> ,
        <https://pid.geoscience.gov.au/def/voc/ga/mode_of_occurrence/symplectic_intergrowth> ,
        <https://pid.geoscience.gov.au/def/voc/ga/mode_of_occurrence/unkown> ,
        <https://pid.geoscience.gov.au/def/voc/ga/mode_of_occurrence/vein> ,
        <https://pid.geoscience.gov.au/def/voc/ga/mode_of_occurrence/volcanic_feature> ,
        <https://pid.geoscience.gov.au/def/voc/ga/mode_of_occurrence/weathering_product> ;
    skos:prefLabel "Field Geology - Mode of Occurrence"@en ;
    dcat:contactPoint "Team Lead - Information Services; Energy, Minerals and Groundwater Division " ;
.

