@prefix cs: <https://pid.geoscience.gov.au/def/voc/ga/proportion_term> .
@prefix dcat: <http://www.w3.org/ns/dcat#> .
@prefix dcterms: <http://purl.org/dc/terms/> .
@prefix owl: <http://www.w3.org/2002/07/owl#> .
@prefix rdfs: <http://www.w3.org/2000/01/rdf-schema#> .
@prefix skos: <http://www.w3.org/2004/02/skos/core#> .
@prefix xsd: <http://www.w3.org/2001/XMLSchema#> .

<https://pid.geoscience.gov.au/def/voc/ga/proportion_term/absent> 
	a skos:Concept ;
    dcterms:identifier "absent"^^xsd:token ;
    rdfs:isDefinedBy <http://resource.geosciml.org/classifier/cgi/proportionterm/all> ;
    skos:definition "The described material is not present."@en ;
    skos:inScheme cs: ;
    skos:prefLabel "absent"@en ;
    skos:topConceptOf cs: .

<https://pid.geoscience.gov.au/def/voc/ga/proportion_term/all> 
	a skos:Concept ;
    dcterms:identifier "all"^^xsd:token ;
    rdfs:isDefinedBy <http://resource.geosciml.org/classifier/cgi/proportionterm/all> ;
    skos:altLabel "only component"@en ;
	skos:broader <https://pid.geoscience.gov.au/def/voc/ga/proportion_term/present> ;
    skos:definition "The component comprises effectively the whole of the observed feature."@en ;
    skos:inScheme cs: ;
    skos:prefLabel "all"@en ;
    skos:topConceptOf cs: .

<https://pid.geoscience.gov.au/def/voc/ga/proportion_term/dominant> 
	a skos:Concept ;
    dcterms:identifier "dominant"^^xsd:token ;
    rdfs:isDefinedBy <http://resource.geosciml.org/classifier/cgi/proportionterm/dominant> ;
    skos:altLabel "predominant"@en ;
	skos:broader <https://pid.geoscience.gov.au/def/voc/ga/proportion_term/present> ;
    skos:definition "The component comprises a major part material of the observed feature, and is significantly greater than any other component; greater than 75%."@en ;
    skos:inScheme cs: ;
    skos:prefLabel "dominant"@en ;
    skos:topConceptOf cs: .

<https://pid.geoscience.gov.au/def/voc/ga/proportion_term/major> 
	a skos:Concept ;
    dcterms:identifier "major"^^xsd:token ;
    rdfs:isDefinedBy <http://resource.geosciml.org/classifier/cgi/proportionterm/major> ;
	skos:broader <https://pid.geoscience.gov.au/def/voc/ga/proportion_term/present> ;
    skos:definition "The component comprises a significant major part of the observed feature; between 50% and 100%."@en ;
    skos:inScheme cs: ;
    skos:prefLabel "major"@en ;
    skos:topConceptOf cs: .

<https://pid.geoscience.gov.au/def/voc/ga/proportion_term/minor> 
	a skos:Concept ;
    dcterms:identifier "minor"^^xsd:token ;
    rdfs:isDefinedBy <http://resource.geosciml.org/classifier/cgi/proportionterm/minor> ;
	skos:broader <https://pid.geoscience.gov.au/def/voc/ga/proportion_term/present> ;
    skos:definition "The component comprises a subordinate minor part of the observed feature; approximately between 5% and 25%."@en ;
    skos:inScheme cs: ;
    skos:prefLabel "minor"@en ;
    skos:topConceptOf cs: .

<https://pid.geoscience.gov.au/def/voc/ga/proportion_term/rare> 
	a skos:Concept ;
    dcterms:identifier "rare"^^xsd:token ;
    rdfs:isDefinedBy <http://resource.geosciml.org/classifier/cgi/proportionterm/rare> ;
	skos:broader <https://pid.geoscience.gov.au/def/voc/ga/proportion_term/present> ;
    skos:definition "The component comprises less than 5% of the observed feature."@en ;
    skos:inScheme cs: ;
    skos:prefLabel "rare"@en ;
    skos:topConceptOf cs: .

<https://pid.geoscience.gov.au/def/voc/ga/proportion_term/subordinate> 
	a skos:Concept ;
    dcterms:identifier "subordinate"^^xsd:token ;
    rdfs:isDefinedBy <http://resource.geosciml.org/classifier/cgi/proportionterm/subordinate> ;
	skos:broader <https://pid.geoscience.gov.au/def/voc/ga/proportion_term/present> ;
    skos:definition "The component comprises a significant, but subordinate, part of the observed feature; approximately between 5% and 50%."@en ;
    skos:inScheme cs: ;
    skos:prefLabel "subordinate"@en ;
    skos:topConceptOf cs: .

<https://pid.geoscience.gov.au/def/voc/ga/proportion_term/trace> 
	a skos:Concept ;
    dcterms:identifier "trace"^^xsd:token ;
    rdfs:isDefinedBy <http://resource.geosciml.org/classifier/cgi/proportionterm/trace> ;
	skos:broader <https://pid.geoscience.gov.au/def/voc/ga/proportion_term/present> ;
    skos:definition "The component comprises less than 1% of the observed feature. Presence is detectable but too small for accurate determination."@en ;
    skos:inScheme cs: ;
    skos:prefLabel "trace"@en ;
    skos:topConceptOf cs: .

<https://pid.geoscience.gov.au/def/voc/ga/proportion_term/variable> 
	a skos:Concept ;
    dcterms:identifier "variable"^^xsd:token ;
    rdfs:isDefinedBy <http://resource.geosciml.org/classifier/cgi/proportionterm/variable> ;
	skos:broader <https://pid.geoscience.gov.au/def/voc/ga/proportion_term/present> ;
    skos:definition "The component varies in proportion throughout the observed feature."@en ;
    skos:inScheme cs: ;
    skos:prefLabel "variable"@en ;
    skos:topConceptOf cs: .

<https://pid.geoscience.gov.au/def/voc/ga/proportion_term/present> 
	a skos:Concept ;
    dcterms:identifier "present"^^xsd:token ;
    skos:definition "The component is present in the observed feature, but the proportion is unknown."@en ;
    skos:inScheme cs: ;
    skos:narrower 
		<https://pid.geoscience.gov.au/def/voc/ga/proportion_term/all> ,
		<https://pid.geoscience.gov.au/def/voc/ga/proportion_term/dominant> ,
		<https://pid.geoscience.gov.au/def/voc/ga/proportion_term/major> ,
		<https://pid.geoscience.gov.au/def/voc/ga/proportion_term/subordinate> ,
		<https://pid.geoscience.gov.au/def/voc/ga/proportion_term/minor> ,
		<https://pid.geoscience.gov.au/def/voc/ga/proportion_term/rare> ,
		<https://pid.geoscience.gov.au/def/voc/ga/proportion_term/trace> ,
		<https://pid.geoscience.gov.au/def/voc/ga/proportion_term/variable> ;
    skos:prefLabel 
		"present"@en ;
    skos:topConceptOf cs: .

cs: a skos:ConceptScheme ;
    dcterms:created "2022-08-09"^^xsd:date ;
    dcterms:creator <https://linked.data.gov.au/org/ga> ;
    dcterms:identifier "proportion_term"^^xsd:token ;
    dcterms:modified "2022-08-09"^^xsd:date ;
    dcterms:provenance "Geoscience Australia Proportion Terms (FGDM.LU_PROPORTION_TERMS)"@en ;
    dcterms:publisher <https://linked.data.gov.au/org/ga> ;
    rdfs:seeAlso <https://pid.geoscience.gov.au/dataset/ga/148553> ;
    owl:versionInfo "1" ;
    skos:definition "The proportion of an observed or sampled feature that is comprised by one or more earth materials. The vocabulary also provides approximate numeric percent ranges that correspond to the qualitative terms"@en ;
    skos:hasTopConcept 
		<https://pid.geoscience.gov.au/def/voc/ga/proportion_term/absent> ,
    <https://pid.geoscience.gov.au/def/voc/ga/proportion_term/present> ,
		<https://pid.geoscience.gov.au/def/voc/ga/proportion_term/all> ,
		<https://pid.geoscience.gov.au/def/voc/ga/proportion_term/dominant> ,
		<https://pid.geoscience.gov.au/def/voc/ga/proportion_term/major> ,
		<https://pid.geoscience.gov.au/def/voc/ga/proportion_term/subordinate> ,
		<https://pid.geoscience.gov.au/def/voc/ga/proportion_term/minor> ,
		<https://pid.geoscience.gov.au/def/voc/ga/proportion_term/rare> ,
		<https://pid.geoscience.gov.au/def/voc/ga/proportion_term/trace> ,
		<https://pid.geoscience.gov.au/def/voc/ga/proportion_term/variable> ;
    skos:prefLabel "Field Geology - Proportion Terms "@en ;
    dcat:contactPoint "Team Lead - Information Services; Energy, Minerals and Groundwater Division" ;
.

