PREFIX : <https://pid.geoscience.gov.au/def/voc/ga/QaStatusCode/>
PREFIX cs: <https://pid.geoscience.gov.au/def/voc/ga/QaStatusCode>
PREFIX dcat: <http://www.w3.org/ns/dcat#>
PREFIX owl: <http://www.w3.org/2002/07/owl#>
PREFIX rdfs: <http://www.w3.org/2000/01/rdf-schema#>
PREFIX schema: <https://schema.org/>
PREFIX skos: <http://www.w3.org/2004/02/skos/core#>
PREFIX xsd: <http://www.w3.org/2001/XMLSchema#>

:c
    a skos:Concept ;
    skos:definition "This data has been checked. The data was entered by an Internal user."@en ;
    skos:inScheme cs: ;
    skos:prefLabel "C"@en ;
    skos:topConceptOf cs: ;
.

:u
    a skos:Concept ;
    skos:definition "This data has not been checked. The data was entered by an Internal user."@en ;
    skos:inScheme cs: ;
    skos:prefLabel "U"@en ;
    skos:topConceptOf cs: ;
.

cs:
    a skos:ConceptScheme ;
    rdfs:seeAlso "https://pid.geoscience.gov.au/dataset/ga/148553" ;
    owl:versionInfo "1" ;
    skos:changeNote "2024-10-16 NJC: update to be VocPub 4.10 valid"@en ;
    schema:citation "Geoscience Australia QA Status Code (A.QA_STATUS_CODES)" ;
    skos:definition "Indicates the status of whether or not QA of the data for this record has been undertaken (C - Checked, U - Unchecked)."@en ;
    skos:hasTopConcept
        :c ,
        :u ;
    skos:prefLabel "General Geology - QA Status Code"@en ;
    dcat:contactPoint "Team Lead - Information Services; Energy, Minerals and Groundwater" ;
    schema:creator <https://linked.data.gov.au/org/ga> ;
    schema:dateCreated "2022-08-09"^^xsd:date ;
    schema:dateModified "2024-10-16"^^xsd:date ;
    schema:publisher <https://linked.data.gov.au/org/ga> ;
.
