PREFIX : <https://pid.geoscience.gov.au/def/voc/ga/SourceRockQuality/>
PREFIX cs: <https://pid.geoscience.gov.au/def/voc/ga/SourceRockQuality>
PREFIX dcat: <http://www.w3.org/ns/dcat#>
PREFIX owl: <http://www.w3.org/2002/07/owl#>
PREFIX rdfs: <http://www.w3.org/2000/01/rdf-schema#>
PREFIX schema: <https://schema.org/>
PREFIX skos: <http://www.w3.org/2004/02/skos/core#>
PREFIX xsd: <http://www.w3.org/2001/XMLSchema#>

:effectiveSourceRock
    a skos:Concept ;
    skos:altLabel "ESR"@en ;
    skos:definition "An organic-rich rock that is presently generating and has expelled hydrocarbons"@en ;
    skos:inScheme cs: ;
    skos:prefLabel "effective source rock"@en ;
    skos:topConceptOf cs: ;
.

:notASourceRock
    a skos:Concept ;
    skos:altLabel "NSR"@en ;
    skos:definition "A sedimentary rock that does not contain enough carbon-rich and hydrogen-rich organic matter to generate hydrocarbons"@en ;
    skos:inScheme cs: ;
    skos:prefLabel "not a source rock"@en ;
    skos:topConceptOf cs: ;
.

:notAssessed
    a skos:Concept ;
    skos:altLabel "NA"@en ;
    skos:definition "Data has not been assessed for source rock quality"@en ;
    skos:inScheme cs: ;
    skos:prefLabel "not assessed"@en ;
    skos:topConceptOf cs: ;
.

:potentialSourceRock
    a skos:Concept ;
    skos:altLabel "PSR"@en ;
    skos:definition "A sedimentary rock that contains enough carbon-rich and hydrogen-rich organic matter to generate and expel hydrocarbons upon maturation"@en ;
    skos:inScheme cs: ;
    skos:prefLabel "potential source rock"@en ;
    skos:topConceptOf cs: ;
.

:relicEffectiveSourceRock
    a skos:Concept ;
    skos:altLabel "RESR"@en ;
    skos:definition "An effective source rock which has ceased to generate and expel hydrocabrons due to thermal cooling (uplift) before exhausting its organic matter supply"@en ;
    skos:inScheme cs: ;
    skos:prefLabel "relic effective source rock"@en ;
    skos:topConceptOf cs: ;
.

:spentSourceRock
    a skos:Concept ;
    skos:altLabel "SSR"@en ;
    skos:definition "An active source rock which has exhausted its ability to generate and expel hydrocarbons either through insufficient remaining organic matter or due to reaching overmaturity"@en ;
    skos:inScheme cs: ;
    skos:prefLabel "spent source rock"@en ;
    skos:topConceptOf cs: ;
.

cs:
    a skos:ConceptScheme ;
    rdfs:seeAlso "https://pid.geoscience.gov.au/dataset/ga/148553" ;
    owl:versionInfo "1" ;
    skos:changeNote "2024-10-16 NJC: update to be VocPub 4.10 valid"@en ;
    schema:citation "Geoscience Australia Source Rock Quality (ORGCHEM.LU_SOURCE_ROCK_QUALITY)" ;
    skos:definition "The quality of source rock from which organic chemistry samples were obtained."@en ;
    skos:hasTopConcept
        :effectiveSourceRock ,
        :notASourceRock ,
        :notAssessed ,
        :potentialSourceRock ,
        :relicEffectiveSourceRock ,
        :spentSourceRock ;
    skos:prefLabel "Boreholes Organic Geochemistry - Source Rock Quality"@en ;
    dcat:contactPoint "Team Lead - Information Services; Energy, Minerals and Groundwater Division" ;
    schema:creator <https://linked.data.gov.au/org/ga> ;
    schema:dateCreated "2022-08-09"^^xsd:date ;
    schema:dateModified "2024-10-16"^^xsd:date ;
    schema:publisher <https://linked.data.gov.au/org/ga> ;
.
