PREFIX cs: <https://pid.geoscience.gov.au/def/voc/ga/StatisticalResultQualifier>
PREFIX dcat: <http://www.w3.org/ns/dcat#>
PREFIX owl: <http://www.w3.org/2002/07/owl#>
PREFIX rdfs: <http://www.w3.org/2000/01/rdf-schema#>
PREFIX schema: <https://schema.org/>
PREFIX skos: <http://www.w3.org/2004/02/skos/core#>
PREFIX xsd: <http://www.w3.org/2001/XMLSchema#>

<https://pid.geoscience.gov.au/def/voc/ga/StatisticalResultQualifier/maximum>
    a skos:Concept ;
    schema:citation "http://resource.geoscience.gov.au/classifier/ga/resultqualifier/maximum" ;
    skos:definition "The highest numeric value of a sample set."@en ;
    skos:inScheme cs: ;
    skos:prefLabel "maximum"@en ;
    skos:topConceptOf cs: ;
.

<https://pid.geoscience.gov.au/def/voc/ga/StatisticalResultQualifier/mean>
    a skos:Concept ;
    skos:altLabel
        "arithmetic mean"@en ,
        "average"@en ;
    schema:citation "http://resource.geoscience.gov.au/classifier/ga/resultqualifier/mean" ;
    skos:definition "The sum of the values in a sample, divided by the number of values in that sample."@en ;
    skos:inScheme cs: ;
    skos:prefLabel "mean"@en ;
    skos:topConceptOf cs: ;
.

<https://pid.geoscience.gov.au/def/voc/ga/StatisticalResultQualifier/median>
    a skos:Concept ;
    schema:citation "http://resource.geoscience.gov.au/classifier/ga/resultqualifier/median" ;
    skos:definition "The numerical value separating the higher half of a data sample, a population, or a probability distribution, from the lower half."@en ;
    skos:inScheme cs: ;
    skos:prefLabel "median"@en ;
    skos:topConceptOf cs: ;
.

<https://pid.geoscience.gov.au/def/voc/ga/StatisticalResultQualifier/minimum>
    a skos:Concept ;
    schema:citation "http://resource.geoscience.gov.au/classifier/ga/resultqualifier/minimum" ;
    skos:definition "The lowest numeric value of a sample set."@en ;
    skos:inScheme cs: ;
    skos:prefLabel "minimum"@en ;
    skos:topConceptOf cs: ;
.

<https://pid.geoscience.gov.au/def/voc/ga/StatisticalResultQualifier/mode>
    a skos:Concept ;
    schema:citation "http://resource.geoscience.gov.au/classifier/ga/resultqualifier/mode" ;
    skos:definition "The value that appears most often in a set of data."@en ;
    skos:inScheme cs: ;
    skos:prefLabel "mode"@en ;
    skos:topConceptOf cs: ;
.

<https://pid.geoscience.gov.au/def/voc/ga/StatisticalResultQualifier/singleMeasurementPartSample>
    a skos:Concept ;
    schema:citation "http://resource.geoscience.gov.au/classifier/ga/resultqualifier/single_measurement_part_sample" ;
    skos:definition "A single or spot measurement of part of a specimen (e.g., a spot measurement of magnetic susceptibility on a rock outcrop) which may be expected to vary with the location or attitude of the instrument on the specimen"@en ;
    skos:inScheme cs: ;
    skos:prefLabel "single measurement - part sample"@en ;
    skos:topConceptOf cs: ;
.

<https://pid.geoscience.gov.au/def/voc/ga/StatisticalResultQualifier/singleMeasurementWholeSample>
    a skos:Concept ;
    schema:citation "http://resource.geoscience.gov.au/classifier/ga/resultqualifier/single_measurement_whole_sample" ;
    skos:definition "A single or spot measurement of the whole specimen, that may be expected to give the same result if repeated."@en ;
    skos:inScheme cs: ;
    skos:prefLabel "single measurement - whole sample"@en ;
    skos:topConceptOf cs: ;
.

<https://pid.geoscience.gov.au/def/voc/ga/StatisticalResultQualifier/unknown>
    a skos:Concept ;
    schema:citation "http://www.opengis.net/def/nil/OGC/0/unknown" ;
    skos:definition "The statistical type of measurement value is not known."@en ;
    skos:inScheme cs: ;
    skos:prefLabel "unknown"@en ;
    skos:topConceptOf cs: ;
.

<https://pid.geoscience.gov.au/def/voc/ga/StatisticalResultQualifier/weightedMean>
    a skos:Concept ;
    schema:citation "https://en.wikipedia.org/wiki/Inverse-variance_weighting" ;
    skos:definition "The sum of values in a sample, weighted proportional to their inverse variance, and divided by n-1 where n is the number of values in the population."@en ;
    skos:inScheme cs: ;
    skos:prefLabel "weighted mean"@en ;
    skos:topConceptOf cs: ;
.

<https://linked.data.gov.au/org/ga>
    a schema:Organization ;
    schema:description "Geoscience Australia is Australia's pre-eminent public sector geoscience organisation. It is the nation's trusted advisor on the geology and geography of Australia. It applies science and technology to describe and understand the Earth for the benefit of Australia."@en ;
    schema:name "Geoscience Australia" ;
    schema:url "https://www.ga.gov.au"^^xsd:anyURI ;
.

cs:
    a skos:ConceptScheme ;
    rdfs:seeAlso "https://pid.geoscience.gov.au/dataset/ga/148553" ;
    owl:versionInfo "1" ;
    skos:changeNote "2024-10-16 NJC: update to be VocPub 4.10 valid"@en ;
    schema:citation "Geoscience Australia Statistical Result Qualifier (ROCKPROPS.LU_RESULTQUALIFIER)" ;
    skos:definition "Statistical qualifier for rock property measurements (e.g. mean, maximum, median)."@en ;
    skos:hasTopConcept
        <https://pid.geoscience.gov.au/def/voc/ga/StatisticalResultQualifier/maximum> ,
        <https://pid.geoscience.gov.au/def/voc/ga/StatisticalResultQualifier/mean> ,
        <https://pid.geoscience.gov.au/def/voc/ga/StatisticalResultQualifier/median> ,
        <https://pid.geoscience.gov.au/def/voc/ga/StatisticalResultQualifier/minimum> ,
        <https://pid.geoscience.gov.au/def/voc/ga/StatisticalResultQualifier/mode> ,
        <https://pid.geoscience.gov.au/def/voc/ga/StatisticalResultQualifier/singleMeasurementPartSample> ,
        <https://pid.geoscience.gov.au/def/voc/ga/StatisticalResultQualifier/singleMeasurementWholeSample> ,
        <https://pid.geoscience.gov.au/def/voc/ga/StatisticalResultQualifier/unknown> ,
        <https://pid.geoscience.gov.au/def/voc/ga/StatisticalResultQualifier/weightedMean> ;
    skos:prefLabel "Geology Rock Properties - Result Qualifier"@en ;
    dcat:contactPoint "Team Lead - Information Services; Energy, Minerals and Groundwater Division" ;
    schema:creator <https://linked.data.gov.au/org/ga> ;
    schema:dateCreated "2022-08-09"^^xsd:date ;
    schema:dateModified "2024-10-16"^^xsd:date ;
    schema:publisher <https://linked.data.gov.au/org/ga> ;
.
