PREFIX : <https://pid.geoscience.gov.au/def/voc/ga/StatisticalUncertaintyTypes/>
PREFIX astatus: <https://linked.data.gov.au/def/reg-statuses/>
PREFIX cs: <https://pid.geoscience.gov.au/def/voc/ga/StatisticalUncertaintyTypes>
PREFIX dcat: <http://www.w3.org/ns/dcat#>
PREFIX dcterms: <http://purl.org/dc/terms/>
PREFIX owl: <http://www.w3.org/2002/07/owl#>
PREFIX rdfs: <http://www.w3.org/2000/01/rdf-schema#>
PREFIX schema: <https://schema.org/>
PREFIX skos: <http://www.w3.org/2004/02/skos/core#>
PREFIX xsd: <http://www.w3.org/2001/XMLSchema#>

:1Sigma
    a skos:Concept ;
    schema:citation <http://resource.geoscience.gov.au/classifier/ga/uncertaintytype/1sigma> ;
    skos:altLabel "standard deviation"@en ;
    skos:definition "The value of the \"sample standard deviation\" of a set of measurements used to derive a mean value. Used to illustrate the extent of \"dispersion\" of the measurements from the mean. For data conforming to a normal distribution, 1 sigma encompasses about 68% of the expected values."@en ;
    skos:inScheme cs: ;
    skos:prefLabel "1 sigma"@en ;
    skos:topConceptOf cs: ;
.

:1StandardError
    a skos:Concept ;
    schema:citation "https://en.wikipedia.org/wiki/Standard_error"^^xsd:anyURI ;
    skos:altLabel "1 standard error"@en ;
    skos:definition "An estimate of 1 standard deviation of the sampling distribution of the mean, derived from a particular sample of analysed data."@en ;
    skos:inScheme cs: ;
    skos:prefLabel "1 standard error"@en ;
    skos:topConceptOf cs: ;
.

:2Sigma
    a skos:Concept ;
    schema:citation <http://resource.geoscience.gov.au/classifier/ga/uncertaintytype/2sigma> ;
    skos:altLabel "twice standard deviation"@en ;
    skos:definition "The value corresponding to double the \"sample standard deviation\" of a set of measurements used to derive a mean value. Used to illustrate the extent of \"dispersion\" of the measurements from the mean. For data conforming to a normal distribution, 2 sigma encompasses about 95% of the expected values."@en ;
    skos:inScheme cs: ;
    skos:prefLabel "2 sigma"@en ;
    skos:topConceptOf cs: ;
.

:2StandardError
    a skos:Concept ;
    schema:citation "https://en.wikipedia.org/wiki/Standard_error"^^xsd:anyURI ;
    skos:altLabel "2 standard error"@en ;
    skos:definition "An estimate of 2 standard deviations of the sampling distribution of the mean, derived from a particular sample of analysed data."@en ;
    skos:inScheme cs: ;
    skos:prefLabel "2 standard error"@en ;
    skos:topConceptOf cs: ;
.

:3Sigma
    a skos:Concept ;
    schema:citation <http://resource.geoscience.gov.au/classifier/ga/uncertaintytype/3sigma> ;
    skos:altLabel "thrice standard deviation"@en ;
    skos:definition "The value corresponding to three times the \"sample standard deviation\" of a set of measurements used to derive a mean value. Used to illustrate the extent of \"dispersion\" of the measurements from the mean. For data conforming to a normal distribution, 3 sigma encompasses about 99.7% of the expected values."@en ;
    skos:inScheme cs: ;
    skos:prefLabel "3 sigma"@en ;
    skos:topConceptOf cs: ;
.

:95pcConfidence
    a skos:Concept ;
    schema:citation <http://resource.geoscience.gov.au/classifier/ga/uncertaintytype/95pc_confidence> ;
    skos:definition "The interval, expressed as a deviation centered on the mean value (and calculated directly from the population observations), which will encompass the true value of the measured parameter 95% of the time, if the underlying statistical model is correct."@en ;
    skos:inScheme cs: ;
    skos:prefLabel "95% confidence"@en ;
    skos:topConceptOf cs: ;
.

:99pcConfidence
    a skos:Concept ;
    schema:citation <http://resource.geoscience.gov.au/classifier/ga/uncertaintytype/95pc_confidence_asymmetric> ;
    skos:definition "The interval, expressed as a deviation centered on the mean value (and calculated directly from the population observations), which will encompass the true value of the measured parameter 99% of the time, if the underlying statistical model is correct."@en ;
    skos:inScheme cs: ;
    skos:prefLabel "99% confidence"@en ;
    skos:topConceptOf cs: ;
.

:alpha95
    a skos:Concept ;
    schema:citation <http://resource.geoscience.gov.au/classifier/ga/uncertaintytype/alpha95> ;
    skos:altLabel "95% angular confidence"@en ;
    skos:definition "A circular 95 % confidence estimate for directional data. An angular estimate of the circle of 95% confidence (p = 0.05) about the mean direction."@en ;
    skos:inScheme cs: ;
    skos:prefLabel "alpha95"@en ;
    skos:topConceptOf cs: ;
.

:delta
    a skos:Concept ;
    schema:citation <http://resource.geoscience.gov.au/classifier/ga/uncertaintytype/delta> ;
    skos:definition "A dispersion parameter for directional data. \"Delta\" decreases as the directions become less dispersed. In practice, when the number of samples is greater than 10 - 20, delta is approximately equal to the circular (or angular) standard deviation."@en ;
    skos:inScheme cs: ;
    skos:prefLabel "delta"@en ;
    skos:topConceptOf cs: ;
.

:kappa
    a skos:Concept ;
    schema:citation <http://resource.geoscience.gov.au/classifier/ga/uncertaintytype/kappa> ;
    skos:definition "A precision parameter for directional data, measuring the concentration of the distribution about the true mean direction. The larger the value of Kappa, the more concentrated the direction; Kappa is 0 for a distribution of directions that is uniform over the sphere and approaches infinite for directions concentrated at a point."@en ;
    skos:inScheme cs: ;
    skos:prefLabel "kappa"@en ;
    skos:topConceptOf cs: ;
.

:plusMinus
    a skos:Concept ;
    schema:citation <http://resource.geoscience.gov.au/classifier/ga/uncertaintytype/plus_minus> ;
    skos:altLabel
        "+/-"@en ,
        "plus or minus"@en ;
    skos:definition "Uncertainty quoted as plus or minus a number"@en ;
    skos:inScheme cs: ;
    skos:prefLabel "plus/minus"@en ;
    skos:topConceptOf cs: ;
.

:unknown
    a skos:Concept ;
    schema:citation <http://www.opengis.net/def/nil/OGC/0/unknown> ;
    skos:definition "The type of uncertainty associated with the measurement is unknown."@en ;
    skos:inScheme cs: ;
    skos:prefLabel "unknown"@en ;
    skos:topConceptOf cs: ;
.

cs:
    a skos:ConceptScheme ;
    dcterms:created "2022-08-09"^^xsd:date ;
    dcterms:creator <https://linked.data.gov.au/org/ga> ;
    dcterms:modified "2022-08-09"^^xsd:date ;
    dcterms:provenance "Geoscience Australia Statistical Uncertainty Type (ROCKPROPS.LU_UNCERTAINTYTYPE)"@en ;
    dcterms:publisher <https://linked.data.gov.au/org/ga> ;
    rdfs:seeAlso <https://pid.geoscience.gov.au/dataset/ga/148553> ;
    owl:versionInfo "1" ;
    skos:definition "The type of statistical uncertainty for rock property measurements (e.g. 1 sigma, 2 sigma, 99 percent confidence, unknown)."@en ;
    skos:hasTopConcept
        :1Sigma ,
        :1StandardError ,
        :2Sigma ,
        :2StandardError ,
        :3Sigma ,
        :95pcConfidence ,
        :99pcConfidence ,
        :alpha95 ,
        :delta ,
        :kappa ,
        :plusMinus ,
        :unknown ;
    skos:prefLabel "Geology Rock Properties - Statistical Uncertainty Type "@en ;
    dcat:contactPoint "Team Lead - Information Services; Energy, Minerals and Groundwater Division" ;
    schema:status astatus:experimental ;
.
