PREFIX cs: <https://pid.geoscience.gov.au/def/voc/ga/statisticalUncertaintyType>
PREFIX dcat: <http://www.w3.org/ns/dcat#>
PREFIX dcterms: <http://purl.org/dc/terms/>
PREFIX owl: <http://www.w3.org/2002/07/owl#>
PREFIX rdfs: <http://www.w3.org/2000/01/rdf-schema#>
PREFIX sdo: <https://schema.org/>
PREFIX skos: <http://www.w3.org/2004/02/skos/core#>
PREFIX xsd: <http://www.w3.org/2001/XMLSchema#>

<https://pid.geoscience.gov.au/def/voc/ga/statisticalUncertaintyType/1Sigma>
    a skos:Concept ;
    dcterms:identifier "1Sigma"^^xsd:token ;
    rdfs:isDefinedBy <http://resource.geoscience.gov.au/classifier/ga/uncertaintytype/1sigma> ;
    skos:altLabel "standard deviation"@en ;
    skos:definition "The value of the \"sample standard deviation\" of a set of measurements used to derive a mean value. Used to illustrate the extent of \"dispersion\" of the measurements from the mean. For data conforming to a normal distribution, 1 sigma encompasses about 68% of the expected values."@en ;
    skos:inScheme cs: ;
    skos:prefLabel "1 sigma"@en ;
    skos:topConceptOf cs: ;
.

<https://pid.geoscience.gov.au/def/voc/ga/statisticalUncertaintyType/1StandardError>
    a skos:Concept ;
    dcterms:identifier "1StandardError"^^xsd:token ;
    rdfs:isDefinedBy <https://en.wikipedia.org/wiki/Standard_error> ;
    skos:altLabel "1 standard error"@en ;
    skos:definition "An estimate of 1 standard deviation of the sampling distribution of the mean, derived from a particular sample of analysed data."@en ;
    skos:inScheme cs: ;
    skos:prefLabel "1 standard error"@en ;
    skos:topConceptOf cs: ;
.

<https://pid.geoscience.gov.au/def/voc/ga/statisticalUncertaintyType/2Sigma>
    a skos:Concept ;
    dcterms:identifier "2Sigma"^^xsd:token ;
    rdfs:isDefinedBy <http://resource.geoscience.gov.au/classifier/ga/uncertaintytype/2sigma> ;
    skos:altLabel "twice standard deviation"@en ;
    skos:definition "The value corresponding to double the \"sample standard deviation\" of a set of measurements used to derive a mean value. Used to illustrate the extent of \"dispersion\" of the measurements from the mean. For data conforming to a normal distribution, 2 sigma encompasses about 95% of the expected values."@en ;
    skos:inScheme cs: ;
    skos:prefLabel "2 sigma"@en ;
    skos:topConceptOf cs: ;
.

<https://pid.geoscience.gov.au/def/voc/ga/statisticalUncertaintyType/2StandardError>
    a skos:Concept ;
    dcterms:identifier "2StandardError"^^xsd:token ;
    rdfs:isDefinedBy <https://en.wikipedia.org/wiki/Standard_error> ;
    skos:altLabel "2 standard error"@en ;
    skos:definition "An estimate of 2 standard deviations of the sampling distribution of the mean, derived from a particular sample of analysed data."@en ;
    skos:inScheme cs: ;
    skos:prefLabel "2 standard error"@en ;
    skos:topConceptOf cs: ;
.

<https://pid.geoscience.gov.au/def/voc/ga/statisticalUncertaintyType/3Sigma>
    a skos:Concept ;
    dcterms:identifier "3Sigma"^^xsd:token ;
    rdfs:isDefinedBy <http://resource.geoscience.gov.au/classifier/ga/uncertaintytype/3sigma> ;
    skos:altLabel "thrice standard deviation"@en ;
    skos:definition "The value corresponding to three times the \"sample standard deviation\" of a set of measurements used to derive a mean value. Used to illustrate the extent of \"dispersion\" of the measurements from the mean. For data conforming to a normal distribution, 3 sigma encompasses about 99.7% of the expected values."@en ;
    skos:inScheme cs: ;
    skos:prefLabel "3 sigma"@en ;
    skos:topConceptOf cs: ;
.

<https://pid.geoscience.gov.au/def/voc/ga/statisticalUncertaintyType/95pcConfidence>
    a skos:Concept ;
    dcterms:identifier "95pcConfidence"^^xsd:token ;
    rdfs:isDefinedBy <http://resource.geoscience.gov.au/classifier/ga/uncertaintytype/95pc_confidence> ;
    skos:definition "The interval, expressed as a deviation centered on the mean value (and calculated directly from the population observations), which will encompass the true value of the measured parameter 95% of the time, if the underlying statistical model is correct."@en ;
    skos:inScheme cs: ;
    skos:prefLabel "95% confidence"@en ;
    skos:topConceptOf cs: ;
.

<https://pid.geoscience.gov.au/def/voc/ga/statisticalUncertaintyType/99pcConfidence>
    a skos:Concept ;
    dcterms:identifier "99pcConfidence"^^xsd:token ;
    rdfs:isDefinedBy <http://resource.geoscience.gov.au/classifier/ga/uncertaintytype/95pc_confidence_asymmetric> ;
    skos:definition "The interval, expressed as a deviation centered on the mean value (and calculated directly from the population observations), which will encompass the true value of the measured parameter 99% of the time, if the underlying statistical model is correct."@en ;
    skos:inScheme cs: ;
    skos:prefLabel "99% confidence"@en ;
    skos:topConceptOf cs: ;
.

<https://pid.geoscience.gov.au/def/voc/ga/statisticalUncertaintyType/alpha95>
    a skos:Concept ;
    dcterms:identifier "alpha95"^^xsd:token ;
    rdfs:isDefinedBy <http://resource.geoscience.gov.au/classifier/ga/uncertaintytype/alpha95> ;
    skos:altLabel "95% angular confidence"@en ;
    skos:definition "A circular 95 % confidence estimate for directional data. An angular estimate of the circle of 95% confidence (p = 0.05) about the mean direction."@en ;
    skos:inScheme cs: ;
    skos:prefLabel "alpha95"@en ;
    skos:topConceptOf cs: ;
.

<https://pid.geoscience.gov.au/def/voc/ga/statisticalUncertaintyType/delta>
    a skos:Concept ;
    dcterms:identifier "delta"^^xsd:token ;
    rdfs:isDefinedBy <http://resource.geoscience.gov.au/classifier/ga/uncertaintytype/delta> ;
    skos:definition "A dispersion parameter for directional data. \"Delta\" decreases as the directions become less dispersed. In practice, when the number of samples is greater than 10 - 20, delta is approximately equal to the circular (or angular) standard deviation."@en ;
    skos:inScheme cs: ;
    skos:prefLabel "delta"@en ;
    skos:topConceptOf cs: ;
.

<https://pid.geoscience.gov.au/def/voc/ga/statisticalUncertaintyType/kappa>
    a skos:Concept ;
    dcterms:identifier "kappa"^^xsd:token ;
    rdfs:isDefinedBy <http://resource.geoscience.gov.au/classifier/ga/uncertaintytype/kappa> ;
    skos:definition "A precision parameter for directional data, measuring the concentration of the distribution about the true mean direction. The larger the value of Kappa, the more concentrated the direction; Kappa is 0 for a distribution of directions that is uniform over the sphere and approaches infinite for directions concentrated at a point."@en ;
    skos:inScheme cs: ;
    skos:prefLabel "kappa"@en ;
    skos:topConceptOf cs: ;
.

<https://pid.geoscience.gov.au/def/voc/ga/statisticalUncertaintyType/plusMinus>
    a skos:Concept ;
    dcterms:identifier "plusMinus"^^xsd:token ;
    rdfs:isDefinedBy <http://resource.geoscience.gov.au/classifier/ga/uncertaintytype/plus_minus> ;
    skos:altLabel
        "+/-"@en ,
        "plus or minus"@en ;
    skos:definition "Uncertainty quoted as plus or minus a number"@en ;
    skos:inScheme cs: ;
    skos:prefLabel "plus/minus"@en ;
    skos:topConceptOf cs: ;
.

<https://pid.geoscience.gov.au/def/voc/ga/statisticalUncertaintyType/unknown>
    a skos:Concept ;
    dcterms:identifier "unknown"^^xsd:token ;
    rdfs:isDefinedBy <http://www.opengis.net/def/nil/OGC/0/unknown> ;
    skos:definition "The type of uncertainty associated with the measurement is unknown."@en ;
    skos:inScheme cs: ;
    skos:prefLabel "unknown"@en ;
    skos:topConceptOf cs: ;
.

<https://linked.data.gov.au/org/ga>
    a sdo:Organization ;
    sdo:description "Geoscience Australia is Australia's pre-eminent public sector geoscience organisation. It is the nation's trusted advisor on the geology and geography of Australia. It applies science and technology to describe and understand the Earth for the benefit of Australia."@en ;
    sdo:name "Geoscience Australia" ;
    sdo:url "https://www.ga.gov.au"^^xsd:anyURI ;
.

cs:
    a skos:ConceptScheme ;
    dcterms:created "2022-08-09"^^xsd:date ;
    dcterms:creator <https://linked.data.gov.au/org/ga> ;
    dcterms:identifier "statisticalUncertaintyType"^^xsd:token ;
    dcterms:modified "2022-08-09"^^xsd:date ;
    dcterms:provenance "Geoscience Australia Statistical Uncertainty Type (ROCKPROPS.LU_UNCERTAINTYTYPE)"@en ;
    dcterms:publisher <https://linked.data.gov.au/org/ga> ;
    rdfs:seeAlso <https://pid.geoscience.gov.au/dataset/ga/148553> ;
    owl:versionInfo "1" ;
    skos:definition "The type of statistical uncertainty for rock property measurements (e.g. 1 sigma, 2 sigma, 99 percent confidence, unknown)."@en ;
    skos:hasTopConcept
        <https://pid.geoscience.gov.au/def/voc/ga/statisticalUncertaintyType/1Sigma> ,
        <https://pid.geoscience.gov.au/def/voc/ga/statisticalUncertaintyType/1StandardError> ,
        <https://pid.geoscience.gov.au/def/voc/ga/statisticalUncertaintyType/2Sigma> ,
        <https://pid.geoscience.gov.au/def/voc/ga/statisticalUncertaintyType/2StandardError> ,
        <https://pid.geoscience.gov.au/def/voc/ga/statisticalUncertaintyType/3Sigma> ,
        <https://pid.geoscience.gov.au/def/voc/ga/statisticalUncertaintyType/95pcConfidence> ,
        <https://pid.geoscience.gov.au/def/voc/ga/statisticalUncertaintyType/99pcConfidence> ,
        <https://pid.geoscience.gov.au/def/voc/ga/statisticalUncertaintyType/alpha95> ,
        <https://pid.geoscience.gov.au/def/voc/ga/statisticalUncertaintyType/delta> ,
        <https://pid.geoscience.gov.au/def/voc/ga/statisticalUncertaintyType/kappa> ,
        <https://pid.geoscience.gov.au/def/voc/ga/statisticalUncertaintyType/plusMinus> ,
        <https://pid.geoscience.gov.au/def/voc/ga/statisticalUncertaintyType/unknown> ;
    skos:prefLabel "Geology Rock Properties - Statisitical Uncertainty Type "@en ;
    dcat:contactPoint "Team Lead - Information Services; Energy, Minerals and Groundwater Division" ;
.
