@prefix cs: <http://def.isotc211.org/iso19115/MD_CoverageContentTypeCode> .
@prefix dcterms: <http://purl.org/dc/terms/> .
@prefix rdfs: <http://www.w3.org/2000/01/rdf-schema#> .
@prefix sdo: <https://schema.org/> .
@prefix skos: <http://www.w3.org/2004/02/skos/core#> .
@prefix xsd: <http://www.w3.org/2001/XMLSchema#> .

<http://def.isotc211.org/iso19115/MD_CoverageContentTypeCode/auxilliaryInformation> a <http://def.isotc211.org/iso19115/-1/2014/ContentInformation#MD_CoverageContentTypeCode>,
        skos:Concept ;
    rdfs:isDefinedBy cs: ;
    skos:definition """calculation of the primary physicalMeasurement coverages in the dataset

EXAMPLE Grid of aerosol optical thickness used in the calculation of a sea surface temperature product."""^^xsd:string ;
    skos:inScheme cs: ;
    skos:prefLabel "auxilliary Information" ;
    skos:topConceptOf cs: .

<http://def.isotc211.org/iso19115/MD_CoverageContentTypeCode/coordinate> a <http://def.isotc211.org/iso19115/-1/2014/ContentInformation#MD_CoverageContentTypeCode>,
        skos:Concept ;
    rdfs:isDefinedBy cs: ;
    skos:definition "data used to provide coordinate axis values"^^xsd:string ;
    skos:inScheme cs: ;
    skos:prefLabel "coordinate" ;
    skos:topConceptOf cs: .

<http://def.isotc211.org/iso19115/MD_CoverageContentTypeCode/image> a <http://def.isotc211.org/iso19115/-1/2014/ContentInformation#MD_CoverageContentTypeCode>,
        skos:Concept ;
    rdfs:isDefinedBy cs: ;
    skos:definition "meaningful numerical representation of a physical parameter that is not the actual value of the physical parameter"^^xsd:string ;
    skos:inScheme cs: ;
    skos:prefLabel "image" ;
    skos:topConceptOf cs: .

<http://def.isotc211.org/iso19115/MD_CoverageContentTypeCode/modelResult> a <http://def.isotc211.org/iso19115/-1/2014/ContentInformation#MD_CoverageContentTypeCode>,
        skos:Concept ;
    rdfs:isDefinedBy cs: ;
    skos:definition "resources with values that are calculated using a model rather than being observed or calculated from observations"^^xsd:string ;
    skos:inScheme cs: ;
    skos:prefLabel "model Result" ;
    skos:topConceptOf cs: .

<http://def.isotc211.org/iso19115/MD_CoverageContentTypeCode/physicalMeasurement> a <http://def.isotc211.org/iso19115/-1/2014/ContentInformation#MD_CoverageContentTypeCode>,
        skos:Concept ;
    rdfs:isDefinedBy cs: ;
    skos:definition "value in physical units of the quantity being measured"^^xsd:string ;
    skos:inScheme cs: ;
    skos:prefLabel "physical Measurement" ;
    skos:topConceptOf cs: .

<http://def.isotc211.org/iso19115/MD_CoverageContentTypeCode/qualityInformation> a <http://def.isotc211.org/iso19115/-1/2014/ContentInformation#MD_CoverageContentTypeCode>,
        skos:Concept ;
    rdfs:isDefinedBy cs: ;
    skos:definition """data used to characterize the quality of the physicalMeasurement coverages in the dataset.
NOTE Typically included in a gmi:QE_CoverageResult."""^^xsd:string ;
    skos:inScheme cs: ;
    skos:prefLabel "quality Information" ;
    skos:topConceptOf cs: .

<http://def.isotc211.org/iso19115/MD_CoverageContentTypeCode/referenceInformation> a <http://def.isotc211.org/iso19115/-1/2014/ContentInformation#MD_CoverageContentTypeCode>,
        skos:Concept ;
    rdfs:isDefinedBy cs: ;
    skos:definition """reference information used to support the calculation or use of the physicalMeasurement coverages in the dataset
EXAMPLE Grids of latitude/longitude used to geolocate the physical measurements."""^^xsd:string ;
    skos:inScheme cs: ;
    skos:prefLabel "reference Information" ;
    skos:topConceptOf cs: .

<http://def.isotc211.org/iso19115/MD_CoverageContentTypeCode/thematicClassification> a <http://def.isotc211.org/iso19115/-1/2014/ContentInformation#MD_CoverageContentTypeCode>,
        skos:Concept ;
    rdfs:isDefinedBy cs: ;
    skos:definition "code value with no quantitative meaning, used to represent a physical quantity"^^xsd:string ;
    skos:inScheme cs: ;
    skos:prefLabel "thematic Classification" ;
    skos:topConceptOf cs: .

<https://linked.data.gov.au/org/ga> a sdo:Organization ;
    sdo:name "Geoscience Australia" ;
    sdo:url <https://www.ga.gov.au> .

<https://linked.data.gov.au/org/iso> a sdo:Organization ;
    sdo:name "International Organization for Standardization" ;
    sdo:url <https://www.iso.org> .

cs: a skos:ConceptScheme ;
    dcterms:created "2016-08-09T05:13:45.567000+00:00"^^xsd:dateTime ;
    dcterms:creator <https://linked.data.gov.au/org/iso> ;
    dcterms:modified "2016-08-09T05:13:01.362000+00:00"^^xsd:dateTime ;
    dcterms:publisher <https://linked.data.gov.au/org/iso> ;
    dcterms:source <http://standards.iso.org/iso/19115/-1/ed-1/en/> ;
    skos:definition "specific type of information represented in the cell"^^xsd:string ;
    skos:hasTopConcept <http://def.isotc211.org/iso19115/MD_CoverageContentTypeCode/auxilliaryInformation>,
        <http://def.isotc211.org/iso19115/MD_CoverageContentTypeCode/coordinate>,
        <http://def.isotc211.org/iso19115/MD_CoverageContentTypeCode/image>,
        <http://def.isotc211.org/iso19115/MD_CoverageContentTypeCode/modelResult>,
        <http://def.isotc211.org/iso19115/MD_CoverageContentTypeCode/physicalMeasurement>,
        <http://def.isotc211.org/iso19115/MD_CoverageContentTypeCode/qualityInformation>,
        <http://def.isotc211.org/iso19115/MD_CoverageContentTypeCode/referenceInformation>,
        <http://def.isotc211.org/iso19115/MD_CoverageContentTypeCode/thematicClassification> ;
    skos:prefLabel "MD Coverage Content Type Code - Concept Scheme" .

