@prefix cs: <http://def.isotc211.org/iso19115/-1/2014/ContentInformation/code/MD_ImagingConditionCode> .
@prefix dcterms: <http://purl.org/dc/terms/> .
@prefix sdo: <https://schema.org/> .
@prefix skos: <http://www.w3.org/2004/02/skos/core#> .
@prefix xsd: <http://www.w3.org/2001/XMLSchema#> .

<https://linked.data.gov.au/org/ga> a sdo:Organization ;
    sdo:name "Geoscience Australia" ;
    sdo:url <https://www.ga.gov.au> .

<http://registry.it.csiro.au/def/isotc211/MD_ImagingConditionCode/blurredImage> a <http://def.isotc211.org/iso19115/-1/2014/ContentInformation#MD_ImagingConditionCode>,
        skos:Concept ;
    dcterms:description "portion of the image is blurred"^^xsd:string ;
    dcterms:source <http://standards.iso.org/iso/19115/-1/ed-1/en/> ;
    skos:definition "portion of the image is blurred"^^xsd:string ;
    skos:inScheme cs: ;
    skos:prefLabel "blurred Image" ;
    skos:topConceptOf cs: .

<http://registry.it.csiro.au/def/isotc211/MD_ImagingConditionCode/cloud> a <http://def.isotc211.org/iso19115/-1/2014/ContentInformation#MD_ImagingConditionCode>,
        skos:Concept ;
    dcterms:description "portion of the image is partially obscured by cloud cover"^^xsd:string ;
    dcterms:source <http://standards.iso.org/iso/19115/-1/ed-1/en/> ;
    skos:definition "portion of the image is partially obscured by cloud cover"^^xsd:string ;
    skos:inScheme cs: ;
    skos:prefLabel "cloud" ;
    skos:topConceptOf cs: .

<http://registry.it.csiro.au/def/isotc211/MD_ImagingConditionCode/degradingObliquity> a <http://def.isotc211.org/iso19115/-1/2014/ContentInformation#MD_ImagingConditionCode>,
        skos:Concept ;
    dcterms:description "acute angle between the plane of the ecliptic (the plane of the Earth’s orbit) and the plane of the celestial equator"^^xsd:string ;
    dcterms:source <http://standards.iso.org/iso/19115/-1/ed-1/en/> ;
    skos:definition "acute angle between the plane of the ecliptic (the plane of the Earth’s orbit) and the plane of the celestial equator"^^xsd:string ;
    skos:inScheme cs: ;
    skos:prefLabel "degrading Obliquity" ;
    skos:topConceptOf cs: .

<http://registry.it.csiro.au/def/isotc211/MD_ImagingConditionCode/fog> a <http://def.isotc211.org/iso19115/-1/2014/ContentInformation#MD_ImagingConditionCode>,
        skos:Concept ;
    dcterms:description "portion of the image is partially obscured by fog"^^xsd:string ;
    dcterms:source <http://standards.iso.org/iso/19115/-1/ed-1/en/> ;
    skos:definition "portion of the image is partially obscured by fog"^^xsd:string ;
    skos:inScheme cs: ;
    skos:prefLabel "fog" ;
    skos:topConceptOf cs: .

<http://registry.it.csiro.au/def/isotc211/MD_ImagingConditionCode/heavySmokeOrDust> a <http://def.isotc211.org/iso19115/-1/2014/ContentInformation#MD_ImagingConditionCode>,
        skos:Concept ;
    dcterms:description "portion of the image is partially obscured by heavy smoke or dust"^^xsd:string ;
    dcterms:source <http://standards.iso.org/iso/19115/-1/ed-1/en/> ;
    skos:definition "portion of the image is partially obscured by heavy smoke or dust"^^xsd:string ;
    skos:inScheme cs: ;
    skos:prefLabel "heavy Smoke Or Dust" ;
    skos:topConceptOf cs: .

<http://registry.it.csiro.au/def/isotc211/MD_ImagingConditionCode/night> a <http://def.isotc211.org/iso19115/-1/2014/ContentInformation#MD_ImagingConditionCode>,
        skos:Concept ;
    dcterms:description "image was taken at night"^^xsd:string ;
    dcterms:source <http://standards.iso.org/iso/19115/-1/ed-1/en/> ;
    skos:definition "image was taken at night"^^xsd:string ;
    skos:inScheme cs: ;
    skos:prefLabel "night" ;
    skos:topConceptOf cs: .

<http://registry.it.csiro.au/def/isotc211/MD_ImagingConditionCode/rain> a <http://def.isotc211.org/iso19115/-1/2014/ContentInformation#MD_ImagingConditionCode>,
        skos:Concept ;
    dcterms:description "image was taken during rainfall"^^xsd:string ;
    dcterms:source <http://standards.iso.org/iso/19115/-1/ed-1/en/> ;
    skos:definition "image was taken during rainfall"^^xsd:string ;
    skos:inScheme cs: ;
    skos:prefLabel "rain" ;
    skos:topConceptOf cs: .

<http://registry.it.csiro.au/def/isotc211/MD_ImagingConditionCode/semiDarkness> a <http://def.isotc211.org/iso19115/-1/2014/ContentInformation#MD_ImagingConditionCode>,
        skos:Concept ;
    dcterms:description "image was taken during semi-dark conditions – twilight conditions"^^xsd:string ;
    dcterms:source <http://standards.iso.org/iso/19115/-1/ed-1/en/> ;
    skos:definition "image was taken during semi-dark conditions – twilight conditions"^^xsd:string ;
    skos:inScheme cs: ;
    skos:prefLabel "semi Darkness" ;
    skos:topConceptOf cs: .

<http://registry.it.csiro.au/def/isotc211/MD_ImagingConditionCode/shadow> a <http://def.isotc211.org/iso19115/-1/2014/ContentInformation#MD_ImagingConditionCode>,
        skos:Concept ;
    dcterms:description "portion of the image is obscured by shadow"^^xsd:string ;
    dcterms:source <http://standards.iso.org/iso/19115/-1/ed-1/en/> ;
    skos:definition "portion of the image is obscured by shadow"^^xsd:string ;
    skos:inScheme cs: ;
    skos:prefLabel "shadow" ;
    skos:topConceptOf cs: .

<http://registry.it.csiro.au/def/isotc211/MD_ImagingConditionCode/snow> a <http://def.isotc211.org/iso19115/-1/2014/ContentInformation#MD_ImagingConditionCode>,
        skos:Concept ;
    dcterms:description "portion of the image is obscured by snow"^^xsd:string ;
    dcterms:source <http://standards.iso.org/iso/19115/-1/ed-1/en/> ;
    skos:definition "portion of the image is obscured by snow"^^xsd:string ;
    skos:inScheme cs: ;
    skos:prefLabel "snow" ;
    skos:topConceptOf cs: .

<http://registry.it.csiro.au/def/isotc211/MD_ImagingConditionCode/terrainMasking> a <http://def.isotc211.org/iso19115/-1/2014/ContentInformation#MD_ImagingConditionCode>,
        skos:Concept ;
    dcterms:description "the absence of collection data of a given point or area caused by the relative location of topographic features which obstruct the collection path between the collector(s) and the subject(s) of interest"^^xsd:string ;
    dcterms:source <http://standards.iso.org/iso/19115/-1/ed-1/en/> ;
    skos:definition "the absence of collection data of a given point or area caused by the relative location of topographic features which obstruct the collection path between the collector(s) and the subject(s) of interest"^^xsd:string ;
    skos:inScheme cs: ;
    skos:prefLabel "terrain Masking" ;
    skos:topConceptOf cs: .

<https://linked.data.gov.au/org/iso> a sdo:Organization ;
    sdo:name "International Organization for Standardization" ;
    sdo:url <https://www.iso.org> .

cs: a skos:ConceptScheme ;
    dcterms:creator <https://linked.data.gov.au/org/iso> ;
    dcterms:publisher <https://linked.data.gov.au/org/ga> ;
    dcterms:published "2016-08-09T05:13:45.584000+00:00"^^xsd:dateTime ;
    dcterms:modified "2016-08-09T05:13:01.354000+00:00"^^xsd:dateTime ;
    dcterms:description "code which indicates conditions which may affect the image"^^xsd:string ;
    skos:hasTopConcept <http://registry.it.csiro.au/def/isotc211/MD_ImagingConditionCode/blurredImage>,
        <http://registry.it.csiro.au/def/isotc211/MD_ImagingConditionCode/cloud>,
        <http://registry.it.csiro.au/def/isotc211/MD_ImagingConditionCode/degradingObliquity>,
        <http://registry.it.csiro.au/def/isotc211/MD_ImagingConditionCode/fog>,
        <http://registry.it.csiro.au/def/isotc211/MD_ImagingConditionCode/heavySmokeOrDust>,
        <http://registry.it.csiro.au/def/isotc211/MD_ImagingConditionCode/night>,
        <http://registry.it.csiro.au/def/isotc211/MD_ImagingConditionCode/rain>,
        <http://registry.it.csiro.au/def/isotc211/MD_ImagingConditionCode/semiDarkness>,
        <http://registry.it.csiro.au/def/isotc211/MD_ImagingConditionCode/shadow>,
        <http://registry.it.csiro.au/def/isotc211/MD_ImagingConditionCode/snow>,
        <http://registry.it.csiro.au/def/isotc211/MD_ImagingConditionCode/terrainMasking> ;
    skos:prefLabel "MD Imaging Condition Code - Concept Scheme" .

