@prefix cs: <http://def.isotc211.org/iso19115/MD_TopologyLevelCode> .
@prefix dcterms: <http://purl.org/dc/terms/> .
@prefix rdfs: <http://www.w3.org/2000/01/rdf-schema#> .
@prefix sdo: <https://schema.org/> .
@prefix skos: <http://www.w3.org/2004/02/skos/core#> .
@prefix xsd: <http://www.w3.org/2001/XMLSchema#> .

<http://def.isotc211.org/iso19115/MD_TopologyLevelCode/abstract> a <http://def.isotc211.org/iso19115/-1/2014/SpatialRepresentationInformation#MD_TopologyLevelCode>,
        skos:Concept ;
    rdfs:isDefinedBy cs: ;
    skos:definition "topological complex without any specified geometric realisation"^^xsd:string ;
    skos:inScheme cs: ;
    skos:prefLabel "abstract" ;
    skos:topConceptOf cs: .

<http://def.isotc211.org/iso19115/MD_TopologyLevelCode/fullPlanarGraph> a <http://def.isotc211.org/iso19115/-1/2014/SpatialRepresentationInformation#MD_TopologyLevelCode>,
        skos:Concept ;
    rdfs:isDefinedBy cs: ;
    skos:definition """2-dimensional topological complex that is planar
NOTE A 2-dimensional topological complex is commonly called “full topology” in a cartographic 2D environment."""^^xsd:string ;
    skos:inScheme cs: ;
    skos:prefLabel "full Planar Graph" ;
    skos:topConceptOf cs: .

<http://def.isotc211.org/iso19115/MD_TopologyLevelCode/fullSurfaceGraph> a <http://def.isotc211.org/iso19115/-1/2014/SpatialRepresentationInformation#MD_TopologyLevelCode>,
        skos:Concept ;
    rdfs:isDefinedBy cs: ;
    skos:definition """1-dimensional topological complex that is isomorphic to a subset of a surface
NOTE A geometric complex is isomorphic to a topological complex if their elements are in a one-to-one, dimensional-and boundary-preserving correspondence to one another."""^^xsd:string ;
    skos:inScheme cs: ;
    skos:prefLabel "full Surface Graph" ;
    skos:topConceptOf cs: .

<http://def.isotc211.org/iso19115/MD_TopologyLevelCode/fullTopology3D> a <http://def.isotc211.org/iso19115/-1/2014/SpatialRepresentationInformation#MD_TopologyLevelCode>,
        skos:Concept ;
    rdfs:isDefinedBy cs: ;
    skos:definition "complete coverage of a 3D Euclidean coordinate space"^^xsd:string ;
    skos:inScheme cs: ;
    skos:prefLabel "full Topology 3D" ;
    skos:topConceptOf cs: .

<http://def.isotc211.org/iso19115/MD_TopologyLevelCode/geometryOnly> a <http://def.isotc211.org/iso19115/-1/2014/SpatialRepresentationInformation#MD_TopologyLevelCode>,
        skos:Concept ;
    rdfs:isDefinedBy cs: ;
    skos:definition "geometry objects without any additional structure which describes topology"^^xsd:string ;
    skos:inScheme cs: ;
    skos:prefLabel "geometry Only" ;
    skos:topConceptOf cs: .

<http://def.isotc211.org/iso19115/MD_TopologyLevelCode/planarGraph> a <http://def.isotc211.org/iso19115/-1/2014/SpatialRepresentationInformation#MD_TopologyLevelCode>,
        skos:Concept ;
    rdfs:isDefinedBy cs: ;
    skos:definition """1-dimensional topological complex that is planar
NOTE A planar graph is a graph that can be drawn in a plane in such a way that no two edges intersect except at a vertex."""^^xsd:string ;
    skos:inScheme cs: ;
    skos:prefLabel "planar Graph" ;
    skos:topConceptOf cs: .

<http://def.isotc211.org/iso19115/MD_TopologyLevelCode/surfaceGraph> a <http://def.isotc211.org/iso19115/-1/2014/SpatialRepresentationInformation#MD_TopologyLevelCode>,
        skos:Concept ;
    rdfs:isDefinedBy cs: ;
    skos:definition """1-dimensional topological complex that is isomorphic to a subset of a surface
NOTE A geometric complex is isomorphic to a topological complex if their elements are in a one-to-one, dimensional-and boundary-preserving correspondence to one another."""^^xsd:string ;
    skos:inScheme cs: ;
    skos:prefLabel "surface Graph" ;
    skos:topConceptOf cs: .

<http://def.isotc211.org/iso19115/MD_TopologyLevelCode/topology1D> a <http://def.isotc211.org/iso19115/-1/2014/SpatialRepresentationInformation#MD_TopologyLevelCode>,
        skos:Concept ;
    rdfs:isDefinedBy cs: ;
    skos:definition "1-dimensional topological complex – commonly called “chain-node” topology"^^xsd:string ;
    skos:inScheme cs: ;
    skos:prefLabel "topology 1D" ;
    skos:topConceptOf cs: .

<http://def.isotc211.org/iso19115/MD_TopologyLevelCode/topology3D> a <http://def.isotc211.org/iso19115/-1/2014/SpatialRepresentationInformation#MD_TopologyLevelCode>,
        skos:Concept ;
    rdfs:isDefinedBy cs: ;
    skos:definition """3-dimensional topological complex
NOTE A topological complex is a collection of topological primitives that are closed under the boundary operations."""^^xsd:string ;
    skos:inScheme cs: ;
    skos:prefLabel "topology 3D" ;
    skos:topConceptOf cs: .

<https://linked.data.gov.au/org/ga> a sdo:Organization ;
    sdo:name "Geoscience Australia" ;
    sdo:url <https://www.ga.gov.au> .

<https://linked.data.gov.au/org/iso> a sdo:Organization ;
    sdo:name "International Organization for Standardization" ;
    sdo:url <https://www.iso.org> .

cs: a skos:ConceptScheme ;
    dcterms:created "2016-08-09T05:13:45.652000+00:00"^^xsd:dateTime ;
    dcterms:creator <https://linked.data.gov.au/org/iso> ;
    dcterms:modified "2016-08-09T05:13:01.227000+00:00"^^xsd:dateTime ;
    dcterms:publisher <https://linked.data.gov.au/org/ga> ;
    dcterms:source <http://standards.iso.org/iso/19115/-1/ed-1/en/> ;
    skos:definition "degree of complexity of the spatial relationships"^^xsd:string ;
    skos:hasTopConcept <http://def.isotc211.org/iso19115/MD_TopologyLevelCode/abstract>,
        <http://def.isotc211.org/iso19115/MD_TopologyLevelCode/fullPlanarGraph>,
        <http://def.isotc211.org/iso19115/MD_TopologyLevelCode/fullSurfaceGraph>,
        <http://def.isotc211.org/iso19115/MD_TopologyLevelCode/fullTopology3D>,
        <http://def.isotc211.org/iso19115/MD_TopologyLevelCode/geometryOnly>,
        <http://def.isotc211.org/iso19115/MD_TopologyLevelCode/planarGraph>,
        <http://def.isotc211.org/iso19115/MD_TopologyLevelCode/surfaceGraph>,
        <http://def.isotc211.org/iso19115/MD_TopologyLevelCode/topology1D>,
        <http://def.isotc211.org/iso19115/MD_TopologyLevelCode/topology3D> ;
    skos:prefLabel "MD Topology Level Code - Concept Scheme" .

