@prefix cs: <http://def.isotc211.org/iso19115/SV_CouplingType> .
@prefix dcterms: <http://purl.org/dc/terms/> .
@prefix rdfs: <http://www.w3.org/2000/01/rdf-schema#> .
@prefix sdo: <https://schema.org/> .
@prefix skos: <http://www.w3.org/2004/02/skos/core#> .
@prefix xsd: <http://www.w3.org/2001/XMLSchema#> .

<http://def.isotc211.org/iso19115/SV_CouplingType/loose> a <http://def.isotc211.org/iso19115/-1/2014/ServiceMetadataInformation#SV_CouplingType>,
        skos:Concept ;
    rdfs:isDefinedBy cs: ;
    skos:definition "service instance is loosely coupled with a data instance, i.e. no MD_DataIdentification class has to be described"^^xsd:string ;
    skos:inScheme cs: ;
    skos:prefLabel "loose" ;
    skos:topConceptOf cs: .

<http://def.isotc211.org/iso19115/SV_CouplingType/mixed> a <http://def.isotc211.org/iso19115/-1/2014/ServiceMetadataInformation#SV_CouplingType>,
        skos:Concept ;
    rdfs:isDefinedBy cs: ;
    skos:definition "service instance is mixed coupled with a data instance, i.e. MD_DataIdentification describes the associated data instance and additionally the service instance might work with other external data instances"^^xsd:string ;
    skos:inScheme cs: ;
    skos:prefLabel "mixed" ;
    skos:topConceptOf cs: .

<http://def.isotc211.org/iso19115/SV_CouplingType/tight> a <http://def.isotc211.org/iso19115/-1/2014/ServiceMetadataInformation#SV_CouplingType>,
        skos:Concept ;
    rdfs:isDefinedBy cs: ;
    skos:definition "service instance is tightly coupled with a data instance, i.e. MD_DataIdentification class MUST be described"^^xsd:string ;
    skos:inScheme cs: ;
    skos:prefLabel "tight" ;
    skos:topConceptOf cs: .

<https://linked.data.gov.au/org/ga> a sdo:Organization ;
    sdo:name "Geoscience Australia" ;
    sdo:url <https://www.ga.gov.au> .

<https://linked.data.gov.au/org/iso> a sdo:Organization ;
    sdo:name "International Organization for Standardization" ;
    sdo:url <https://www.iso.org> .

cs: a skos:ConceptScheme ;
    dcterms:created "2016-08-09T05:13:45.662000+00:00"^^xsd:dateTime ;
    dcterms:creator <https://linked.data.gov.au/org/iso> ;
    dcterms:modified "2016-08-09T05:13:01.301000+00:00"^^xsd:dateTime ;
    dcterms:publisher <https://linked.data.gov.au/org/ga> ;
    dcterms:source <http://standards.iso.org/iso/19115/-1/ed-1/en/> ;
    skos:definition "class of information to which the referencing entity applies"^^xsd:string ;
    skos:hasTopConcept <http://def.isotc211.org/iso19115/SV_CouplingType/loose>,
        <http://def.isotc211.org/iso19115/SV_CouplingType/mixed>,
        <http://def.isotc211.org/iso19115/SV_CouplingType/tight> ;
    skos:prefLabel "SV Coupling Type - Concept Scheme" .

